@prefix schema: <https://schema.org/>.
@prefix skos: <http://www.w3.org/2004/02/skos/core#>.
@prefix rdf: <http://www.w3.org/1999/02/22-rdf-syntax-ns#>.
@prefix rdfs: <http://www.w3.org/2000/01/rdf-schema#>.
@prefix foaf: <http://xmlns.com/foaf/0.1/>.
@prefix xsd: <http://www.w3.org/2001/XMLSchema#>.
@prefix dcterms: <http://purl.org/dc/terms/>.
@prefix owl: <http://www.w3.org/2002/07/owl#>.
@prefix jsonsc: <https://www.w3.org/2019/wot/json-schema#>.
@prefix gbfs: <https://w3id.org/gbfs#>.
@prefix jsonsc-ld: <http://w3id.org/jsonsc-ld/>.
@prefix api: <http://purl.org/linked-data/api/vocab>.
@prefix geo: <http://www.w3.org/2003/01/geo/wgs84_pos#>.
@prefix mobivoc: <http://schema.mobivoc.org/#>.
@prefix geosparql: <http://www.opengis.net/ont/geosparql#>.

<https://github.com/NABSA/gbfs/blob/v2.3-RC/gbfs.md#station_informationjson-ld> rdf:type jsonsc-ld:Schema;
    jsonsc-ld:enriches <https://github.com/NABSA/gbfs/blob/v1.0/gbfs.md#free_bike_statusjson>.
<https://github.com/NABSA/gbfs/blob/v1.0/gbfs.md#free_bike_statusjson> rdf:type rdfs:Class.
<https://github.com/NABSA/gbfs/blob/v2.3-RC/gbfs.md#station_informationjson-ld> dcterms:title "The GBFS LD configuration";
    dcterms:description "A file containing extra configuration to map the GBFS json schemas to an RDFS vocabulary";
    dcterms:creator <https://pietercolpaert.be/#me>, <https://w3id.org/people/brechtvdv/#me>, <https://data.knows.idlab.ugent.be/person/andreipopescu/#me>, <https://data.knows.idlab.ugent.be/person/jilong/#me>;
    dcterms:license "MIT";
    dcterms:rights "Copyright statement";
    dcterms:modified "2022-06-02T11:32:52.12679".
<https://github.com/NABSA/gbfs/blob/v1.0/gbfs.md#free_bike_statusjson> dcterms:description "Describes the vehicles that are available for rent (as of v2.1-RC2).".
dcterms:modified rdfs:domain <https://github.com/NABSA/gbfs/blob/v1.0/gbfs.md#free_bike_statusjson>;
    rdfs:range xsd:integer.
gbfs:ttl dcterms:description "Number of seconds before the data in the feed will be updated again (0 if the data should always be refreshed).";
    rdf:type rdf:Property;
    rdfs:label "ttl";
    rdfs:domain <https://github.com/NABSA/gbfs/blob/v1.0/gbfs.md#free_bike_statusjson>;
    rdfs:range xsd:integer.
gbfs:Bike dcterms:description "bikes that are available for rent";
    rdf:type rdfs:Class;
    rdfs:label "Bike".
dcterms:identifier rdfs:domain gbfs:Bike;
    rdfs:range xsd:string.
geo:lat rdfs:domain gbfs:Bike;
    rdfs:range xsd:decimal.
geo:long rdfs:domain gbfs:Bike;
    rdfs:range xsd:decimal.
gbfs:is_reserved dcterms:description "Is the vehicle currently reserved?";
    rdf:type rdf:Property;
    rdfs:label "is_reserved";
    rdfs:domain <https://github.com/NABSA/gbfs/blob/v1.0/gbfs.md#free_bike_statusjson>.
gbfs:is_disabled dcterms:description "Is the vehicle currently disabled (broken)?";
    rdf:type rdf:Property;
    rdfs:label "is_disabled";
    rdfs:domain <https://github.com/NABSA/gbfs/blob/v1.0/gbfs.md#free_bike_statusjson>.
