@prefix schema: <http://schema.org/#>.
@prefix skos: <http://www.w3.org/2004/02/skos/core#>.
@prefix rdf: <http://www.w3.org/1999/02/22-rdf-syntax-ns#>.
@prefix rdfs: <http://www.w3.org/2000/01/rdf-schema#>.
@prefix foaf: <http://xmlns.com/foaf/0.1/>.
@prefix xsd: <http://www.w3.org/2001/XMLSchema#>.
@prefix dcterms: <http://purl.org/dc/terms/>.
@prefix owl: <http://www.w3.org/2002/07/owl#>.
@prefix jsonsc: <https://www.w3.org/2019/wot/json-schema#>.
@prefix gbfs: <https://w3id.org/gbfs#>.
@prefix jsonsc-ld: <http://w3id.org/jsonsc-ld/>.
@prefix api: <http://purl.org/linked-data/api/vocab>.
@prefix geo: <http://www.w3.org/2003/01/geo/wgs84_pos#>.

<https://github.com/NABSA/gbfs/blob/v2.3-RC/gbfs.md#station_informationjson-ld> rdf:type jsonsc-ld:Schema;
    jsonsc-ld:enriches <https://github.com/NABSA/gbfs/blob/v2.3/gbfs.md#station_statusjson>.
<https://github.com/NABSA/gbfs/blob/v2.3/gbfs.md#station_statusjson> rdf:type rdfs:Class.
<https://github.com/NABSA/gbfs/blob/v2.3-RC/gbfs.md#station_informationjson-ld> dcterms:title "The GBFS LD configuration";
    dcterms:description "A file containing extra configuration to map the GBFS json schemas to an RDFS vocabulary";
    dcterms:creator <https://pietercolpaert.be/#me>, <https://w3id.org/people/brechtvdv/#me>, <https://data.knows.idlab.ugent.be/person/andreipopescu/#me>, <https://data.knows.idlab.ugent.be/person/jilong/#me>;
    dcterms:license "MIT";
    dcterms:rights "Copyright statement";
    dcterms:modified "2022-06-02T11:32:52.12679".
<https://github.com/NABSA/gbfs/blob/v2.3/gbfs.md#station_statusjson> dcterms:description "Describes the capacity and rental availability of the station".
dcterms:modified rdfs:domain <https://github.com/NABSA/gbfs/blob/v2.3/gbfs.md#station_statusjson>;
    rdfs:range xsd:integer.
gbfs:ttl dcterms:description "Number of seconds before the data in the feed will be updated again (0 if the data should always be refreshed).";
    rdf:type rdf:Property;
    rdfs:label "ttl";
    rdfs:domain <https://github.com/NABSA/gbfs/blob/v2.3/gbfs.md#station_statusjson>;
    rdfs:range xsd:integer.
gbfs:Station rdf:type rdfs:Class;
    rdfs:label "Station".
dcterms:identifier rdfs:domain gbfs:Station;
    rdfs:range xsd:string.
gbfs:num_bikes_available dcterms:description "Number of vehicles of any type physically available for rental at the station.";
    rdf:type rdf:Property;
    rdfs:label "num_bikes_available";
    rdfs:domain gbfs:Station;
    rdfs:range xsd:integer.
gbfs:VehicleTypeAvailable dcterms:description "Array of objects displaying the total number of each vehicle type at the station (added in v2.1-RC).";
    rdf:type rdfs:Class;
    rdfs:label "VehicleTypeAvailable".
gbfs:vehicle_type_id dcterms:description "The vehicle_type_id of vehicle at the station (added in v2.1-RC).";
    rdf:type rdf:Property;
    rdfs:label "vehicle_type_id";
    rdfs:domain gbfs:VehicleTypeAvailable;
    rdfs:range xsd:string.
gbfs:count dcterms:description "A number representing the total amount of this vehicle type at the station (added in v2.1-RC).";
    rdf:type rdf:Property;
    rdfs:label "count";
    rdfs:domain gbfs:VehicleTypeAvailable;
    rdfs:range xsd:integer.
gbfs:num_bikes_disabled dcterms:description "Number of disabled vehicles of any type at the station.";
    rdf:type rdf:Property;
    rdfs:label "num_bikes_disabled";
    rdfs:domain gbfs:Station;
    rdfs:range xsd:integer.
gbfs:num_docks_available dcterms:description "Number of functional docks physically at the station.";
    rdf:type rdf:Property;
    rdfs:label "num_docks_available";
    rdfs:domain gbfs:Station;
    rdfs:range xsd:integer.
gbfs:num_docks_disabled dcterms:description "Number of empty but disabled docks at the station.";
    rdf:type rdf:Property;
    rdfs:label "num_docks_disabled";
    rdfs:domain gbfs:Station;
    rdfs:range xsd:integer.
gbfs:is_installed dcterms:description "Is the station currently on the street?";
    rdf:type rdf:Property;
    rdfs:label "is_installed";
    rdfs:domain gbfs:Station;
    rdfs:range xsd:boolean.
gbfs:is_renting dcterms:description "Is the station currently renting vehicles?";
    rdf:type rdf:Property;
    rdfs:label "is_renting";
    rdfs:domain gbfs:Station;
    rdfs:range xsd:boolean.
gbfs:is_returning dcterms:description "Is the station accepting vehicle returns?";
    rdf:type rdf:Property;
    rdfs:label "is_returning";
    rdfs:domain gbfs:Station;
    rdfs:range xsd:boolean.
gbfs:last_reported dcterms:description "The last time this station reported its status to the operator's backend in POSIX time.";
    rdf:type rdf:Property;
    rdfs:label "last_reported";
    rdfs:domain gbfs:Station;
    rdfs:range xsd:integer.
gbfs:VehicleDocksAvailable dcterms:description "Object displaying available docks by vehicle type (added in v2.1-RC).";
    rdf:type rdfs:Class;
    rdfs:label "VehicleDocksAvailable".
gbfs:vehicle_type_ids rdf:type rdf:Property;
    rdfs:label "vehicle_type_ids";
    rdfs:domain gbfs:VehicleDocksAvailable;
    rdfs:range xsd:string.
gbfs:count dcterms:description "A number representing the total number of available docks for the defined vehicle type (added in v2.1-RC).";
    rdf:type rdf:Property;
    rdfs:label "count";
    rdfs:domain gbfs:VehicleDocksAvailable;
    rdfs:range xsd:integer.
