@prefix schema: <http://schema.org/#>.
@prefix skos: <http://www.w3.org/2004/02/skos/core#>.
@prefix rdf: <http://www.w3.org/1999/02/22-rdf-syntax-ns#>.
@prefix rdfs: <http://www.w3.org/2000/01/rdf-schema#>.
@prefix foaf: <http://xmlns.com/foaf/0.1/>.
@prefix xsd: <http://www.w3.org/2001/XMLSchema#>.
@prefix dcterms: <http://purl.org/dc/terms/>.
@prefix owl: <http://www.w3.org/2002/07/owl#>.
@prefix jsonsc: <https://www.w3.org/2019/wot/json-schema#>.
@prefix gbfs: <https://w3id.org/gbfs#>.
@prefix jsonsc-ld: <http://w3id.org/jsonsc-ld/>.
@prefix api: <http://purl.org/linked-data/api/vocab>.
@prefix geo: <http://www.w3.org/2003/01/geo/wgs84_pos#>.

<https://github.com/NABSA/gbfs/blob/v2.3-RC/gbfs.md#station_informationjson-ld> rdf:type jsonsc-ld:Schema;
    jsonsc-ld:enriches <https://github.com/NABSA/gbfs/blob/v2.3-RC/gbfs.md#system_regionsjson>.
<https://github.com/NABSA/gbfs/blob/v2.3-RC/gbfs.md#system_regionsjson> rdf:type rdfs:Class.
<https://github.com/NABSA/gbfs/blob/v2.3-RC/gbfs.md#station_informationjson-ld> dcterms:title "The GBFS LD configuration";
    dcterms:description "A file containing extra configuration to map the GBFS json schemas to an RDFS vocabulary";
    dcterms:creator <https://pietercolpaert.be/#me>, <https://w3id.org/people/brechtvdv/#me>, <https://data.knows.idlab.ugent.be/person/andreipopescu/#me>, <https://data.knows.idlab.ugent.be/person/jilong/#me>;
    dcterms:license "MIT";
    dcterms:rights "Copyright statement";
    dcterms:modified "2022-06-02T11:32:52.12679".
<https://github.com/NABSA/gbfs/blob/v2.3-RC/gbfs.md#system_regionsjson> dcterms:description "Describes regions for a system that is broken up by geographic or political region.".
dcterms:modified rdfs:domain <https://github.com/NABSA/gbfs/blob/v2.3-RC/gbfs.md#system_regionsjson>;
    rdfs:range xsd:integer.
gbfs:ttl dcterms:description "Number of seconds before the data in the feed will be updated again (0 if the data should always be refreshed).";
    rdf:type rdf:Property;
    rdfs:label "ttl";
    rdfs:domain <https://github.com/NABSA/gbfs/blob/v2.3-RC/gbfs.md#system_regionsjson>;
    rdfs:range xsd:integer.
gbfs:Region dcterms:description "Array of regions.";
    rdf:type rdfs:Class;
    rdfs:label "Region".
gbfs:region_id dcterms:description "identifier of the region.";
    rdf:type rdf:Property;
    rdfs:label "region_id";
    rdfs:domain gbfs:Region;
    rdfs:range xsd:string.
gbfs:name dcterms:description "Public name for this region.";
    rdf:type rdf:Property;
    rdfs:label "name";
    rdfs:domain gbfs:Region;
    rdfs:range xsd:string.
