@prefix schema: <http://schema.org/#>.
@prefix skos: <http://www.w3.org/2004/02/skos/core#>.
@prefix rdf: <http://www.w3.org/1999/02/22-rdf-syntax-ns#>.
@prefix rdfs: <http://www.w3.org/2000/01/rdf-schema#>.
@prefix foaf: <http://xmlns.com/foaf/0.1/>.
@prefix xsd: <http://www.w3.org/2001/XMLSchema#>.
@prefix dcterms: <http://purl.org/dc/terms/>.
@prefix owl: <http://www.w3.org/2002/07/owl#>.
@prefix jsonsc: <https://www.w3.org/2019/wot/json-schema#>.
@prefix gbfs: <https://w3id.org/gbfs#>.
@prefix jsonsc-ld: <http://w3id.org/jsonsc-ld/>.
@prefix api: <http://purl.org/linked-data/api/vocab>.

<https://github.com/NABSA/gbfs/blob/v2.3-RC/gbfs.md#station_informationjson-ld> rdf:type jsonsc-ld:Schema;
    jsonsc-ld:enriches <https://github.com/NABSA/gbfs/blob/v2.3-RC/gbfs.md#system_pricing_plansjson>.
<https://github.com/NABSA/gbfs/blob/v2.3-RC/gbfs.md#system_pricing_plansjson> rdf:type rdfs:Class.
<https://github.com/NABSA/gbfs/blob/v2.3-RC/gbfs.md#station_informationjson-ld> dcterms:title "The GBFS LD configuration";
    dcterms:description "A file containing extra configuration to map the GBFS json schemas to an RDFS vocabulary";
    dcterms:creator <https://pietercolpaert.be/#me>, <https://w3id.org/people/brechtvdv/#me>, <https://data.knows.idlab.ugent.be/person/andreipopescu/#me>, <https://data.knows.idlab.ugent.be/person/jilong/#me>;
    dcterms:license "MIT";
    dcterms:rights "Copyright statement";
    dcterms:modified "2022-06-02T11:32:52.12679".
<https://github.com/NABSA/gbfs/blob/v2.3-RC/gbfs.md#system_pricing_plansjson> dcterms:description "Describes the pricing schemes of the system.".
dcterms:modified rdfs:domain <https://github.com/NABSA/gbfs/blob/v2.3-RC/gbfs.md#system_pricing_plansjson>;
    rdfs:range xsd:integer.
gbfs:ttl dcterms:description "Number of seconds before the data in the feed will be updated again (0 if the data should always be refreshed).";
    rdf:type rdf:Property;
    rdfs:domain <https://github.com/NABSA/gbfs/blob/v2.3-RC/gbfs.md#system_pricing_plansjson>;
    rdfs:range xsd:integer.
gbfs:PricePlan rdf:type rdfs:Class.
gbfs:plan_id dcterms:description "Identifier of a pricing plan in the system.";
    rdf:type rdf:Property;
    rdfs:domain gbfs:PricePlan;
    rdfs:range xsd:string.
gbfs:url dcterms:description "URL where the customer can learn more about this pricing plan.";
    rdf:type rdf:Property;
    rdfs:domain gbfs:PricePlan;
    rdfs:range xsd:string.
gbfs:name dcterms:description "Name of this pricing plan.";
    rdf:type rdf:Property;
    rdfs:domain gbfs:PricePlan;
    rdfs:range xsd:string.
gbfs:currency dcterms:description "Currency used to pay the fare in ISO 4217 code.";
    rdf:type rdf:Property;
    rdfs:domain gbfs:PricePlan;
    rdfs:range xsd:string.
gbfs:price dcterms:description "Fare price.";
    rdf:type rdf:Property;
    rdfs:domain gbfs:PricePlan;
    rdfs:range xsd:decimal.
gbfs:is_taxable dcterms:description "Will additional tax be added to the base price?";
    rdf:type rdf:Property;
    rdfs:domain gbfs:PricePlan;
    rdfs:range xsd:boolean.
gbfs:description dcterms:description "Customer-readable description of the pricing plan.";
    rdf:type rdf:Property;
    rdfs:domain gbfs:PricePlan;
    rdfs:range xsd:string.
gbfs:PerKmPrice dcterms:description "Array of segments when the price is a function of distance travelled, displayed in kilometers (added in v2.1-RC2).";
    rdf:type rdfs:Class.
gbfs:start dcterms:description "Number of kilometers that have to elapse before this segment starts applying (added in v2.1-RC2).";
    rdf:type rdf:Property;
    rdfs:domain gbfs:PerKmPrice;
    rdfs:range xsd:integer.
gbfs:rate dcterms:description "Rate that is charged for each kilometer interval after the start (added in v2.1-RC2).";
    rdf:type rdf:Property;
    rdfs:domain gbfs:PerKmPrice;
    rdfs:range xsd:decimal.
gbfs:interval dcterms:description "Interval in kilometers at which the rate of this segment is either reapplied indefinitely, or if defined, up until (but not including) end kilometer (added in v2.1-RC2).";
    rdf:type rdf:Property;
    rdfs:domain gbfs:PerKmPrice;
    rdfs:range xsd:integer.
gbfs:end dcterms:description "The kilometer at which the rate will no longer apply (added in v2.1-RC2).";
    rdf:type rdf:Property;
    rdfs:domain gbfs:PerKmPrice;
    rdfs:range xsd:integer.
gbfs:PerMinPrice dcterms:description "Array of segments when the price is a function of time travelled, displayed in minutes (added in v2.1-RC2).";
    rdf:type rdfs:Class.
gbfs:start dcterms:description "Number of minutes that have to elapse before this segment starts applying (added in v2.1-RC2).";
    rdf:type rdf:Property;
    rdfs:domain gbfs:PerMinPrice;
    rdfs:range xsd:integer.
gbfs:rate dcterms:description "Rate that is charged for each minute interval after the start (added in v2.1-RC2).";
    rdf:type rdf:Property;
    rdfs:domain gbfs:PerMinPrice;
    rdfs:range xsd:decimal.
gbfs:interval dcterms:description "Interval in minutes at which the rate of this segment is either reapplied (added in v2.1-RC2).";
    rdf:type rdf:Property;
    rdfs:domain gbfs:PerMinPrice;
    rdfs:range xsd:integer.
gbfs:end dcterms:description "The minute at which the rate will no longer apply (added in v2.1-RC2).";
    rdf:type rdf:Property;
    rdfs:domain gbfs:PerMinPrice;
    rdfs:range xsd:integer.
gbfs:surge_pricing dcterms:description "Is there currently an increase in price in response to increased demand in this pricing plan? (added in v2.1-RC2)";
    rdf:type rdf:Property;
    rdfs:domain gbfs:PricePlan;
    rdfs:range xsd:boolean.
