@prefix schema: <https://schema.org/>.
@prefix skos: <http://www.w3.org/2004/02/skos/core#>.
@prefix rdf: <http://www.w3.org/1999/02/22-rdf-syntax-ns#>.
@prefix rdfs: <http://www.w3.org/2000/01/rdf-schema#>.
@prefix foaf: <http://xmlns.com/foaf/0.1/>.
@prefix xsd: <http://www.w3.org/2001/XMLSchema#>.
@prefix dcterms: <http://purl.org/dc/terms/>.
@prefix owl: <http://www.w3.org/2002/07/owl#>.
@prefix jsonsc: <https://www.w3.org/2019/wot/json-schema#>.
@prefix jsonsc-ld: <http://w3id.org/jsonsc-ld/>.
@prefix api: <http://purl.org/linked-data/api/vocab>.
@prefix geo: <http://www.w3.org/2003/01/geo/wgs84_pos#>.
@prefix mobivoc: <http://schema.mobivoc.org/#>.
@prefix geosparql: <http://www.opengis.net/ont/geosparql#>.
@prefix gbfs: <https://w3id.org/gbfs#>.

<https://github.com/NABSA/gbfs/blob/v2.3/gbfs.md#gbfsjson> dcterms:description "Auto-discovery file that links to all of the other files published by the system.".
gbfs:last_updated dcterms:description "Last time the data in the feed was updated in POSIX time.";
    rdf:type rdf:Property;
    rdfs:label "last_updated";
    rdfs:domain <https://github.com/NABSA/gbfs/blob/v2.3/gbfs.md#gbfsjson>;
    rdfs:range xsd:integer.
gbfs:ttl dcterms:description "Number of seconds before the data in the feed will be updated again (0 if the data should always be refreshed).";
    rdf:type rdf:Property;
    rdfs:label "ttl";
    rdfs:domain <https://github.com/NABSA/gbfs/blob/v2.3/gbfs.md#gbfsjson>;
    rdfs:range xsd:integer.
gbfs:version dcterms:description "GBFS version number to which the feed conforms, according to the versioning framework (added in v1.1).";
    rdf:type rdf:Property;
    rdfs:label "version";
    rdfs:domain <https://github.com/NABSA/gbfs/blob/v2.3/gbfs.md#gbfsjson>;
    rdfs:range xsd:string.
gbfs:data dcterms:description "Response data in the form of name:value pairs.";
    rdf:type rdf:Property;
    rdfs:label "data";
    rdfs:domain <https://github.com/NABSA/gbfs/blob/v2.3/gbfs.md#gbfsjson>;
    rdfs:range gbfs:Datum.
gbfs:Datum rdf:type rdfs:Class;
    rdfs:label "Datum".
gbfs:feeds dcterms:description "An array of all of the feeds that are published by the auto-discovery file. Each element in the array is an object with the keys below.";
    rdf:type rdf:Property;
    rdfs:label "feeds";
    rdfs:domain gbfs:Datum;
    rdfs:range gbfs:Feed.
gbfs:Feed rdf:type rdfs:Class;
    rdfs:label "Feed".
gbfs:name dcterms:description "Key identifying the type of feed this is. The key must be the base file name defined in the spec for the corresponding feed type.";
    rdf:type rdf:Property;
    rdfs:label "name";
    rdfs:domain gbfs:Feed.
gbfs:Name rdf:type skos:ConceptScheme.
gbfs:name rdfs:range [
  owl:oneOf ()
].
gbfs:url dcterms:description "URL for the feed.";
    rdf:type rdf:Property;
    rdfs:label "url";
    rdfs:domain gbfs:Feed;
    rdfs:range xsd:anyURI.
