@prefix schema: <https://schema.org/>.
@prefix skos: <http://www.w3.org/2004/02/skos/core#>.
@prefix rdf: <http://www.w3.org/1999/02/22-rdf-syntax-ns#>.
@prefix rdfs: <http://www.w3.org/2000/01/rdf-schema#>.
@prefix foaf: <http://xmlns.com/foaf/0.1/>.
@prefix xsd: <http://www.w3.org/2001/XMLSchema#>.
@prefix dcterms: <http://purl.org/dc/terms/>.
@prefix owl: <http://www.w3.org/2002/07/owl#>.
@prefix jsonsc: <https://www.w3.org/2019/wot/json-schema#>.
@prefix jsonsc-ld: <http://w3id.org/jsonsc-ld/>.
@prefix api: <http://purl.org/linked-data/api/vocab>.
@prefix geo: <http://www.w3.org/2003/01/geo/wgs84_pos#>.
@prefix mobivoc: <http://schema.mobivoc.org/#>.
@prefix geosparql: <http://www.opengis.net/ont/geosparql#>.
@prefix sdm: <https://w3id.org/sdm#>.

<https://smart-data-models.github.io/dataModel.Weather/WeatherObserved/schema.json> dcterms:title "Weather Observed schema - Smart Data Models";
    dcterms:description "An observation of weather conditions at a certain place and time. This data model has been developed in cooperation with mobile operators and the GSMA.".
sdm:type dcterms:description "Property. NGSI Entity type. It has to be WeatherObserved";
    rdf:type rdf:Property;
    rdfs:label "type";
    rdfs:domain <https://smart-data-models.github.io/dataModel.Weather/WeatherObserved/schema.json>.
sdm:Type rdf:type skos:ConceptScheme.
sdm:type rdfs:range [
  owl:oneOf (sdm:WeatherObserved)
].
sdm:WeatherObserved rdf:type skos:Concept;
    skos:inScheme sdm:Type;
    rdfs:label "WeatherObserved".
sdm:precipitation dcterms:description "Property. Model:'https://schema.org/Number'. Amount of water rain registered. Units:'Liters per square meter'. ";
    rdf:type rdf:Property;
    rdfs:label "precipitation";
    rdfs:domain <https://smart-data-models.github.io/dataModel.Weather/WeatherObserved/schema.json>;
    rdfs:range xsd:decimal.
sdm:solarRadiation dcterms:description "Property. Model:'https://schema.org/Number'. The solar radiation observed measured in Watts per square. Units:'w/m2'";
    rdf:type rdf:Property;
    rdfs:label "solarRadiation";
    rdfs:domain <https://smart-data-models.github.io/dataModel.Weather/WeatherObserved/schema.json>;
    rdfs:range xsd:decimal.
sdm:pressureTendency dcterms:description "Property. Enum:'falling, raising, steady'. Is the pressure rising or falling? It can be expressed in quantitative terms or qualitative terms.";
    rdf:type rdf:Property;
    rdfs:label "pressureTendency";
    rdfs:domain <https://smart-data-models.github.io/dataModel.Weather/WeatherObserved/schema.json>.
sdm:dewPoint dcterms:description "Property. Model:'https://schema.org/Number'. Units:'Celsius degrees'. The dew point encoded as a number. Observed temperature to which air must be cooled to become saturated with water vapor";
    rdf:type rdf:Property;
    rdfs:label "dewPoint";
    rdfs:domain <https://smart-data-models.github.io/dataModel.Weather/WeatherObserved/schema.json>;
    rdfs:range xsd:decimal.
sdm:refDevice dcterms:description "Relationship. Model:'https://schema.org/URL'. A reference to the device(s) which captured this observation.";
    rdf:type rdf:Property;
    rdfs:label "refDevice";
    rdfs:domain <https://smart-data-models.github.io/dataModel.Weather/WeatherObserved/schema.json>.
sdm:streamGauge dcterms:description "Property. Model:'https://schema.org/Number'. The water level surface elevation observed by Hydrometric measurement sensors, namely a [Stream Gauge](https://en.wikipedia.org/wiki/Stream_gauge) expressed in centimeters. Units:'centimeters'";
    rdf:type rdf:Property;
    rdfs:label "streamGauge";
    rdfs:domain <https://smart-data-models.github.io/dataModel.Weather/WeatherObserved/schema.json>;
    rdfs:range xsd:decimal.
sdm:snowHeight dcterms:description "Property. Model:'https://schema.org/Number'. The snow height observed by generic snow depth measurement sensors, expressed in centimeters. Units:'centimeters'";
    rdf:type rdf:Property;
    rdfs:label "snowHeight";
    rdfs:domain <https://smart-data-models.github.io/dataModel.Weather/WeatherObserved/schema.json>;
    rdfs:range xsd:decimal.
sdm:uVIndexMax dcterms:description "Property. Model:'https://schema.org/Number'. The maximum UV index for the period, based on the World Health Organization's UV Index measure. [http://www.who.int/uv/intersunprogramme/activities/uv_index/en/](http://www.who.int/uv/intersunprogramme/activities/uv_index/en/) the values between 1 and 11 are the valid range for the index. The value 0 is for describing that no signal is detected so no value is stored.";
    rdf:type rdf:Property;
    rdfs:label "uVIndexMax";
    rdfs:domain <https://smart-data-models.github.io/dataModel.Weather/WeatherObserved/schema.json>;
    rdfs:range xsd:decimal.
sdm:aqiMajorPollutant dcterms:description "Property. Model:'https://schema.org/Text'. Major pollutant in the Air Quality Index (AQI).";
    rdf:type rdf:Property;
    rdfs:label "aqiMajorPollutant";
    rdfs:domain <https://smart-data-models.github.io/dataModel.Weather/WeatherObserved/schema.json>;
    rdfs:range xsd:string.
sdm:aqiMajorPollutantForecast dcterms:description "Property. Model:'https://schema.org/Text'. Forecasted major air pollutant in the Air Quality Index (AQI) over a certain duration in future.";
    rdf:type rdf:Property;
    rdfs:label "aqiMajorPollutantForecast";
    rdfs:domain <https://smart-data-models.github.io/dataModel.Weather/WeatherObserved/schema.json>;
    rdfs:range xsd:string.
sdm:airTemperatureForecast dcterms:description "Property. Model:'https://schema.org/Number'. Forecasted value of air temperature over a certain duration in future.";
    rdf:type rdf:Property;
    rdfs:label "airTemperatureForecast";
    rdfs:domain <https://smart-data-models.github.io/dataModel.Weather/WeatherObserved/schema.json>;
    rdfs:range xsd:decimal.
sdm:precipitationForecast dcterms:description "Property. Model:'https://schema.org/Number'. Forecasted rainfall over a certain duration in future.";
    rdf:type rdf:Property;
    rdfs:label "precipitationForecast";
    rdfs:domain <https://smart-data-models.github.io/dataModel.Weather/WeatherObserved/schema.json>;
    rdfs:range xsd:decimal.
sdm:airQualityIndex dcterms:description "Property. Model:'https://schema.org/Number'. Air quality index is a number used to report the quality of the air on any given day.";
    rdf:type rdf:Property;
    rdfs:label "airQualityIndex";
    rdfs:domain <https://smart-data-models.github.io/dataModel.Weather/WeatherObserved/schema.json>;
    rdfs:range xsd:decimal.
sdm:relativeHumidityForecast dcterms:description "Property. Model:'https://schema.org/Number'. Forecasted relative humidity (water vapour in air) over a certain duration in future";
    rdf:type rdf:Property;
    rdfs:label "relativeHumidityForecast";
    rdfs:domain <https://smart-data-models.github.io/dataModel.Weather/WeatherObserved/schema.json>;
    rdfs:range xsd:decimal.
sdm:illuminance dcterms:description "Property. Observed instantaneous ambient light intensity. Units:'Lux'";
    rdf:type rdf:Property;
    rdfs:label "illuminance";
    rdfs:domain <https://smart-data-models.github.io/dataModel.Weather/WeatherObserved/schema.json>;
    rdfs:range xsd:decimal.
sdm:airQualityIndexForecast dcterms:description "Property. Model:'https://schema.org/Number'. Forecasted overall Air Quality Index (AQI) over a certain duration in future.";
    rdf:type rdf:Property;
    rdfs:label "airQualityIndexForecast";
    rdfs:domain <https://smart-data-models.github.io/dataModel.Weather/WeatherObserved/schema.json>;
    rdfs:range xsd:decimal.
sdm:airTemperatureTSA dcterms:description "Property. Air temperature time series aggregation";
    rdf:type rdf:Property;
    rdfs:label "airTemperatureTSA";
    rdfs:domain <https://smart-data-models.github.io/dataModel.Weather/WeatherObserved/schema.json>;
    rdfs:range sdm:AirTemperatureTSA.
sdm:AirTemperatureTSA rdf:type rdfs:Class;
    rdfs:label "AirTemperatureTSA".
