@prefix schema: <https://schema.org/>.
@prefix skos: <http://www.w3.org/2004/02/skos/core#>.
@prefix rdf: <http://www.w3.org/1999/02/22-rdf-syntax-ns#>.
@prefix rdfs: <http://www.w3.org/2000/01/rdf-schema#>.
@prefix foaf: <http://xmlns.com/foaf/0.1/>.
@prefix xsd: <http://www.w3.org/2001/XMLSchema#>.
@prefix dcterms: <http://purl.org/dc/terms/>.
@prefix owl: <http://www.w3.org/2002/07/owl#>.
@prefix jsonsc: <https://www.w3.org/2019/wot/json-schema#>.
@prefix jsonsc-ld: <http://w3id.org/jsonsc-ld/>.
@prefix api: <http://purl.org/linked-data/api/vocab>.
@prefix geo: <http://www.w3.org/2003/01/geo/wgs84_pos#>.
@prefix mobivoc: <http://schema.mobivoc.org/#>.
@prefix geosparql: <http://www.opengis.net/ont/geosparql#>.
@prefix sdm: <https://w3id.org/sdm#>.

<https://smart-data-models.github.io/data-models/Environment/WaterObserved/schema.js> dcterms:title "Water Observed schema";
    dcterms:description " Water observation data model is intended to represent the parameters of flow, level and volume of water observed, as well as the swell information, over a fixed or variable area. This observation also includes the masses of floating objects on this area. The data collected is provided by Sensors, Cameras,Water stations positioned at specific or sensitive locations for rivers, streams, torrent, lakes, seas, etc.".
sdm:type dcterms:description "Property. NGSI Entity type. It has to be WaterObserved";
    rdf:type rdf:Property;
    rdfs:label "type";
    rdfs:domain <https://smart-data-models.github.io/data-models/Environment/WaterObserved/schema.js>.
sdm:Type rdf:type skos:ConceptScheme.
sdm:type rdfs:range [
  owl:oneOf (sdm:WaterObserved)
].
sdm:WaterObserved rdf:type skos:Concept;
    skos:inScheme sdm:Type;
    rdfs:label "WaterObserved".
sdm:refDevice dcterms:description "Relationship. A reference to a point of interest associated to this observation.";
    rdf:type rdf:Property;
    rdfs:label "refDevice";
    rdfs:domain <https://smart-data-models.github.io/data-models/Environment/WaterObserved/schema.js>.
sdm:dateObserved dcterms:description "Property. Model:'https://schema.org/DateTime'. Date and time of this observation represented by an ISO8601 UTC format.";
    rdf:type rdf:Property;
    rdfs:label "dateObserved";
    rdfs:domain <https://smart-data-models.github.io/data-models/Environment/WaterObserved/schema.js>;
    rdfs:range xsd:dateTime.
sdm:dateObservedFrom dcterms:description "Property. Model:'https://schema.org/DateTime'. Observation period : Start date and time in an ISO8601 UTC format.";
    rdf:type rdf:Property;
    rdfs:label "dateObservedFrom";
    rdfs:domain <https://smart-data-models.github.io/data-models/Environment/WaterObserved/schema.js>;
    rdfs:range xsd:dateTime.
sdm:dateObservedTo dcterms:description "Property. Model:'https://schema.org/DateTime'. Observation period : End date and time in an ISO8601 UTC format.";
    rdf:type rdf:Property;
    rdfs:label "dateObservedTo";
    rdfs:domain <https://smart-data-models.github.io/data-models/Environment/WaterObserved/schema.js>;
    rdfs:range xsd:dateTime.
sdm:flow dcterms:description "Property. Model:'https://schema.org/Number'. Water Flow observed. The unit code (text) of measurement given using the UN/CEFACAT";
    rdf:type rdf:Property;
    rdfs:label "flow";
    rdfs:domain <https://smart-data-models.github.io/data-models/Environment/WaterObserved/schema.js>;
    rdfs:range xsd:decimal.
sdm:height dcterms:description "Property. Model:'https://schema.org/height'. Water height - Level reach on alert coasts.";
    rdf:type rdf:Property;
    rdfs:label "height";
    rdfs:domain <https://smart-data-models.github.io/data-models/Environment/WaterObserved/schema.js>;
    rdfs:range xsd:decimal.
sdm:swellHeight dcterms:description "Property. Model:'https://schema.org/height'. Swell height observed.";
    rdf:type rdf:Property;
    rdfs:label "swellHeight";
    rdfs:domain <https://smart-data-models.github.io/data-models/Environment/WaterObserved/schema.js>;
    rdfs:range xsd:decimal.
sdm:swellPeriod dcterms:description "Property. Model:'https://schema.org/Number'. Swells period observed.";
    rdf:type rdf:Property;
    rdfs:label "swellPeriod";
    rdfs:domain <https://smart-data-models.github.io/data-models/Environment/WaterObserved/schema.js>;
    rdfs:range xsd:decimal.
sdm:swellDirection dcterms:description "Property. Model:'https://schema.org/Number'. Swells Direction observed.";
    rdf:type rdf:Property;
    rdfs:label "swellDirection";
    rdfs:domain <https://smart-data-models.github.io/data-models/Environment/WaterObserved/schema.js>;
    rdfs:range xsd:decimal.
sdm:waveLength dcterms:description "Property. Model:'https://schema.org/Number'. Wave Length observed. ";
    rdf:type rdf:Property;
    rdfs:label "waveLength";
    rdfs:domain <https://smart-data-models.github.io/data-models/Environment/WaterObserved/schema.js>;
    rdfs:range xsd:decimal.
sdm:measuredArea dcterms:description "Property. Model:'https://schema.org/Number'. Reference of the surface measured. Units:'square meters'. The unit code (text) of measurement given using the [UN/CEFACT Common Codes](http://wiki.goodrelations-vocabulary.org/Documentation/UN/CEFACT_Common_Codes) (max. 3 characters). For instance, <code>MTK</code> represents MÂ².";
    rdf:type rdf:Property;
    rdfs:label "measuredArea";
    rdfs:domain <https://smart-data-models.github.io/data-models/Environment/WaterObserved/schema.js>;
    rdfs:range xsd:decimal.
sdm:objectArea dcterms:description "Property. Model:'https://schema.org/Number'. Percentage occupied by floating object in the area. The unit code (text) of measurement given using the [UN/CEFACT Common Codes](http://wiki.goodrelations-vocabulary.org/Documentation/UN/CEFACT_Common_Codes) (max. 3 characters). For instance, <code>P1</code> represents Percentage.";
    rdf:type rdf:Property;
    rdfs:label "objectArea";
    rdfs:domain <https://smart-data-models.github.io/data-models/Environment/WaterObserved/schema.js>;
    rdfs:range xsd:decimal.
sdm:objectHeightAverage dcterms:description "Property. Model:'https://schema.org/Number'. Average height raised. Units:'meters'. The unit code (text) of measurement given using the [UN/CEFACT Common Codes](http://wiki.goodrelations-vocabulary.org/Documentation/UN/CEFACT_Common_Codes) (max. 3 characters). For instance, <code>MTR</code> represents Meter.";
    rdf:type rdf:Property;
    rdfs:label "objectHeightAverage";
    rdfs:domain <https://smart-data-models.github.io/data-models/Environment/WaterObserved/schema.js>;
    rdfs:range xsd:decimal.
sdm:objectHeightMax dcterms:description "Property. Model:'https://schema.org/Number'. Maximum height raised. Units:'meters'. The unit code (text) of measurement given using the [UN/CEFACT Common Codes](http://wiki.goodrelations-vocabulary.org/Documentation/UN/CEFACT_Common_Codes) (max. 3 characters). For instance, <code>MTR</code> represents Meter.";
    rdf:type rdf:Property;
    rdfs:label "objectHeightMax";
    rdfs:domain <https://smart-data-models.github.io/data-models/Environment/WaterObserved/schema.js>;
    rdfs:range xsd:decimal.
sdm:objectVolume dcterms:description "Property. Model:'https://schema.org/Number'. Estimated volume raised. The unit code (text) of measurement given using the [UN/CEFACT Common Codes](http://wiki.goodrelations-vocabulary.org/Documentation/UN/CEFACT_Common_Codes) (max. 3 characters). For instance, <code>MTQ</code> represents Cubic Meters. Units:'cubic meters'";
    rdf:type rdf:Property;
    rdfs:label "objectVolume";
    rdfs:domain <https://smart-data-models.github.io/data-models/Environment/WaterObserved/schema.js>;
    rdfs:range xsd:decimal.
sdm:waterLevel dcterms:description "Property. Model:'https://schema.org/Number'. Current water level corresponding to this observation. Units:'metre'. The unit code (text) of measurement given using the [UN/CEFACT Common Codes](http://wiki.goodrelations-vocabulary.org/Documentation/UN/CEFACT_Common_Codes) (max. 3 characters). For instance, <code>MTR</code> represents Metre.";
    rdf:type rdf:Property;
    rdfs:label "waterLevel";
    rdfs:domain <https://smart-data-models.github.io/data-models/Environment/WaterObserved/schema.js>;
    rdfs:range xsd:decimal.
sdm:waterDischarge dcterms:description "Property. Model:'https://schema.org/Number'. Discharge into the water from stormwater and wastewater treatment plants. Units:'cubic metre'. The unit code (text) of measurement given using the [UN/CEFACT Common Codes](http://wiki.goodrelations-vocabulary.org/Documentation/UN/CEFACT_Common_Codes) (max. 3 characters). For instance, <code>MTQ</code> represents Cubic Metre.";
    rdf:type rdf:Property;
    rdfs:label "waterDischarge";
    rdfs:domain <https://smart-data-models.github.io/data-models/Environment/WaterObserved/schema.js>;
    rdfs:range xsd:decimal.
