@prefix schema: <https://schema.org/>.
@prefix skos: <http://www.w3.org/2004/02/skos/core#>.
@prefix rdf: <http://www.w3.org/1999/02/22-rdf-syntax-ns#>.
@prefix rdfs: <http://www.w3.org/2000/01/rdf-schema#>.
@prefix foaf: <http://xmlns.com/foaf/0.1/>.
@prefix xsd: <http://www.w3.org/2001/XMLSchema#>.
@prefix dcterms: <http://purl.org/dc/terms/>.
@prefix owl: <http://www.w3.org/2002/07/owl#>.
@prefix jsonsc: <https://www.w3.org/2019/wot/json-schema#>.
@prefix jsonsc-ld: <http://w3id.org/jsonsc-ld/>.
@prefix api: <http://purl.org/linked-data/api/vocab>.
@prefix geo: <http://www.w3.org/2003/01/geo/wgs84_pos#>.
@prefix mobivoc: <http://schema.mobivoc.org/#>.
@prefix geosparql: <http://www.opengis.net/ont/geosparql#>.
@prefix sdm: <https://w3id.org/sdm#>.

<https://github.com/smart-data-models/dataModel.OSLO/raw/master/BicycleParkingStationForecast/schema.json> dcterms:title "Bicycle Parking Station PTH-AP schema";
    dcterms:description "Bicycle Parking Station Schema meeting Passenger Transport Hubs AP Schema specification".
sdm:type dcterms:description "Property. NGSI Entity type. It has to be BicycleParkingStation";
    rdf:type rdf:Property;
    rdfs:label "type";
    rdfs:domain <https://github.com/smart-data-models/dataModel.OSLO/raw/master/BicycleParkingStationForecast/schema.json>.
sdm:Type rdf:type skos:ConceptScheme.
sdm:type rdfs:range [
  owl:oneOf (sdm:BicycleParkingStationForecast)
].
sdm:BicycleParkingStationForecast rdf:type skos:Concept;
    skos:inScheme sdm:Type;
    rdfs:label "BicycleParkingStationForecast".
sdm:ParkingFacility.capacity dcterms:description "Property. Capacity of a civic structure. Model:'http://schema.mobivoc.org/#capacity'. ";
    rdf:type rdf:Property;
    rdfs:label "ParkingFacility.capacity";
    rdfs:domain <https://github.com/smart-data-models/dataModel.OSLO/raw/master/BicycleParkingStationForecast/schema.json>;
    rdfs:range sdm:ParkingFacility.capacity;
    rdf:type rdfs:Class;
    rdfs:label "ParkingFacility.capacity".
sdm:type rdf:type rdf:Property;
    rdfs:label "type";
    rdfs:domain sdm:ParkingFacility.capacity.
sdm:Type rdf:type skos:ConceptScheme.
sdm:type rdfs:range [
  owl:oneOf (sdm:Capacity)
].
sdm:Capacity rdf:type skos:Concept;
    skos:inScheme sdm:Type;
    rdfs:label "Capacity".
sdm:Capacity.total dcterms:description "Property. Model: 'http://schema.mobivoc.org/#totalCapacity'. Indicates the capacity of a resource.";
    rdf:type rdf:Property;
    rdfs:label "Capacity.total";
    rdfs:domain sdm:ParkingFacility.capacity;
    rdfs:range xsd:decimal.
sdm:InfrastructureElement.geometry dcterms:description "Property. Model:'http://www.w3.org/ns/locn#geometry'. The geometry corresponding to the infrastructure element.";
    rdf:type rdf:Property;
    rdfs:label "InfrastructureElement.geometry";
    rdfs:domain <https://github.com/smart-data-models/dataModel.OSLO/raw/master/BicycleParkingStationForecast/schema.json>;
    rdfs:range sdm:InfrastructureElement.geometry;
    rdf:type rdfs:Class;
    rdfs:label "InfrastructureElement.geometry".
sdm:type dcterms:description "Property. Model: 'http://www.w3.org/ns/locn#Geometry'";
    rdf:type rdf:Property;
    rdfs:label "type";
    rdfs:domain sdm:InfrastructureElement.geometry.
sdm:Type rdf:type skos:ConceptScheme.
sdm:type rdfs:range [
  owl:oneOf (sdm:Geometry)
].
sdm:Geometry rdf:type skos:Concept;
    skos:inScheme sdm:Type;
    rdfs:label "Geometry".
sdm:Geometry.wkt dcterms:description "Property. Model:'http://www.opengis.net/ont/geosparql#asWKT'. Geometry expressed in wkt format.";
    rdf:type rdf:Property;
    rdfs:label "Geometry.wkt";
    rdfs:domain sdm:InfrastructureElement.geometry;
    rdfs:range xsd:string.
sdm:validity dcterms:description "Property. Model:'https://schema.org/Text'. Includes the validity period for this forecast as a ISO8601 time interval. It can be also used two separate attributes: `validFrom`, `validTo`.";
    rdf:type rdf:Property;
    rdfs:label "validity";
    rdfs:domain <https://github.com/smart-data-models/dataModel.OSLO/raw/master/BicycleParkingStationForecast/schema.json>;
    rdfs:range xsd:string.
sdm:validFrom dcterms:description "Property. Model:'https://schema.org/DateTime'. Validity period start date and time.";
    rdf:type rdf:Property;
    rdfs:label "validFrom";
    rdfs:domain <https://github.com/smart-data-models/dataModel.OSLO/raw/master/BicycleParkingStationForecast/schema.json>;
    rdfs:range xsd:dateTime.
sdm:validTo dcterms:description "Property. Model:'https://schema.org/DateTime'. Validity period end date and time.";
    rdf:type rdf:Property;
    rdfs:label "validTo";
    rdfs:domain <https://github.com/smart-data-models/dataModel.OSLO/raw/master/BicycleParkingStationForecast/schema.json>;
    rdfs:range xsd:dateTime.
