@prefix schema: <https://schema.org/>.
@prefix skos: <http://www.w3.org/2004/02/skos/core#>.
@prefix rdf: <http://www.w3.org/1999/02/22-rdf-syntax-ns#>.
@prefix rdfs: <http://www.w3.org/2000/01/rdf-schema#>.
@prefix foaf: <http://xmlns.com/foaf/0.1/>.
@prefix xsd: <http://www.w3.org/2001/XMLSchema#>.
@prefix dcterms: <http://purl.org/dc/terms/>.
@prefix owl: <http://www.w3.org/2002/07/owl#>.
@prefix jsonsc: <https://www.w3.org/2019/wot/json-schema#>.
@prefix jsonsc-ld: <http://w3id.org/jsonsc-ld/>.
@prefix api: <http://purl.org/linked-data/api/vocab>.
@prefix geo: <http://www.w3.org/2003/01/geo/wgs84_pos#>.
@prefix mobivoc: <http://schema.mobivoc.org/#>.
@prefix geosparql: <http://www.opengis.net/ont/geosparql#>.
@prefix sdm: <https://w3id.org/sdm#>.

<https://smart-data-models.github.io/dataModel.Agrifood/AnimalMovement/schema.json> dcterms:title "Animal Movement";
    dcterms:description "Object modelling of an animal movement for a livestock farm.".
sdm:type dcterms:description "Property. NGSI entity type. It has to be AnimalMovement";
    rdf:type rdf:Property;
    rdfs:label "type";
    rdfs:domain <https://smart-data-models.github.io/dataModel.Agrifood/AnimalMovement/schema.json>.
sdm:Type rdf:type skos:ConceptScheme.
sdm:type rdfs:range [
  owl:oneOf (sdm:AnimalMovement)
].
sdm:AnimalMovement rdf:type skos:Concept;
    skos:inScheme sdm:Type;
    rdfs:label "AnimalMovement".
sdm:date dcterms:description "Property. Date of animal movement.";
    rdf:type rdf:Property;
    rdfs:label "date";
    rdfs:domain <https://smart-data-models.github.io/dataModel.Agrifood/AnimalMovement/schema.json>;
    rdfs:range xsd:dateTime.
sdm:animal rdf:type rdf:Property;
    rdfs:label "animal";
    rdfs:domain <https://smart-data-models.github.io/dataModel.Agrifood/AnimalMovement/schema.json>;
    rdfs:range xsd:anyURI.
sdm:movement dcterms:description "Property. Type of movement: input/output. Input means that animals enter the farm/enclosure, while output means that they leave.";
    rdf:type rdf:Property;
    rdfs:label "movement";
    rdfs:domain <https://smart-data-models.github.io/dataModel.Agrifood/AnimalMovement/schema.json>;
    rdfs:range xsd:string.
sdm:farm dcterms:description "Relationship. Farm object of the movement. Model:'https://github.com/smart-data-models/dataModel.Agrifood/blob/master/AgriFarm/schema.json'";
    rdf:type rdf:Property;
    rdfs:label "farm";
    rdfs:domain <https://smart-data-models.github.io/dataModel.Agrifood/AnimalMovement/schema.json>;
    rdfs:range xsd:anyURI.
sdm:parcel dcterms:description "Relationship. Parcel object of the movement. Model:'https://github.com/smart-data-models/dataModel.Agrifood/blob/master/AgriParcel/schema.json'";
    rdf:type rdf:Property;
    rdfs:label "parcel";
    rdfs:domain <https://smart-data-models.github.io/dataModel.Agrifood/AnimalMovement/schema.json>;
    rdfs:range xsd:anyURI.
sdm:pen dcterms:description "Relationship. Pen object of the movement. Model:'https://github.com/smart-data-models/dataModel.Agrifood/blob/master/Pen/schema.json'";
    rdf:type rdf:Property;
    rdfs:label "pen";
    rdfs:domain <https://smart-data-models.github.io/dataModel.Agrifood/AnimalMovement/schema.json>;
    rdfs:range xsd:anyURI.
