@prefix schema: <https://schema.org/>.
@prefix skos: <http://www.w3.org/2004/02/skos/core#>.
@prefix rdf: <http://www.w3.org/1999/02/22-rdf-syntax-ns#>.
@prefix rdfs: <http://www.w3.org/2000/01/rdf-schema#>.
@prefix foaf: <http://xmlns.com/foaf/0.1/>.
@prefix xsd: <http://www.w3.org/2001/XMLSchema#>.
@prefix dcterms: <http://purl.org/dc/terms/>.
@prefix owl: <http://www.w3.org/2002/07/owl#>.
@prefix jsonsc: <https://www.w3.org/2019/wot/json-schema#>.
@prefix jsonsc-ld: <http://w3id.org/jsonsc-ld/>.
@prefix api: <http://purl.org/linked-data/api/vocab>.
@prefix geo: <http://www.w3.org/2003/01/geo/wgs84_pos#>.
@prefix mobivoc: <http://schema.mobivoc.org/#>.
@prefix geosparql: <http://www.opengis.net/ont/geosparql#>.
@prefix sdm: <https://w3id.org/sdm#>.

<https://smart-data-models.github.io/dataModels.CIMEnergyClasses/ExcSEXS/schema.json> dcterms:title " Smart Data Models - ExcSEXS";
    dcterms:description "Adapted from CIM data models. Simplified Excitation System Model.".
sdm:type dcterms:description "Property. NGSI type. It has to be ExcSEXS";
    rdf:type rdf:Property;
    rdfs:label "type";
    rdfs:domain <https://smart-data-models.github.io/dataModels.CIMEnergyClasses/ExcSEXS/schema.json>.
sdm:Type rdf:type skos:ConceptScheme.
sdm:type rdfs:range [
  owl:oneOf (sdm:ExcSEXS)
].
sdm:ExcSEXS rdf:type skos:Concept;
    skos:inScheme sdm:Type;
    rdfs:label "ExcSEXS".
sdm:efdmax dcterms:description "Property. Model:'https://schema.org/Number'. Field voltage clipping maximum limit (Efdmax).  Typical Value = 5. Default: 0.0";
    rdf:type rdf:Property;
    rdfs:label "efdmax";
    rdfs:domain <https://smart-data-models.github.io/dataModels.CIMEnergyClasses/ExcSEXS/schema.json>;
    rdfs:range xsd:decimal.
sdm:efdmin dcterms:description "Property. Model:'https://schema.org/Number'. Field voltage clipping minimum limit (Efdmin).  Typical Value = -5. Default: 0.0";
    rdf:type rdf:Property;
    rdfs:label "efdmin";
    rdfs:domain <https://smart-data-models.github.io/dataModels.CIMEnergyClasses/ExcSEXS/schema.json>;
    rdfs:range xsd:decimal.
sdm:emax dcterms:description "Property. Model:'https://schema.org/Number'. Maximum field voltage output (Emax).  Typical Value = 5. Default: 0.0";
    rdf:type rdf:Property;
    rdfs:label "emax";
    rdfs:domain <https://smart-data-models.github.io/dataModels.CIMEnergyClasses/ExcSEXS/schema.json>;
    rdfs:range xsd:decimal.
sdm:emin dcterms:description "Property. Model:'https://schema.org/Number'. Minimum field voltage output (Emin).  Typical Value = -5. Default: 0.0";
    rdf:type rdf:Property;
    rdfs:label "emin";
    rdfs:domain <https://smart-data-models.github.io/dataModels.CIMEnergyClasses/ExcSEXS/schema.json>;
    rdfs:range xsd:decimal.
sdm:k dcterms:description "Property. Model:'https://schema.org/Number'. Gain (K) (>0).  Typical Value = 100. Default: 0.0";
    rdf:type rdf:Property;
    rdfs:label "k";
    rdfs:domain <https://smart-data-models.github.io/dataModels.CIMEnergyClasses/ExcSEXS/schema.json>;
    rdfs:range xsd:decimal.
sdm:kc dcterms:description "Property. Model:'https://schema.org/Number'. PI controller gain (Kc).  Typical Value = 0.08. Default: 0.0";
    rdf:type rdf:Property;
    rdfs:label "kc";
    rdfs:domain <https://smart-data-models.github.io/dataModels.CIMEnergyClasses/ExcSEXS/schema.json>;
    rdfs:range xsd:decimal.
sdm:tatb dcterms:description "Property. Model:'https://schema.org/Number'. Ta/Tb - gain reduction ratio of lag-lead element (TaTb).  Typical Value = 0.1. Default: 0.0";
    rdf:type rdf:Property;
    rdfs:label "tatb";
    rdfs:domain <https://smart-data-models.github.io/dataModels.CIMEnergyClasses/ExcSEXS/schema.json>;
    rdfs:range xsd:decimal.
sdm:tb dcterms:description "Property. Model:'https://schema.org/Number'. Denominator time constant of lag-lead block (Tb).  Typical Value = 10. Default: 0";
    rdf:type rdf:Property;
    rdfs:label "tb";
    rdfs:domain <https://smart-data-models.github.io/dataModels.CIMEnergyClasses/ExcSEXS/schema.json>;
    rdfs:range xsd:decimal.
sdm:tc dcterms:description "Property. Model:'https://schema.org/Number'. PI controller phase lead time constant (Tc).  Typical Value = 0. Default: 0";
    rdf:type rdf:Property;
    rdfs:label "tc";
    rdfs:domain <https://smart-data-models.github.io/dataModels.CIMEnergyClasses/ExcSEXS/schema.json>;
    rdfs:range xsd:decimal.
sdm:te dcterms:description "Property. Model:'https://schema.org/Number'. Time constant of gain block (Te).  Typical Value = 0.05. Default: 0";
    rdf:type rdf:Property;
    rdfs:label "te";
    rdfs:domain <https://smart-data-models.github.io/dataModels.CIMEnergyClasses/ExcSEXS/schema.json>;
    rdfs:range xsd:decimal.
