@prefix schema: <https://schema.org/>.
@prefix skos: <http://www.w3.org/2004/02/skos/core#>.
@prefix rdf: <http://www.w3.org/1999/02/22-rdf-syntax-ns#>.
@prefix rdfs: <http://www.w3.org/2000/01/rdf-schema#>.
@prefix foaf: <http://xmlns.com/foaf/0.1/>.
@prefix xsd: <http://www.w3.org/2001/XMLSchema#>.
@prefix dcterms: <http://purl.org/dc/terms/>.
@prefix owl: <http://www.w3.org/2002/07/owl#>.
@prefix jsonsc: <https://www.w3.org/2019/wot/json-schema#>.
@prefix jsonsc-ld: <http://w3id.org/jsonsc-ld/>.
@prefix api: <http://purl.org/linked-data/api/vocab>.
@prefix geo: <http://www.w3.org/2003/01/geo/wgs84_pos#>.
@prefix mobivoc: <http://schema.mobivoc.org/#>.
@prefix geosparql: <http://www.opengis.net/ont/geosparql#>.
@prefix sdm: <https://w3id.org/sdm#>.

<https://smart-data-models.github.io/dataModel.Environment/TrafficEnvironmentImpactForecast/schema.json> dcterms:title "Smart Data Models - Traffic Environment Impact Forecast";
    dcterms:description "Environmental Impact of traffic based on the vehicles traffic expectations and their emission characteristics".
sdm:type dcterms:description "Property. NGSI type. It has to be TrafficEnvironmentImpactForecast";
    rdf:type rdf:Property;
    rdfs:label "type";
    rdfs:domain <https://smart-data-models.github.io/dataModel.Environment/TrafficEnvironmentImpactForecast/schema.json>.
sdm:Type rdf:type skos:ConceptScheme.
sdm:type rdfs:range [
  owl:oneOf (sdm:TrafficEnvironmentImpact)
].
sdm:TrafficEnvironmentImpact rdf:type skos:Concept;
    skos:inScheme sdm:Type;
    rdfs:label "TrafficEnvironmentImpact".
sdm:co2 dcterms:description "Property. The expected C02 emission concentration. Units:'mg/L'";
    rdf:type rdf:Property;
    rdfs:label "co2";
    rdfs:domain <https://smart-data-models.github.io/dataModel.Environment/TrafficEnvironmentImpactForecast/schema.json>;
    rdfs:range xsd:decimal.
sdm:validFrom dcterms:description "Property. The start of the validity period for this forecast as a ISO8601 format";
    rdf:type rdf:Property;
    rdfs:label "validFrom";
    rdfs:domain <https://smart-data-models.github.io/dataModel.Environment/TrafficEnvironmentImpactForecast/schema.json>;
    rdfs:range xsd:dateTime.
sdm:validTo dcterms:description "Property. The end of the validity period for this forecast as a ISO8601 format";
    rdf:type rdf:Property;
    rdfs:label "validTo";
    rdfs:domain <https://smart-data-models.github.io/dataModel.Environment/TrafficEnvironmentImpactForecast/schema.json>;
    rdfs:range xsd:dateTime.
sdm:validity dcterms:description "Property. Model:'https://schema.org/Text'. Includes the validity period for this forecast as a ISO8601 time interval.";
    rdf:type rdf:Property;
    rdfs:label "validity";
    rdfs:domain <https://smart-data-models.github.io/dataModel.Environment/TrafficEnvironmentImpactForecast/schema.json>;
    rdfs:range xsd:string.
sdm:dateIssued dcterms:description "Property. The date and time the forecast was issued by the service provider in ISO8601 UTC format.";
    rdf:type rdf:Property;
    rdfs:label "dateIssued";
    rdfs:domain <https://smart-data-models.github.io/dataModel.Environment/TrafficEnvironmentImpactForecast/schema.json>;
    rdfs:range xsd:dateTime.
sdm:traffic dcterms:description "Property. Array of objects containing the expected values for intensity, occupation an speed of the different vehicle types";
    rdf:type rdf:Property;
    rdfs:label "traffic";
    rdfs:domain <https://smart-data-models.github.io/dataModel.Environment/TrafficEnvironmentImpactForecast/schema.json>;
    rdfs:range sdm:Traffic.
sdm:Traffic rdf:type rdfs:Class;
    rdfs:label "Traffic".
sdm:vehicleClass dcterms:description "Property. Enumeration of the vehicle classes";
    rdf:type rdf:Property;
    rdfs:label "vehicleClass";
    rdfs:domain sdm:Traffic;
    rdfs:range xsd:string.
sdm:intensityExpected dcterms:description "Property. Total number of vehicles expected during this forecast period. Model:'https://schema.org/Number'.";
    rdf:type rdf:Property;
    rdfs:label "intensityExpected";
    rdfs:domain sdm:Traffic;
    rdfs:range xsd:decimal.
sdm:occupancyExpected dcterms:description "Property. Fraction of the observation time where a vehicle has been occupying the observed lane. Model:'https://schema.org/Number'.";
    rdf:type rdf:Property;
    rdfs:label "occupancyExpected";
    rdfs:domain sdm:Traffic;
    rdfs:range xsd:decimal.
sdm:averageVehicleSpeedExpected dcterms:description "Property. Average speed expected of the vehicles transiting during the observation period. Model:'https://schema.org/Number'. Units:'Kilometer per hour (Km/h)'";
    rdf:type rdf:Property;
    rdfs:label "averageVehicleSpeedExpected";
    rdfs:domain sdm:Traffic;
    rdfs:range xsd:decimal.
