@prefix schema: <https://schema.org/>.
@prefix skos: <http://www.w3.org/2004/02/skos/core#>.
@prefix rdf: <http://www.w3.org/1999/02/22-rdf-syntax-ns#>.
@prefix rdfs: <http://www.w3.org/2000/01/rdf-schema#>.
@prefix foaf: <http://xmlns.com/foaf/0.1/>.
@prefix xsd: <http://www.w3.org/2001/XMLSchema#>.
@prefix dcterms: <http://purl.org/dc/terms/>.
@prefix owl: <http://www.w3.org/2002/07/owl#>.
@prefix jsonsc: <https://www.w3.org/2019/wot/json-schema#>.
@prefix jsonsc-ld: <http://w3id.org/jsonsc-ld/>.
@prefix api: <http://purl.org/linked-data/api/vocab>.
@prefix geo: <http://www.w3.org/2003/01/geo/wgs84_pos#>.
@prefix mobivoc: <http://schema.mobivoc.org/#>.
@prefix geosparql: <http://www.opengis.net/ont/geosparql#>.
@prefix sdm: <https://w3id.org/sdm#>.

<https://smart-data-models.github.io/dataModel.UrbanMobility/GtfsFrequency/schema.json> dcterms:title "Smart Data Models. GTFS Schema - Frequency";
    dcterms:description "GTFS Frequency".
sdm:type dcterms:description "Property. NGSI Entity type. It has to be GtfsFrequency";
    rdf:type rdf:Property;
    rdfs:label "type";
    rdfs:domain <https://smart-data-models.github.io/dataModel.UrbanMobility/GtfsFrequency/schema.json>.
sdm:Type rdf:type skos:ConceptScheme.
sdm:type rdfs:range [
  owl:oneOf (sdm:GtfsFrequency)
].
sdm:GtfsFrequency rdf:type skos:Concept;
    skos:inScheme sdm:Type;
    rdfs:label "GtfsFrequency".
sdm:startTime dcterms:description "Property. Same as GTFS `start_time`. Model:'https://schema.org/Text'";
    rdf:type rdf:Property;
    rdfs:label "startTime";
    rdfs:domain <https://smart-data-models.github.io/dataModel.UrbanMobility/GtfsFrequency/schema.json>;
    rdfs:range xsd:string.
sdm:endTime dcterms:description "Property. Same as GTFS `end_time`. Model:'https://schema.org/Text'";
    rdf:type rdf:Property;
    rdfs:label "endTime";
    rdfs:domain <https://smart-data-models.github.io/dataModel.UrbanMobility/GtfsFrequency/schema.json>;
    rdfs:range xsd:string.
sdm:headwaySeconds dcterms:description "Property. Same as GTFS `headway_secs`. Model:'https://schema.org/Number'";
    rdf:type rdf:Property;
    rdfs:label "headwaySeconds";
    rdfs:domain <https://smart-data-models.github.io/dataModel.UrbanMobility/GtfsFrequency/schema.json>;
    rdfs:range xsd:integer.
sdm:exactTimes dcterms:description "Property. Same as GTFS `exact_times` but encoded as a Boolean; `false`: Frequency-based trips are not exactly scheduled. `true`: Frequency-based trips are exactly scheduled. Model:'https://schema.org/Boolean'";
    rdf:type rdf:Property;
    rdfs:label "exactTimes";
    rdfs:domain <https://smart-data-models.github.io/dataModel.UrbanMobility/GtfsFrequency/schema.json>;
    rdfs:range xsd:boolean.
