@prefix schema: <https://schema.org/>.
@prefix skos: <http://www.w3.org/2004/02/skos/core#>.
@prefix rdf: <http://www.w3.org/1999/02/22-rdf-syntax-ns#>.
@prefix rdfs: <http://www.w3.org/2000/01/rdf-schema#>.
@prefix foaf: <http://xmlns.com/foaf/0.1/>.
@prefix xsd: <http://www.w3.org/2001/XMLSchema#>.
@prefix dcterms: <http://purl.org/dc/terms/>.
@prefix owl: <http://www.w3.org/2002/07/owl#>.
@prefix jsonsc: <https://www.w3.org/2019/wot/json-schema#>.
@prefix jsonsc-ld: <http://w3id.org/jsonsc-ld/>.
@prefix api: <http://purl.org/linked-data/api/vocab>.
@prefix geo: <http://www.w3.org/2003/01/geo/wgs84_pos#>.
@prefix mobivoc: <http://schema.mobivoc.org/#>.
@prefix geosparql: <http://www.opengis.net/ont/geosparql#>.
@prefix sdm: <https://w3id.org/sdm#>.

<https://smart-data-models.github.io/dataModels.CIMEnergyClasses/PFVArType1IEEEVArController/schema.json> dcterms:title " Smart Data Models - PFVArType1IEEEVArController";
    dcterms:description "Adapted from CIM data models. The class represents IEEE VAR Controller Type 1 which operates by moving the voltage reference directly.  Reference: IEEE Standard 421.5-2005 Section 11.3.".
sdm:type dcterms:description "Property. NGSI type. It has to be PFVArType1IEEEVArController";
    rdf:type rdf:Property;
    rdfs:label "type";
    rdfs:domain <https://smart-data-models.github.io/dataModels.CIMEnergyClasses/PFVArType1IEEEVArController/schema.json>.
sdm:Type rdf:type skos:ConceptScheme.
sdm:type rdfs:range [
  owl:oneOf (sdm:PFVArType1IEEEVArController)
].
sdm:PFVArType1IEEEVArController rdf:type skos:Concept;
    skos:inScheme sdm:Type;
    rdfs:label "PFVArType1IEEEVArController".
sdm:tvarc dcterms:description "Property. Model:'https://schema.org/Number'. Var controller time delay ().  Typical Value = 5. Default: 0";
    rdf:type rdf:Property;
    rdfs:label "tvarc";
    rdfs:domain <https://smart-data-models.github.io/dataModels.CIMEnergyClasses/PFVArType1IEEEVArController/schema.json>;
    rdfs:range xsd:decimal.
sdm:vvar dcterms:description "Property. Model:'https://schema.org/Number'. Synchronous machine power factor (). Default: 0.0";
    rdf:type rdf:Property;
    rdfs:label "vvar";
    rdfs:domain <https://smart-data-models.github.io/dataModels.CIMEnergyClasses/PFVArType1IEEEVArController/schema.json>;
    rdfs:range xsd:decimal.
sdm:vvarcbw dcterms:description "Property. Model:'https://schema.org/Number'. Var controller dead band ().  Typical Value = 0.02. Default: 0.0";
    rdf:type rdf:Property;
    rdfs:label "vvarcbw";
    rdfs:domain <https://smart-data-models.github.io/dataModels.CIMEnergyClasses/PFVArType1IEEEVArController/schema.json>;
    rdfs:range xsd:decimal.
sdm:vvarref dcterms:description "Property. Model:'https://schema.org/Number'. Var controller reference (). Default: 0.0";
    rdf:type rdf:Property;
    rdfs:label "vvarref";
    rdfs:domain <https://smart-data-models.github.io/dataModels.CIMEnergyClasses/PFVArType1IEEEVArController/schema.json>;
    rdfs:range xsd:decimal.
sdm:vvtmax dcterms:description "Property. Model:'https://schema.org/Number'. Maximum machine terminal voltage needed for pf/var controller to be enabled (). Default: 0.0";
    rdf:type rdf:Property;
    rdfs:label "vvtmax";
    rdfs:domain <https://smart-data-models.github.io/dataModels.CIMEnergyClasses/PFVArType1IEEEVArController/schema.json>;
    rdfs:range xsd:decimal.
sdm:vvtmin dcterms:description "Property. Model:'https://schema.org/Number'. Minimum machine terminal voltage needed to enable pf/var controller (). Default: 0.0";
    rdf:type rdf:Property;
    rdfs:label "vvtmin";
    rdfs:domain <https://smart-data-models.github.io/dataModels.CIMEnergyClasses/PFVArType1IEEEVArController/schema.json>;
    rdfs:range xsd:decimal.
