@prefix schema: <https://schema.org/>.
@prefix skos: <http://www.w3.org/2004/02/skos/core#>.
@prefix rdf: <http://www.w3.org/1999/02/22-rdf-syntax-ns#>.
@prefix rdfs: <http://www.w3.org/2000/01/rdf-schema#>.
@prefix foaf: <http://xmlns.com/foaf/0.1/>.
@prefix xsd: <http://www.w3.org/2001/XMLSchema#>.
@prefix dcterms: <http://purl.org/dc/terms/>.
@prefix owl: <http://www.w3.org/2002/07/owl#>.
@prefix jsonsc: <https://www.w3.org/2019/wot/json-schema#>.
@prefix jsonsc-ld: <http://w3id.org/jsonsc-ld/>.
@prefix api: <http://purl.org/linked-data/api/vocab>.
@prefix geo: <http://www.w3.org/2003/01/geo/wgs84_pos#>.
@prefix mobivoc: <http://schema.mobivoc.org/#>.
@prefix geosparql: <http://www.opengis.net/ont/geosparql#>.
@prefix sdm: <https://w3id.org/sdm#>.

<https://smart-data-models.github.io/dataModels.CIMEnergyClasses/SvPowerFlow/schema.json> dcterms:title " Smart Data Models - SvPowerFlow";
    dcterms:description "Adapted from CIM data models. State variable for power flow. Load convention is used for flow direction. This means flow out from the TopologicalNode into the equipment is positive.".
sdm:type dcterms:description "Property. NGSI type. It has to be SvPowerFlow";
    rdf:type rdf:Property;
    rdfs:label "type";
    rdfs:domain <https://smart-data-models.github.io/dataModels.CIMEnergyClasses/SvPowerFlow/schema.json>.
sdm:Type rdf:type skos:ConceptScheme.
sdm:type rdfs:range [
  owl:oneOf (sdm:SvPowerFlow)
].
sdm:SvPowerFlow rdf:type skos:Concept;
    skos:inScheme sdm:Type;
    rdfs:label "SvPowerFlow".
sdm:Terminal dcterms:description "Property. Model:'https://schema.org/Number'. The terminal associated with the power flow state variable. Default: None";
    rdf:type rdf:Property;
    rdfs:label "Terminal";
    rdfs:domain <https://smart-data-models.github.io/dataModels.CIMEnergyClasses/SvPowerFlow/schema.json>;
    rdfs:range xsd:decimal.
sdm:p dcterms:description "Property. Model:'https://schema.org/Number'. The active power flow. Load sign convention is used, i.e. positive sign means flow out from a TopologicalNode (bus) into the conducting equipment. Default: 0.0";
    rdf:type rdf:Property;
    rdfs:label "p";
    rdfs:domain <https://smart-data-models.github.io/dataModels.CIMEnergyClasses/SvPowerFlow/schema.json>;
    rdfs:range xsd:decimal.
sdm:q dcterms:description "Property. Model:'https://schema.org/Number'. The reactive power flow. Load sign convention is used, i.e. positive sign means flow out from a TopologicalNode (bus) into the conducting equipment. Default: 0.0";
    rdf:type rdf:Property;
    rdfs:label "q";
    rdfs:domain <https://smart-data-models.github.io/dataModels.CIMEnergyClasses/SvPowerFlow/schema.json>;
    rdfs:range xsd:decimal.
