@prefix schema: <https://schema.org/>.
@prefix skos: <http://www.w3.org/2004/02/skos/core#>.
@prefix rdf: <http://www.w3.org/1999/02/22-rdf-syntax-ns#>.
@prefix rdfs: <http://www.w3.org/2000/01/rdf-schema#>.
@prefix foaf: <http://xmlns.com/foaf/0.1/>.
@prefix xsd: <http://www.w3.org/2001/XMLSchema#>.
@prefix dcterms: <http://purl.org/dc/terms/>.
@prefix owl: <http://www.w3.org/2002/07/owl#>.
@prefix jsonsc: <https://www.w3.org/2019/wot/json-schema#>.
@prefix jsonsc-ld: <http://w3id.org/jsonsc-ld/>.
@prefix api: <http://purl.org/linked-data/api/vocab>.
@prefix geo: <http://www.w3.org/2003/01/geo/wgs84_pos#>.
@prefix mobivoc: <http://schema.mobivoc.org/#>.
@prefix geosparql: <http://www.opengis.net/ont/geosparql#>.
@prefix sdm: <https://w3id.org/sdm#>.

<https://smart-data-models.github.io/dataModel.Weather/RainFallRadarObserved/schema.json> dcterms:title "Rain Fall Radar Observation schema";
    dcterms:description "The Data Model is intended to measure the water slides on a predefined area by a set of 4 Location represented by a Geo property format.".
sdm:type dcterms:description "Property. NGSI Entity type. It has to be RainFallRadarObserved";
    rdf:type rdf:Property;
    rdfs:label "type";
    rdfs:domain <https://smart-data-models.github.io/dataModel.Weather/RainFallRadarObserved/schema.json>.
sdm:Type rdf:type skos:ConceptScheme.
sdm:type rdfs:range [
  owl:oneOf (sdm:RainFallRadarObserved)
].
sdm:RainFallRadarObserved rdf:type skos:Concept;
    skos:inScheme sdm:Type;
    rdfs:label "RainFallRadarObserved".
sdm:refDevice dcterms:description "Relationship. Reference to a [Device](https://github.com/smart-data-models/dataModel.Device/blob/master/Device/doc/spec.md) which captured this observation. Model:'https://schema.org/URL'";
    rdf:type rdf:Property;
    rdfs:label "refDevice";
    rdfs:domain <https://smart-data-models.github.io/dataModel.Weather/RainFallRadarObserved/schema.json>.
sdm:refPointOfInterest dcterms:description "Relationship. Reference to a [PointOfInterest](https://github.com/smart-data-models/dataModel.PointOfInterest/blob/master/PointOfInterest/doc/spec.md) linked with the observation. Model:'https://schema.org/URL'";
    rdf:type rdf:Property;
    rdfs:label "refPointOfInterest";
    rdfs:domain <https://smart-data-models.github.io/dataModel.Weather/RainFallRadarObserved/schema.json>.
sdm:dateObserved dcterms:description "Property. The date and time of this observation in ISO8601 UTC format. It can be represented by a specific time instant or by an ISO8601 interval. Model:'https://schema.org/DateTime'";
    rdf:type rdf:Property;
    rdfs:label "dateObserved";
    rdfs:domain <https://smart-data-models.github.io/dataModel.Weather/RainFallRadarObserved/schema.json>;
    rdfs:range xsd:dateTime.
sdm:dateObservedFrom dcterms:description "Property. Observation period start date and time. See dateObserved. It can be represented by a specific time instant or by an ISO8601 interval. Model:'https://schema.org/DateTime'";
    rdf:type rdf:Property;
    rdfs:label "dateObservedFrom";
    rdfs:domain <https://smart-data-models.github.io/dataModel.Weather/RainFallRadarObserved/schema.json>;
    rdfs:range xsd:dateTime.
sdm:dateObservedTo dcterms:description "Property. Observation period end date and time. See dateObserved. It can be represented by a specific time instant or by an ISO8601 interval. Model:'https://schema.org/DateTime'";
    rdf:type rdf:Property;
    rdfs:label "dateObservedTo";
    rdfs:domain <https://smart-data-models.github.io/dataModel.Weather/RainFallRadarObserved/schema.json>;
    rdfs:range xsd:dateTime.
sdm:rainFallRadarContent dcterms:description "Property. Path and filename which provided the information observed. Model:'https://schema.org/Text'";
    rdf:type rdf:Property;
    rdfs:label "rainFallRadarContent";
    rdfs:domain <https://smart-data-models.github.io/dataModel.Weather/RainFallRadarObserved/schema.json>;
    rdfs:range xsd:string.
sdm:numberOfRow dcterms:description "Property. Number of Rows allowing the reading of the `rainFallradarContent` attribute. Model:'https://schema.org/Number'";
    rdf:type rdf:Property;
    rdfs:label "numberOfRow";
    rdfs:domain <https://smart-data-models.github.io/dataModel.Weather/RainFallRadarObserved/schema.json>;
    rdfs:range xsd:decimal.
sdm:numberOfCol dcterms:description "Property. Number of Cols allowing the reading of the `rainFallradarContent` attribute. Model:'https://schema.org/Number'";
    rdf:type rdf:Property;
    rdfs:label "numberOfCol";
    rdfs:domain <https://smart-data-models.github.io/dataModel.Weather/RainFallRadarObserved/schema.json>;
    rdfs:range xsd:decimal.
sdm:cellsSize dcterms:description "Property. Size of each cell constituting the radar. The unit code (text) of measurement is given using the [UN/CEFACT Common Codes](http://wiki.goodrelations-vocabulary.org/Documentation/UN/CEFACT_Common_Codes). For instance, **MTR** represents **Meters**. Model:'https://schema.org/Number'";
    rdf:type rdf:Property;
    rdfs:label "cellsSize";
    rdfs:domain <https://smart-data-models.github.io/dataModel.Weather/RainFallRadarObserved/schema.json>;
    rdfs:range xsd:decimal.
sdm:mapScale dcterms:description "Property. Map Scale. Relationship between the length of the cellSize and its representation on the map. Model:'https://schema.org/Text'";
    rdf:type rdf:Property;
    rdfs:label "mapScale";
    rdfs:domain <https://smart-data-models.github.io/dataModel.Weather/RainFallRadarObserved/schema.json>;
    rdfs:range xsd:string.
sdm:measuredArea dcterms:description "Property. Reference of the surface measured. The unit code (text) is given using the [UN/CEFACT Common Codes](http://wiki.goodrelations-vocabulary.org/Documentation/UN/CEFACT_Common_Codes). For instance, **MTK** represents Square Meters. Model:'https://schema.org/Number'. Units:'square meters'";
    rdf:type rdf:Property;
    rdfs:label "measuredArea";
    rdfs:domain <https://smart-data-models.github.io/dataModel.Weather/RainFallRadarObserved/schema.json>;
    rdfs:range xsd:decimal.
