@prefix schema: <https://schema.org/>.
@prefix skos: <http://www.w3.org/2004/02/skos/core#>.
@prefix rdf: <http://www.w3.org/1999/02/22-rdf-syntax-ns#>.
@prefix rdfs: <http://www.w3.org/2000/01/rdf-schema#>.
@prefix foaf: <http://xmlns.com/foaf/0.1/>.
@prefix xsd: <http://www.w3.org/2001/XMLSchema#>.
@prefix dcterms: <http://purl.org/dc/terms/>.
@prefix owl: <http://www.w3.org/2002/07/owl#>.
@prefix jsonsc: <https://www.w3.org/2019/wot/json-schema#>.
@prefix jsonsc-ld: <http://w3id.org/jsonsc-ld/>.
@prefix api: <http://purl.org/linked-data/api/vocab>.
@prefix geo: <http://www.w3.org/2003/01/geo/wgs84_pos#>.
@prefix mobivoc: <http://schema.mobivoc.org/#>.
@prefix geosparql: <http://www.opengis.net/ont/geosparql#>.
@prefix sdm: <https://w3id.org/sdm#>.

<https://smart-data-models.github.io/dataModel.UnmannedAerialVehicle/UnmannedAerialVehicleADSB/schema.json> dcterms:title "Smart Data models - UAV-ADSB schema";
    dcterms:description "This entity contains a harmonised description of a generic UnmannedAerialVehicle (UAV) Automatic Dependent Surveillanceâ€“Broadcast. This entity is primarily associated with the control and management of Unmanned Aerial Vehicles. Each UAVADSB instance will be related to a specific UAV instance.".
sdm:type dcterms:description "Property. NGSI Entity identifier. It has to be UnmannedAerialVehicleADSB";
    rdf:type rdf:Property;
    rdfs:label "type";
    rdfs:domain <https://smart-data-models.github.io/dataModel.UnmannedAerialVehicle/UnmannedAerialVehicleADSB/schema.json>.
sdm:Type rdf:type skos:ConceptScheme.
sdm:type rdfs:range [
  owl:oneOf (sdm:UnmannedAerialVehicleADSB)
].
sdm:UnmannedAerialVehicleADSB rdf:type skos:Concept;
    skos:inScheme sdm:Type;
    rdfs:label "UnmannedAerialVehicleADSB".
sdm:UnmannedAerialVehicle dcterms:description "Relationship. Reference to the Unmanned Aerial Vehicle entity to which this broadcast message relates.";
    rdf:type rdf:Property;
    rdfs:label "UnmannedAerialVehicle";
    rdfs:domain <https://smart-data-models.github.io/dataModel.UnmannedAerialVehicle/UnmannedAerialVehicleADSB/schema.json>.
sdm:observedAt dcterms:description "Property. Indicates the date/time of the DBS broadcast.";
    rdf:type rdf:Property;
    rdfs:label "observedAt";
    rdfs:domain <https://smart-data-models.github.io/dataModel.UnmannedAerialVehicle/UnmannedAerialVehicleADSB/schema.json>;
    rdfs:range xsd:dateTime.
sdm:originatedByUnmannedAerialVehicle dcterms:description "Property. A logical indicator of source of the message. True indicates it is the UAV itself, false indicates that it is a different source, a listening station software application or a different UAV.";
    rdf:type rdf:Property;
    rdfs:label "originatedByUnmannedAerialVehicle";
    rdfs:domain <https://smart-data-models.github.io/dataModel.UnmannedAerialVehicle/UnmannedAerialVehicleADSB/schema.json>;
    rdfs:range xsd:boolean.
sdm:originator dcterms:description "Relationship. Refers to a third party UAV instance or other entity (e.g. listening station) that reported the information in the case the message was not directly originated by the UAV.";
    rdf:type rdf:Property;
    rdfs:label "originator";
    rdfs:domain <https://smart-data-models.github.io/dataModel.UnmannedAerialVehicle/UnmannedAerialVehicleADSB/schema.json>.
sdm:UnmannedAerialVehicleADSBroadcast dcterms:description "Property. A flight message describing the current flight status as a DBSB Message stored as a string of hexadecimal digits.";
    rdf:type rdf:Property;
    rdfs:label "UnmannedAerialVehicleADSBroadcast";
    rdfs:domain <https://smart-data-models.github.io/dataModel.UnmannedAerialVehicle/UnmannedAerialVehicleADSB/schema.json>;
    rdfs:range xsd:string.
