@prefix schema: <https://schema.org/>.
@prefix skos: <http://www.w3.org/2004/02/skos/core#>.
@prefix rdf: <http://www.w3.org/1999/02/22-rdf-syntax-ns#>.
@prefix rdfs: <http://www.w3.org/2000/01/rdf-schema#>.
@prefix foaf: <http://xmlns.com/foaf/0.1/>.
@prefix xsd: <http://www.w3.org/2001/XMLSchema#>.
@prefix dcterms: <http://purl.org/dc/terms/>.
@prefix owl: <http://www.w3.org/2002/07/owl#>.
@prefix jsonsc: <https://www.w3.org/2019/wot/json-schema#>.
@prefix jsonsc-ld: <http://w3id.org/jsonsc-ld/>.
@prefix api: <http://purl.org/linked-data/api/vocab>.
@prefix geo: <http://www.w3.org/2003/01/geo/wgs84_pos#>.
@prefix mobivoc: <http://schema.mobivoc.org/#>.
@prefix geosparql: <http://www.opengis.net/ont/geosparql#>.
@prefix sdm: <https://w3id.org/sdm#>.

<https://smart-data-models.github.io/data-models.OpenChannelManagement/OpenChannelSystem/schema.json> dcterms:title "Open Channel Management - OpenChannelSystem";
    dcterms:description "This entity contains a harmonised description of a generic system made for Raw-Water (Open Channels) System Management domain. This entity represents either a system composed of different components (e.g., channels, junctions, cross-sections etc.) or just a component (e.g., a SluiceGate).".
sdm:type dcterms:description "Property. NGSI-LD Entity Type. It has to be OpenChannelSystem";
    rdf:type rdf:Property;
    rdfs:label "type";
    rdfs:domain <https://smart-data-models.github.io/data-models.OpenChannelManagement/OpenChannelSystem/schema.json>.
sdm:Type rdf:type skos:ConceptScheme.
sdm:type rdfs:range [
  owl:oneOf (sdm:OpenChannelSystem)
].
sdm:OpenChannelSystem rdf:type skos:Concept;
    skos:inScheme sdm:Type;
    rdfs:label "OpenChannelSystem".
sdm:isComposedOf dcterms:description "Relationship. Reference to the component entities of the open-channel system, of type Channel, Cross-Section, Junction, Regulation Structure, SluiceGate, Spillway.";
    rdf:type rdf:Property;
    rdfs:label "isComposedOf";
    rdfs:domain <https://smart-data-models.github.io/data-models.OpenChannelManagement/OpenChannelSystem/schema.json>.
sdm:hasSubSystem dcterms:description "Relationship. Reference to an entity of type OpenChannelSystem - an open-channel sub-system.";
    rdf:type rdf:Property;
    rdfs:label "hasSubSystem";
    rdfs:domain <https://smart-data-models.github.io/data-models.OpenChannelManagement/OpenChannelSystem/schema.json>.
sdm:mostUpstreamPoint dcterms:description "Relationship. A relationship indicating the ID of the most upstream node (e.g., a Junction or a Cross-section) of the system.";
    rdf:type rdf:Property;
    rdfs:label "mostUpstreamPoint";
    rdfs:domain <https://smart-data-models.github.io/data-models.OpenChannelManagement/OpenChannelSystem/schema.json>.
sdm:mostDownstreamPoint dcterms:description "Relationship. A relationship indicating the ID of the most downstream node (e.g., a Junction or a Cross-section) of the system.";
    rdf:type rdf:Property;
    rdfs:label "mostDownstreamPoint";
    rdfs:domain <https://smart-data-models.github.io/data-models.OpenChannelManagement/OpenChannelSystem/schema.json>.
