@prefix schema: <https://schema.org/>.
@prefix skos: <http://www.w3.org/2004/02/skos/core#>.
@prefix rdf: <http://www.w3.org/1999/02/22-rdf-syntax-ns#>.
@prefix rdfs: <http://www.w3.org/2000/01/rdf-schema#>.
@prefix foaf: <http://xmlns.com/foaf/0.1/>.
@prefix xsd: <http://www.w3.org/2001/XMLSchema#>.
@prefix dcterms: <http://purl.org/dc/terms/>.
@prefix owl: <http://www.w3.org/2002/07/owl#>.
@prefix jsonsc: <https://www.w3.org/2019/wot/json-schema#>.
@prefix jsonsc-ld: <http://w3id.org/jsonsc-ld/>.
@prefix api: <http://purl.org/linked-data/api/vocab>.
@prefix geo: <http://www.w3.org/2003/01/geo/wgs84_pos#>.
@prefix mobivoc: <http://schema.mobivoc.org/#>.
@prefix geosparql: <http://www.opengis.net/ont/geosparql#>.
@prefix sdm: <https://w3id.org/sdm#>.

<https://smart-data-models.github.io/dataModels.CIMEnergyClasses/PFVArType2IEEEPFController/schema.json> dcterms:title " Smart Data Models - PFVArType2IEEEPFController";
    dcterms:description "Adapted from CIM data models. The class represents IEEE PF Controller Type 2 which is a summing point type controller and makes up the outside loop of a two-loop system. This controller is implemented as a slow PI type controller. The voltage regulator forms the inner loop and is implemented as a fast controller.  Reference: IEEE Standard 421.5-2005 Section 11.4.".
sdm:type dcterms:description "Property. NGSI type. It has to be PFVArType2IEEEPFController";
    rdf:type rdf:Property;
    rdfs:label "type";
    rdfs:domain <https://smart-data-models.github.io/dataModels.CIMEnergyClasses/PFVArType2IEEEPFController/schema.json>.
sdm:Type rdf:type skos:ConceptScheme.
sdm:type rdfs:range [
  owl:oneOf (sdm:PFVArType2IEEEPFController)
].
sdm:PFVArType2IEEEPFController rdf:type skos:Concept;
    skos:inScheme sdm:Type;
    rdfs:label "PFVArType2IEEEPFController".
sdm:exlon dcterms:description "Property. Model:'https://schema.org/Number'. Overexcitation or under excitation flag () true = 1 (not in the overexcitation or underexcitation state, integral action is active) false = 0 (in the overexcitation or underexcitation state, so integral action is disabled to allow the limiter to play its role). Default: False";
    rdf:type rdf:Property;
    rdfs:label "exlon";
    rdfs:domain <https://smart-data-models.github.io/dataModels.CIMEnergyClasses/PFVArType2IEEEPFController/schema.json>;
    rdfs:range xsd:decimal.
sdm:ki dcterms:description "Property. Model:'https://schema.org/Number'. Integral gain of the pf controller ().  Typical Value = 1. Default: 0.0";
    rdf:type rdf:Property;
    rdfs:label "ki";
    rdfs:domain <https://smart-data-models.github.io/dataModels.CIMEnergyClasses/PFVArType2IEEEPFController/schema.json>;
    rdfs:range xsd:decimal.
sdm:kp dcterms:description "Property. Model:'https://schema.org/Number'. Proportional gain of the pf controller ().  Typical Value = 1. Default: 0.0";
    rdf:type rdf:Property;
    rdfs:label "kp";
    rdfs:domain <https://smart-data-models.github.io/dataModels.CIMEnergyClasses/PFVArType2IEEEPFController/schema.json>;
    rdfs:range xsd:decimal.
sdm:pfref dcterms:description "Property. Model:'https://schema.org/Number'. Power factor reference (). Default: 0.0";
    rdf:type rdf:Property;
    rdfs:label "pfref";
    rdfs:domain <https://smart-data-models.github.io/dataModels.CIMEnergyClasses/PFVArType2IEEEPFController/schema.json>;
    rdfs:range xsd:decimal.
sdm:vclmt dcterms:description "Property. Model:'https://schema.org/Number'. Maximum output of the pf controller ().  Typical Value = 0.1. Default: 0.0";
    rdf:type rdf:Property;
    rdfs:label "vclmt";
    rdfs:domain <https://smart-data-models.github.io/dataModels.CIMEnergyClasses/PFVArType2IEEEPFController/schema.json>;
    rdfs:range xsd:decimal.
sdm:vref dcterms:description "Property. Model:'https://schema.org/Number'. Voltage regulator reference (). Default: 0.0";
    rdf:type rdf:Property;
    rdfs:label "vref";
    rdfs:domain <https://smart-data-models.github.io/dataModels.CIMEnergyClasses/PFVArType2IEEEPFController/schema.json>;
    rdfs:range xsd:decimal.
sdm:vs dcterms:description "Property. Model:'https://schema.org/Number'. Generator sensing voltage (). Default: 0.0";
    rdf:type rdf:Property;
    rdfs:label "vs";
    rdfs:domain <https://smart-data-models.github.io/dataModels.CIMEnergyClasses/PFVArType2IEEEPFController/schema.json>;
    rdfs:range xsd:decimal.
