@prefix schema: <https://schema.org/>.
@prefix skos: <http://www.w3.org/2004/02/skos/core#>.
@prefix rdf: <http://www.w3.org/1999/02/22-rdf-syntax-ns#>.
@prefix rdfs: <http://www.w3.org/2000/01/rdf-schema#>.
@prefix foaf: <http://xmlns.com/foaf/0.1/>.
@prefix xsd: <http://www.w3.org/2001/XMLSchema#>.
@prefix dcterms: <http://purl.org/dc/terms/>.
@prefix owl: <http://www.w3.org/2002/07/owl#>.
@prefix jsonsc: <https://www.w3.org/2019/wot/json-schema#>.
@prefix jsonsc-ld: <http://w3id.org/jsonsc-ld/>.
@prefix api: <http://purl.org/linked-data/api/vocab>.
@prefix geo: <http://www.w3.org/2003/01/geo/wgs84_pos#>.
@prefix mobivoc: <http://schema.mobivoc.org/#>.
@prefix geosparql: <http://www.opengis.net/ont/geosparql#>.
@prefix sdm: <https://w3id.org/sdm#>.

<https://smart-data-models.github.io/dataModel.GreenEnergy/GreenEnergyMeasurement/schema.json> dcterms:title "GSMA / Smart Data Models - GreenEnergyMeasurement";
    dcterms:description "A instantaneous measure of power generation using green energy sources".
sdm:type dcterms:description "Property. NGSI Entity Type. It has to be GreenEnergyMeasurement";
    rdf:type rdf:Property;
    rdfs:label "type";
    rdfs:domain <https://smart-data-models.github.io/dataModel.GreenEnergy/GreenEnergyMeasurement/schema.json>.
sdm:Type rdf:type skos:ConceptScheme.
sdm:type rdfs:range [
  owl:oneOf (sdm:GreenEnergyMeasurement)
].
sdm:GreenEnergyMeasurement rdf:type skos:Concept;
    skos:inScheme sdm:Type;
    rdfs:label "GreenEnergyMeasurement".
sdm:solarPowerGenerated dcterms:description "Property. Model:'https://schema.org/Number'. Specifies the amount of power generated using solar energy. Units:'KWT'. The unit code (text) of measurement given using the UN/CEFACT Common Code (max. 3 characters).";
    rdf:type rdf:Property;
    rdfs:label "solarPowerGenerated";
    rdfs:domain <https://smart-data-models.github.io/dataModel.GreenEnergy/GreenEnergyMeasurement/schema.json>;
    rdfs:range xsd:decimal.
sdm:eolicPowerGenerated dcterms:description "Property. Model:'https://schema.org/Number'. Specifies the amount of power generated using eolic energy. Units:'KWT'. The unit code (text) of measurement given using the UN/CEFACT Common Code (max. 3 characters).";
    rdf:type rdf:Property;
    rdfs:label "eolicPowerGenerated";
    rdfs:domain <https://smart-data-models.github.io/dataModel.GreenEnergy/GreenEnergyMeasurement/schema.json>;
    rdfs:range xsd:decimal.
sdm:hydroPowerGenerated dcterms:description "Property. Model:'https://schema.org/Number'. Specifies the amount of power generated using hydropower energy. Units:'KWT'. The unit code (text) of measurement given using the UN/CEFACT Common Code (max. 3 characters).";
    rdf:type rdf:Property;
    rdfs:label "hydroPowerGenerated";
    rdfs:domain <https://smart-data-models.github.io/dataModel.GreenEnergy/GreenEnergyMeasurement/schema.json>;
    rdfs:range xsd:decimal.
sdm:biomassPowerGenerated dcterms:description "Property. Model:'https://schema.org/Number'. Specifies the amount of power generated using biomass energy. Units:'KWT'. The unit code (text) of measurement given using the UN/CEFACT Common Code (max. 3 characters).";
    rdf:type rdf:Property;
    rdfs:label "biomassPowerGenerated";
    rdfs:domain <https://smart-data-models.github.io/dataModel.GreenEnergy/GreenEnergyMeasurement/schema.json>;
    rdfs:range xsd:decimal.
sdm:geothermalPowerGenerated dcterms:description "Property. Model:'https://schema.org/Number'. Specifies the amount of power generated using geothermal energy. Units:'KWT'. The unit code (text) of measurement given using the UN/CEFACT Common Code (max. 3 characters).";
    rdf:type rdf:Property;
    rdfs:label "geothermalPowerGenerated";
    rdfs:domain <https://smart-data-models.github.io/dataModel.GreenEnergy/GreenEnergyMeasurement/schema.json>;
    rdfs:range xsd:decimal.
sdm:refGreenEnergyGenerator dcterms:description "Relationship. Model:'https://schema.org/URL'. A reference to the entity `GreenEnergyGenerator` which it belongs the measurement.";
    rdf:type rdf:Property;
    rdfs:label "refGreenEnergyGenerator";
    rdfs:domain <https://smart-data-models.github.io/dataModel.GreenEnergy/GreenEnergyMeasurement/schema.json>.
