@prefix schema: <https://schema.org/>.
@prefix skos: <http://www.w3.org/2004/02/skos/core#>.
@prefix rdf: <http://www.w3.org/1999/02/22-rdf-syntax-ns#>.
@prefix rdfs: <http://www.w3.org/2000/01/rdf-schema#>.
@prefix foaf: <http://xmlns.com/foaf/0.1/>.
@prefix xsd: <http://www.w3.org/2001/XMLSchema#>.
@prefix dcterms: <http://purl.org/dc/terms/>.
@prefix owl: <http://www.w3.org/2002/07/owl#>.
@prefix jsonsc: <https://www.w3.org/2019/wot/json-schema#>.
@prefix jsonsc-ld: <http://w3id.org/jsonsc-ld/>.
@prefix api: <http://purl.org/linked-data/api/vocab>.
@prefix geo: <http://www.w3.org/2003/01/geo/wgs84_pos#>.
@prefix mobivoc: <http://schema.mobivoc.org/#>.
@prefix geosparql: <http://www.opengis.net/ont/geosparql#>.
@prefix sdm: <https://w3id.org/sdm#>.

<https://smart-data-models.github.io/dataModel.Device/SmartMeteringObservation/schema.json> dcterms:title " Smart Data Models - Smart Metering Observation";
    dcterms:description "This entity contains a harmonised description of a Smart Meter Observation, generally applicable for Smart Homes, Industry, Cities and Agriculture. It is based mostly in the GSMA entity definition but it is extended".
sdm:type dcterms:description "Property. It has to be SmartMeteringObservation. NGSI entity type";
    rdf:type rdf:Property;
    rdfs:label "type";
    rdfs:domain <https://smart-data-models.github.io/dataModel.Device/SmartMeteringObservation/schema.json>.
sdm:Type rdf:type skos:ConceptScheme.
sdm:type rdfs:range [
  owl:oneOf (sdm:SmartMeteringObservation)
].
sdm:SmartMeteringObservation rdf:type skos:Concept;
    skos:inScheme sdm:Type;
    rdfs:label "SmartMeteringObservation".
sdm:entityVersion dcterms:description "Property. Model:'https://schema.org/Text'. The entity specification version. A version number of 2.0 or later denotes the entity is represented using NGSI-LD";
    rdf:type rdf:Property;
    rdfs:label "entityVersion";
    rdfs:domain <https://smart-data-models.github.io/dataModel.Device/SmartMeteringObservation/schema.json>.
sdm:EntityVersion rdf:type skos:ConceptScheme.
sdm:entityVersion rdfs:range [
  owl:oneOf (sdm:2.0 sdm:LD)
].
sdm:2.0 rdf:type skos:Concept;
    skos:inScheme sdm:EntityVersion;
    rdfs:label "2.0".
sdm:LD rdf:type skos:Concept;
    skos:inScheme sdm:EntityVersion;
    rdfs:label "LD".
sdm:meterType dcterms:description "Property. The type of supply being metered e.g.: Electricity, Gasoline, Water, Methane, Diesel.";
    rdf:type rdf:Property;
    rdfs:label "meterType";
    rdfs:domain <https://smart-data-models.github.io/dataModel.Device/SmartMeteringObservation/schema.json>;
    rdfs:range xsd:string.
sdm:refDevice dcterms:description "Relationship. Unique identifier of the entity (Device) linked to the SmartMeteringObservation";
    rdf:type rdf:Property;
    rdfs:label "refDevice";
    rdfs:domain <https://smart-data-models.github.io/dataModel.Device/SmartMeteringObservation/schema.json>.
sdm:totalConsumption dcterms:description "Property. The total amount of product supplied as recorded by the meter since installation. The relevant unitCode should be specified such as KWH (Kilo Watt Hours) for Electricity, LTR (Litre) or MTQ (Cubic Metre) for gases or liquids.";
    rdf:type rdf:Property;
    rdfs:label "totalConsumption";
    rdfs:domain <https://smart-data-models.github.io/dataModel.Device/SmartMeteringObservation/schema.json>;
    rdfs:range xsd:decimal.
sdm:peakConsumption dcterms:description "Property. The total amount of product supplied during 'peak' hours (particularly relevant to Electricity supply) as recorded by the meter since installation. The relevant unitCode should be specified such as KWH (Kilo Watt Hours) for Electricity, LTR (Litre) or MTQ (Cubic Metre) for gases or liquids.";
    rdf:type rdf:Property;
    rdfs:label "peakConsumption";
    rdfs:domain <https://smart-data-models.github.io/dataModel.Device/SmartMeteringObservation/schema.json>;
    rdfs:range xsd:decimal.
sdm:offPeakConsumption dcterms:description "Property. The total amount of product supplied during 'off-peak' hours (particularly relevant to Electricity supply) as recorded by the meter since installation. The relevant unitCode should be specified such as KWH (Kilo Watt Hours) for Electricity, LTR (Litre) or MTQ (Cubic Metre) for gases or liquids.";
    rdf:type rdf:Property;
    rdfs:label "offPeakConsumption";
    rdfs:domain <https://smart-data-models.github.io/dataModel.Device/SmartMeteringObservation/schema.json>;
    rdfs:range xsd:decimal.
sdm:powerFactor dcterms:description "Property. Relevant to 3-Phase electricity supplies often used in industry - the power factor ranges from -1 to +1 depending on the net balance between capacitive and inductive loads. If used this measures the average power factor since meter installation.";
    rdf:type rdf:Property;
    rdfs:label "powerFactor";
    rdfs:domain <https://smart-data-models.github.io/dataModel.Device/SmartMeteringObservation/schema.json>;
    rdfs:range xsd:decimal.
