@prefix schema: <https://schema.org/>.
@prefix skos: <http://www.w3.org/2004/02/skos/core#>.
@prefix rdf: <http://www.w3.org/1999/02/22-rdf-syntax-ns#>.
@prefix rdfs: <http://www.w3.org/2000/01/rdf-schema#>.
@prefix foaf: <http://xmlns.com/foaf/0.1/>.
@prefix xsd: <http://www.w3.org/2001/XMLSchema#>.
@prefix dcterms: <http://purl.org/dc/terms/>.
@prefix owl: <http://www.w3.org/2002/07/owl#>.
@prefix jsonsc: <https://www.w3.org/2019/wot/json-schema#>.
@prefix jsonsc-ld: <http://w3id.org/jsonsc-ld/>.
@prefix api: <http://purl.org/linked-data/api/vocab>.
@prefix geo: <http://www.w3.org/2003/01/geo/wgs84_pos#>.
@prefix mobivoc: <http://schema.mobivoc.org/#>.
@prefix geosparql: <http://www.opengis.net/ont/geosparql#>.
@prefix sdm: <https://w3id.org/sdm#>.

<https://smart-data-models.github.io/dataModels.CIMEnergyClasses/ExcAC4A/schema.json> dcterms:title " Smart Data Models - ExcAC4A";
    dcterms:description "Adapted from CIM data models. Modified IEEE AC4A alternator-supplied rectifier excitation system with different minimum controller output.".
sdm:type dcterms:description "Property. NGSI type. It has to be ExcAC4A";
    rdf:type rdf:Property;
    rdfs:label "type";
    rdfs:domain <https://smart-data-models.github.io/dataModels.CIMEnergyClasses/ExcAC4A/schema.json>.
sdm:Type rdf:type skos:ConceptScheme.
sdm:type rdfs:range [
  owl:oneOf (sdm:ExcAC4A)
].
sdm:ExcAC4A rdf:type skos:Concept;
    skos:inScheme sdm:Type;
    rdfs:label "ExcAC4A".
sdm:ka dcterms:description "Property. Model:'https://schema.org/Number'. Voltage regulator gain (Ka).  Typical Value = 200. Default: 0.0";
    rdf:type rdf:Property;
    rdfs:label "ka";
    rdfs:domain <https://smart-data-models.github.io/dataModels.CIMEnergyClasses/ExcAC4A/schema.json>;
    rdfs:range xsd:decimal.
sdm:kc dcterms:description "Property. Model:'https://schema.org/Number'. Rectifier loading factor proportional to commutating reactance (Kc).  Typical Value = 0. Default: 0.0";
    rdf:type rdf:Property;
    rdfs:label "kc";
    rdfs:domain <https://smart-data-models.github.io/dataModels.CIMEnergyClasses/ExcAC4A/schema.json>;
    rdfs:range xsd:decimal.
sdm:ta dcterms:description "Property. Model:'https://schema.org/Number'. Voltage regulator time constant (Ta).  Typical Value = 0.015. Default: 0";
    rdf:type rdf:Property;
    rdfs:label "ta";
    rdfs:domain <https://smart-data-models.github.io/dataModels.CIMEnergyClasses/ExcAC4A/schema.json>;
    rdfs:range xsd:decimal.
sdm:tb dcterms:description "Property. Model:'https://schema.org/Number'. Voltage regulator time constant (Tb).  Typical Value = 10. Default: 0";
    rdf:type rdf:Property;
    rdfs:label "tb";
    rdfs:domain <https://smart-data-models.github.io/dataModels.CIMEnergyClasses/ExcAC4A/schema.json>;
    rdfs:range xsd:decimal.
sdm:tc dcterms:description "Property. Model:'https://schema.org/Number'. Voltage regulator time constant (Tc).  Typical Value = 1. Default: 0";
    rdf:type rdf:Property;
    rdfs:label "tc";
    rdfs:domain <https://smart-data-models.github.io/dataModels.CIMEnergyClasses/ExcAC4A/schema.json>;
    rdfs:range xsd:decimal.
sdm:vimax dcterms:description "Property. Model:'https://schema.org/Number'. Maximum voltage regulator input limit (Vimax).  Typical Value = 10. Default: 0.0";
    rdf:type rdf:Property;
    rdfs:label "vimax";
    rdfs:domain <https://smart-data-models.github.io/dataModels.CIMEnergyClasses/ExcAC4A/schema.json>;
    rdfs:range xsd:decimal.
sdm:vimin dcterms:description "Property. Model:'https://schema.org/Number'. Minimum voltage regulator input limit (Vimin).  Typical Value = -10. Default: 0.0";
    rdf:type rdf:Property;
    rdfs:label "vimin";
    rdfs:domain <https://smart-data-models.github.io/dataModels.CIMEnergyClasses/ExcAC4A/schema.json>;
    rdfs:range xsd:decimal.
sdm:vrmax dcterms:description "Property. Model:'https://schema.org/Number'. Maximum voltage regulator output (Vrmax).  Typical Value = 5.64. Default: 0.0";
    rdf:type rdf:Property;
    rdfs:label "vrmax";
    rdfs:domain <https://smart-data-models.github.io/dataModels.CIMEnergyClasses/ExcAC4A/schema.json>;
    rdfs:range xsd:decimal.
sdm:vrmin dcterms:description "Property. Model:'https://schema.org/Number'. Minimum voltage regulator output (Vrmin).  Typical Value = -4.53. Default: 0.0";
    rdf:type rdf:Property;
    rdfs:label "vrmin";
    rdfs:domain <https://smart-data-models.github.io/dataModels.CIMEnergyClasses/ExcAC4A/schema.json>;
    rdfs:range xsd:decimal.
