@prefix schema: <https://schema.org/>.
@prefix skos: <http://www.w3.org/2004/02/skos/core#>.
@prefix rdf: <http://www.w3.org/1999/02/22-rdf-syntax-ns#>.
@prefix rdfs: <http://www.w3.org/2000/01/rdf-schema#>.
@prefix foaf: <http://xmlns.com/foaf/0.1/>.
@prefix xsd: <http://www.w3.org/2001/XMLSchema#>.
@prefix dcterms: <http://purl.org/dc/terms/>.
@prefix owl: <http://www.w3.org/2002/07/owl#>.
@prefix jsonsc: <https://www.w3.org/2019/wot/json-schema#>.
@prefix jsonsc-ld: <http://w3id.org/jsonsc-ld/>.
@prefix api: <http://purl.org/linked-data/api/vocab>.
@prefix geo: <http://www.w3.org/2003/01/geo/wgs84_pos#>.
@prefix mobivoc: <http://schema.mobivoc.org/#>.
@prefix geosparql: <http://www.opengis.net/ont/geosparql#>.
@prefix sdm: <https://w3id.org/sdm#>.

<https://smart-data-models.github.io/data-models/specs/WasteWaterTreatment/WasteWaterJunction/schema.json> dcterms:title "WasteWaterTreatment - Junction";
    dcterms:description "This entity contains an harmonised description of a generic Junction made for the Wastewater treatment domain. Junctions could be in place in certain sections of thetreatment plant. In wastewater treatment purposes, the junction is most useful if it is a locationof a sensor that measures a specific variable.".
sdm:type dcterms:description "Property. It has to be WasteWaterJunction. NGSI-LD Entity Type";
    rdf:type rdf:Property;
    rdfs:label "type";
    rdfs:domain <https://smart-data-models.github.io/data-models/specs/WasteWaterTreatment/WasteWaterJunction/schema.json>.
sdm:Type rdf:type skos:ConceptScheme.
sdm:type rdfs:range [
  owl:oneOf (sdm:WasteWaterJunction)
].
sdm:WasteWaterJunction rdf:type skos:Concept;
    skos:inScheme sdm:Type;
    rdfs:label "WasteWaterJunction".
sdm:toc dcterms:description "Property. Model: https://schema.org/Number. Units: 'mg/L'. Total Organic Carbon concentration measured in the influent or effluent.";
    rdf:type rdf:Property;
    rdfs:label "toc";
    rdfs:domain <https://smart-data-models.github.io/data-models/specs/WasteWaterTreatment/WasteWaterJunction/schema.json>;
    rdfs:range xsd:decimal.
sdm:tic dcterms:description "Property. Model: https://schema.org/Number. Units: 'mg/L'. Total Inorganic Carbon concentration measured in the influent or effluent.";
    rdf:type rdf:Property;
    rdfs:label "tic";
    rdfs:domain <https://smart-data-models.github.io/data-models/specs/WasteWaterTreatment/WasteWaterJunction/schema.json>;
    rdfs:range xsd:decimal.
sdm:po4 dcterms:description "Property. Model: https://schema.org/Number. Units: 'mg/L'. Ortho-phosphate concentration measured in wastewater.";
    rdf:type rdf:Property;
    rdfs:label "po4";
    rdfs:domain <https://smart-data-models.github.io/data-models/specs/WasteWaterTreatment/WasteWaterJunction/schema.json>;
    rdfs:range xsd:decimal.
sdm:bod dcterms:description "Property. Model: https://schema.org/Number. Units: 'mg/L'. Biological Oxygen Demand concentration measured in the influent or effluent.";
    rdf:type rdf:Property;
    rdfs:label "bod";
    rdfs:domain <https://smart-data-models.github.io/data-models/specs/WasteWaterTreatment/WasteWaterJunction/schema.json>;
    rdfs:range xsd:decimal.
sdm:cod dcterms:description "Property. Model: https://schema.org/Number. Units: 'mg/L'. Chemical Oxygen Demand concentration measured in the influent or effluent.";
    rdf:type rdf:Property;
    rdfs:label "cod";
    rdfs:domain <https://smart-data-models.github.io/data-models/specs/WasteWaterTreatment/WasteWaterJunction/schema.json>;
    rdfs:range xsd:decimal.
sdm:flowrate dcterms:description "Property. Model: https://schema.org/Number. Units: 'm3/h'. Flowrate of wastewater.";
    rdf:type rdf:Property;
    rdfs:label "flowrate";
    rdfs:domain <https://smart-data-models.github.io/data-models/specs/WasteWaterTreatment/WasteWaterJunction/schema.json>;
    rdfs:range xsd:decimal.
sdm:pressure dcterms:description "Property. Model: https://schema.org/Number. Units: kPa. Pressure measured at given location. Most relevant for airflow as provided by blowers to wastewater tanks";
    rdf:type rdf:Property;
    rdfs:label "pressure";
    rdfs:domain <https://smart-data-models.github.io/data-models/specs/WasteWaterTreatment/WasteWaterJunction/schema.json>;
    rdfs:range xsd:decimal.
sdm:emissionFlow dcterms:description "Property. Model: https://schema.org/Number. Units: 'm3'. Gas emission flow volume measured at a junction prior to being emitted in an off-gas stack.";
    rdf:type rdf:Property;
    rdfs:label "emissionFlow";
    rdfs:domain <https://smart-data-models.github.io/data-models/specs/WasteWaterTreatment/WasteWaterJunction/schema.json>;
    rdfs:range xsd:decimal.
sdm:startsAt dcterms:description "Relationship. A relationship indicating the entity the junction is connected to in the upstream point";
    rdf:type rdf:Property;
    rdfs:label "startsAt";
    rdfs:domain <https://smart-data-models.github.io/data-models/specs/WasteWaterTreatment/WasteWaterJunction/schema.json>;
    rdfs:range xsd:anyURI.
sdm:endsAt dcterms:description "Relationship. A relationship indicating the entity the junction is connected to in the downstream point";
    rdf:type rdf:Property;
    rdfs:label "endsAt";
    rdfs:domain <https://smart-data-models.github.io/data-models/specs/WasteWaterTreatment/WasteWaterJunction/schema.json>;
    rdfs:range xsd:anyURI.
