@prefix schema: <https://schema.org/>.
@prefix skos: <http://www.w3.org/2004/02/skos/core#>.
@prefix rdf: <http://www.w3.org/1999/02/22-rdf-syntax-ns#>.
@prefix rdfs: <http://www.w3.org/2000/01/rdf-schema#>.
@prefix foaf: <http://xmlns.com/foaf/0.1/>.
@prefix xsd: <http://www.w3.org/2001/XMLSchema#>.
@prefix dcterms: <http://purl.org/dc/terms/>.
@prefix owl: <http://www.w3.org/2002/07/owl#>.
@prefix jsonsc: <https://www.w3.org/2019/wot/json-schema#>.
@prefix jsonsc-ld: <http://w3id.org/jsonsc-ld/>.
@prefix api: <http://purl.org/linked-data/api/vocab>.
@prefix geo: <http://www.w3.org/2003/01/geo/wgs84_pos#>.
@prefix mobivoc: <http://schema.mobivoc.org/#>.
@prefix geosparql: <http://www.opengis.net/ont/geosparql#>.
@prefix sdm: <https://w3id.org/sdm#>.

<https://smart-data-models.github.io/data-models/Environment/ElectroMagneticObserved/schema.json> dcterms:title "Smart - Data - Models. Electro Magnetic Observed schema";
    dcterms:description "The Data Model is intended to measure excessive electric and magnetic fields (EMFs), or radiation in a work or public environment according to the level of exposure to electromagnetic fields on the air. The frequency of the hertzian waves is conventionally lower than 300 GHz, propagating in space without artificial guide. They are between 9 kHz and 300 GHz.".
sdm:type dcterms:description "Property. Model:'https://schema.org/Text'. It has to be ElectroMagneticObserved";
    rdf:type rdf:Property;
    rdfs:label "type";
    rdfs:domain <https://smart-data-models.github.io/data-models/Environment/ElectroMagneticObserved/schema.json>.
sdm:Type rdf:type skos:ConceptScheme.
sdm:type rdfs:range [
  owl:oneOf (sdm:ElectroMagneticObserved)
].
sdm:ElectroMagneticObserved rdf:type skos:Concept;
    skos:inScheme sdm:Type;
    rdfs:label "ElectroMagneticObserved".
sdm:refDevice dcterms:description "Relationship. Model:'https://schema.org/URL'. Reference to a [Device](https://github.com/smart-data-models/dataModel.Device/blob/master/Device/doc/spec.md) which captured this observation.";
    rdf:type rdf:Property;
    rdfs:label "refDevice";
    rdfs:domain <https://smart-data-models.github.io/data-models/Environment/ElectroMagneticObserved/schema.json>.
sdm:refPointOfInterest dcterms:description "Relationship. Model:'https://schema.org/URL'. Reference to a [Point Of Interest](https://github.com/smart-data-models/dataModel.PointOfInterest/blob/master/PointOfInterest/doc/spec.md) linked with the observation.";
    rdf:type rdf:Property;
    rdfs:label "refPointOfInterest";
    rdfs:domain <https://smart-data-models.github.io/data-models/Environment/ElectroMagneticObserved/schema.json>.
sdm:dateObserved dcterms:description "Property. Model:'https://schema.org/DateTime'. Date and time of this observation represented by an ISO8601 UTC format. It can be represented by an specific time instant or by an ISO8601 interval to separate attributes `dateObservedFrom`, `dateObservedTo`. ";
    rdf:type rdf:Property;
    rdfs:label "dateObserved";
    rdfs:domain <https://smart-data-models.github.io/data-models/Environment/ElectroMagneticObserved/schema.json>;
    rdfs:range xsd:dateTime.
sdm:dateObservedFrom dcterms:description "Property. Model:'https://schema.org/DateTime'. Observation period: Start date and time in an ISO8601 UTC format. The attribute can be used in addition to the `dateObserved` attribute when it corresponds to a time interval to be highlighted. ";
    rdf:type rdf:Property;
    rdfs:label "dateObservedFrom";
    rdfs:domain <https://smart-data-models.github.io/data-models/Environment/ElectroMagneticObserved/schema.json>;
    rdfs:range xsd:dateTime.
sdm:dateObservedTo dcterms:description "Property. Model:'https://schema.org/'. Observation period: End date and time in an ISO8601 UTC format. The attribute can be used in addition to the `dateObserved` attribute when it corresponds to a time interval to be highlighted.";
    rdf:type rdf:Property;
    rdfs:label "dateObservedTo";
    rdfs:domain <https://smart-data-models.github.io/data-models/Environment/ElectroMagneticObserved/schema.json>;
    rdfs:range xsd:dateTime.
sdm:eMF dcterms:description "Property. Model:'https://schema.org/Number'. Level corresponding to the observed survey. The unit code (text) is given using the [UN/CEFACT Common Codes](http://wiki.goodrelations-vocabulary.org/Documentation/UN/CEFACT_Common_Codes). For instance, **MHz** represents Mega Hertz. ";
    rdf:type rdf:Property;
    rdfs:label "eMF";
    rdfs:domain <https://smart-data-models.github.io/data-models/Environment/ElectroMagneticObserved/schema.json>;
    rdfs:range xsd:decimal.
sdm:reliability dcterms:description "Property. Model:'https://schema.org/'. Percent for confidence Factor. The unit code (text) is given using the [UN/CEFACT Common Codes](http://wiki.goodrelations-vocabulary.org/Documentation/UN/CEFACT_Common_Codes). For instance, **P1** represents Percent. ";
    rdf:type rdf:Property;
    rdfs:label "reliability";
    rdfs:domain <https://smart-data-models.github.io/data-models/Environment/ElectroMagneticObserved/schema.json>;
    rdfs:range xsd:decimal.
