@prefix schema: <https://schema.org/>.
@prefix skos: <http://www.w3.org/2004/02/skos/core#>.
@prefix rdf: <http://www.w3.org/1999/02/22-rdf-syntax-ns#>.
@prefix rdfs: <http://www.w3.org/2000/01/rdf-schema#>.
@prefix foaf: <http://xmlns.com/foaf/0.1/>.
@prefix xsd: <http://www.w3.org/2001/XMLSchema#>.
@prefix dcterms: <http://purl.org/dc/terms/>.
@prefix owl: <http://www.w3.org/2002/07/owl#>.
@prefix jsonsc: <https://www.w3.org/2019/wot/json-schema#>.
@prefix jsonsc-ld: <http://w3id.org/jsonsc-ld/>.
@prefix api: <http://purl.org/linked-data/api/vocab>.
@prefix geo: <http://www.w3.org/2003/01/geo/wgs84_pos#>.
@prefix mobivoc: <http://schema.mobivoc.org/#>.
@prefix geosparql: <http://www.opengis.net/ont/geosparql#>.
@prefix sdm: <https://w3id.org/sdm#>.

<https://smart-data-models.github.io/data-models.OpenChannelManagement/CrossSection/schema.json> dcterms:title "Smart Data Models - CrossSection ";
    dcterms:description "This entity contains a harmonised description of a generic Cross-Section made for Raw-Water (Open Channels) System Management domain. A CrossSection defines any point of the system where raw-water properties are monitored by a device and/or computed via simulation.".
sdm:type dcterms:description "Property. NGSI-LD Entity Type. It has to be CrossSection.";
    rdf:type rdf:Property;
    rdfs:label "type";
    rdfs:domain <https://smart-data-models.github.io/data-models.OpenChannelManagement/CrossSection/schema.json>.
sdm:Type rdf:type skos:ConceptScheme.
sdm:type rdfs:range [
  owl:oneOf (sdm:CrossSection)
].
sdm:CrossSection rdf:type skos:Concept;
    skos:inScheme sdm:Type;
    rdfs:label "CrossSection".
sdm:attachedTo dcterms:description "Relationship. A relationship to the ID of the channel where the cross-section 'lives in'. Reference to an entity of type Channel.";
    rdf:type rdf:Property;
    rdfs:label "attachedTo";
    rdfs:domain <https://smart-data-models.github.io/data-models.OpenChannelManagement/CrossSection/schema.json>.
sdm:observedBy dcterms:description "Relationship. A relationship to the ID of the device that monitors raw-water properties. Model:'https://smart-data-models.github.io/dataModel.Device/device-schema.json'";
    rdf:type rdf:Property;
    rdfs:label "observedBy";
    rdfs:domain <https://smart-data-models.github.io/data-models.OpenChannelManagement/CrossSection/schema.json>.
sdm:position dcterms:description "Property. Object providing information about the distance with the rest of the elements and a relationship with them.";
    rdf:type rdf:Property;
    rdfs:label "position";
    rdfs:domain <https://smart-data-models.github.io/data-models.OpenChannelManagement/CrossSection/schema.json>;
    rdfs:range sdm:Position.
sdm:Position rdf:type rdfs:Class;
    rdfs:label "Position".
sdm:distance dcterms:description "Property. The distance between this Entity and a reference point (e.g., the most upstream point of the system).";
    rdf:type rdf:Property;
    rdfs:label "distance";
    rdfs:domain sdm:Position;
    rdfs:range xsd:decimal.
sdm:refPoint dcterms:description "Relationship. The reference point distance is measured from.";
    rdf:type rdf:Property;
    rdfs:label "refPoint";
    rdfs:domain sdm:Position.
sdm:waterFlow dcterms:description "Property. Water flow at the cross-section.";
    rdf:type rdf:Property;
    rdfs:label "waterFlow";
    rdfs:domain <https://smart-data-models.github.io/data-models.OpenChannelManagement/CrossSection/schema.json>;
    rdfs:range xsd:decimal.
sdm:waterVelocity dcterms:description "Property. Water Velocity at the cross-section.";
    rdf:type rdf:Property;
    rdfs:label "waterVelocity";
    rdfs:domain <https://smart-data-models.github.io/data-models.OpenChannelManagement/CrossSection/schema.json>;
    rdfs:range xsd:decimal.
sdm:waterTemperature dcterms:description "Property. Water temperature at the cross-section.";
    rdf:type rdf:Property;
    rdfs:label "waterTemperature";
    rdfs:domain <https://smart-data-models.github.io/data-models.OpenChannelManagement/CrossSection/schema.json>;
    rdfs:range xsd:decimal.
sdm:turbidity dcterms:description "Property. Water turbidity at the cross-section.";
    rdf:type rdf:Property;
    rdfs:label "turbidity";
    rdfs:domain <https://smart-data-models.github.io/data-models.OpenChannelManagement/CrossSection/schema.json>;
    rdfs:range xsd:decimal.
sdm:specificConductivity dcterms:description "Property. Water conductivity at the cross-section.";
    rdf:type rdf:Property;
    rdfs:label "specificConductivity";
    rdfs:domain <https://smart-data-models.github.io/data-models.OpenChannelManagement/CrossSection/schema.json>;
    rdfs:range xsd:decimal.
sdm:waterLevel dcterms:description "Property. Water level at the cross-section.";
    rdf:type rdf:Property;
    rdfs:label "waterLevel";
    rdfs:domain <https://smart-data-models.github.io/data-models.OpenChannelManagement/CrossSection/schema.json>;
    rdfs:range xsd:decimal.
sdm:energyHead dcterms:description "Property. The total energy head at the cross-section.";
    rdf:type rdf:Property;
    rdfs:label "energyHead";
    rdfs:domain <https://smart-data-models.github.io/data-models.OpenChannelManagement/CrossSection/schema.json>;
    rdfs:range xsd:decimal.
sdm:crossSectionGeometry dcterms:description "Property. The geometry of the cross-section. Enum:'Circular, Trapezoidal'.";
    rdf:type rdf:Property;
    rdfs:label "crossSectionGeometry";
    rdfs:domain <https://smart-data-models.github.io/data-models.OpenChannelManagement/CrossSection/schema.json>.
sdm:CrossSectionGeometry rdf:type skos:ConceptScheme.
sdm:crossSectionGeometry rdfs:range [
  owl:oneOf (sdm:Circular sdm:Trapezoidal)
].
sdm:Circular rdf:type skos:Concept;
    skos:inScheme sdm:CrossSectionGeometry;
    rdfs:label "Circular".
sdm:Trapezoidal rdf:type skos:Concept;
    skos:inScheme sdm:CrossSectionGeometry;
    rdfs:label "Trapezoidal".
sdm:bottomSlope dcterms:description "Property. The bottom slope of the channel where the cross-section 'lives in'. All units are accepted in CEFACT code.";
    rdf:type rdf:Property;
    rdfs:label "bottomSlope";
    rdfs:domain <https://smart-data-models.github.io/data-models.OpenChannelManagement/CrossSection/schema.json>;
    rdfs:range xsd:decimal.
sdm:leftSideSlope dcterms:description "Property. The slope of the left bank of the cross-section (for 'Trapezoidal' geometry). All units are accepted in CEFACT code.";
    rdf:type rdf:Property;
    rdfs:label "leftSideSlope";
    rdfs:domain <https://smart-data-models.github.io/data-models.OpenChannelManagement/CrossSection/schema.json>;
    rdfs:range xsd:decimal.
sdm:rightSideSlope dcterms:description "Property. The slope of the right bank of the cross-section (for 'Trapezoidal' geometry). All units are accepted in CEFACT code.";
    rdf:type rdf:Property;
    rdfs:label "rightSideSlope";
    rdfs:domain <https://smart-data-models.github.io/data-models.OpenChannelManagement/CrossSection/schema.json>;
    rdfs:range xsd:decimal.
sdm:bottomWidth dcterms:description "Property. The bottom width of the cross-section (for 'Trapezoidal' geometry). All units are accepted in CEFACT code.";
    rdf:type rdf:Property;
    rdfs:label "bottomWidth";
    rdfs:domain <https://smart-data-models.github.io/data-models.OpenChannelManagement/CrossSection/schema.json>;
    rdfs:range xsd:decimal.
sdm:diameter dcterms:description "Property. The diameter of a circular cross-section.";
    rdf:type rdf:Property;
    rdfs:label "diameter";
    rdfs:domain <https://smart-data-models.github.io/data-models.OpenChannelManagement/CrossSection/schema.json>;
    rdfs:range xsd:decimal.
sdm:maxWaterDepth dcterms:description "Property. The maximum allowable water depth at the cross-section. All units are accepted in CEFACT code.";
    rdf:type rdf:Property;
    rdfs:label "maxWaterDepth";
    rdfs:domain <https://smart-data-models.github.io/data-models.OpenChannelManagement/CrossSection/schema.json>;
    rdfs:range xsd:decimal.
sdm:inheritsFrom dcterms:description "Relationship. URI of a Channel component from which the value of a property is obtained.";
    rdf:type rdf:Property;
    rdfs:label "inheritsFrom";
    rdfs:domain <https://smart-data-models.github.io/data-models.OpenChannelManagement/CrossSection/schema.json>.
