@prefix schema: <https://schema.org/>.
@prefix skos: <http://www.w3.org/2004/02/skos/core#>.
@prefix rdf: <http://www.w3.org/1999/02/22-rdf-syntax-ns#>.
@prefix rdfs: <http://www.w3.org/2000/01/rdf-schema#>.
@prefix foaf: <http://xmlns.com/foaf/0.1/>.
@prefix xsd: <http://www.w3.org/2001/XMLSchema#>.
@prefix dcterms: <http://purl.org/dc/terms/>.
@prefix owl: <http://www.w3.org/2002/07/owl#>.
@prefix jsonsc: <https://www.w3.org/2019/wot/json-schema#>.
@prefix jsonsc-ld: <http://w3id.org/jsonsc-ld/>.
@prefix api: <http://purl.org/linked-data/api/vocab>.
@prefix geo: <http://www.w3.org/2003/01/geo/wgs84_pos#>.
@prefix mobivoc: <http://schema.mobivoc.org/#>.
@prefix geosparql: <http://www.opengis.net/ont/geosparql#>.
@prefix sdm: <https://w3id.org/sdm#>.

<https://smart-data-models.github.io/dataModels.CIMEnergyClasses/VAdjIEEE/schema.json> dcterms:title " Smart Data Models - VAdjIEEE";
    dcterms:description "Adapted from CIM data models. The class represents IEEE Voltage Adjuster which is used to represent the voltage adjuster in either a power factor or var control system.  Reference: IEEE Standard 421.5-2005 Section 11.1.".
sdm:type dcterms:description "Property. NGSI type. It has to be VAdjIEEE";
    rdf:type rdf:Property;
    rdfs:label "type";
    rdfs:domain <https://smart-data-models.github.io/dataModels.CIMEnergyClasses/VAdjIEEE/schema.json>.
sdm:Type rdf:type skos:ConceptScheme.
sdm:type rdfs:range [
  owl:oneOf (sdm:VAdjIEEE)
].
sdm:VAdjIEEE rdf:type skos:Concept;
    skos:inScheme sdm:Type;
    rdfs:label "VAdjIEEE".
sdm:adjslew dcterms:description "Property. Model:'https://schema.org/Number'. Rate at which output of adjuster changes ().  Unit = sec./PU.  Typical Value = 300. Default: 0.0";
    rdf:type rdf:Property;
    rdfs:label "adjslew";
    rdfs:domain <https://smart-data-models.github.io/dataModels.CIMEnergyClasses/VAdjIEEE/schema.json>;
    rdfs:range xsd:decimal.
sdm:taoff dcterms:description "Property. Model:'https://schema.org/Number'. Time that adjuster pulses are off ().  Typical Value = 0.5. Default: 0";
    rdf:type rdf:Property;
    rdfs:label "taoff";
    rdfs:domain <https://smart-data-models.github.io/dataModels.CIMEnergyClasses/VAdjIEEE/schema.json>;
    rdfs:range xsd:decimal.
sdm:taon dcterms:description "Property. Model:'https://schema.org/Number'. Time that adjuster pulses are on ().  Typical Value = 0.1. Default: 0";
    rdf:type rdf:Property;
    rdfs:label "taon";
    rdfs:domain <https://smart-data-models.github.io/dataModels.CIMEnergyClasses/VAdjIEEE/schema.json>;
    rdfs:range xsd:decimal.
sdm:vadjf dcterms:description "Property. Model:'https://schema.org/Number'. Set high to provide a continuous raise or lower (). Default: 0.0";
    rdf:type rdf:Property;
    rdfs:label "vadjf";
    rdfs:domain <https://smart-data-models.github.io/dataModels.CIMEnergyClasses/VAdjIEEE/schema.json>;
    rdfs:range xsd:decimal.
sdm:vadjmax dcterms:description "Property. Model:'https://schema.org/Number'. Maximum output of the adjuster ().  Typical Value = 1.1. Default: 0.0";
    rdf:type rdf:Property;
    rdfs:label "vadjmax";
    rdfs:domain <https://smart-data-models.github.io/dataModels.CIMEnergyClasses/VAdjIEEE/schema.json>;
    rdfs:range xsd:decimal.
sdm:vadjmin dcterms:description "Property. Model:'https://schema.org/Number'. Minimum output of the adjuster ().  Typical Value = 0.9. Default: 0.0";
    rdf:type rdf:Property;
    rdfs:label "vadjmin";
    rdfs:domain <https://smart-data-models.github.io/dataModels.CIMEnergyClasses/VAdjIEEE/schema.json>;
    rdfs:range xsd:decimal.
