@prefix schema: <https://schema.org/>.
@prefix skos: <http://www.w3.org/2004/02/skos/core#>.
@prefix rdf: <http://www.w3.org/1999/02/22-rdf-syntax-ns#>.
@prefix rdfs: <http://www.w3.org/2000/01/rdf-schema#>.
@prefix foaf: <http://xmlns.com/foaf/0.1/>.
@prefix xsd: <http://www.w3.org/2001/XMLSchema#>.
@prefix dcterms: <http://purl.org/dc/terms/>.
@prefix owl: <http://www.w3.org/2002/07/owl#>.
@prefix jsonsc: <https://www.w3.org/2019/wot/json-schema#>.
@prefix jsonsc-ld: <http://w3id.org/jsonsc-ld/>.
@prefix api: <http://purl.org/linked-data/api/vocab>.
@prefix geo: <http://www.w3.org/2003/01/geo/wgs84_pos#>.
@prefix mobivoc: <http://schema.mobivoc.org/#>.
@prefix geosparql: <http://www.opengis.net/ont/geosparql#>.
@prefix sdm: <https://w3id.org/sdm#>.

<https://smart-data-models.github.io/dataModels.CIMEnergyClasses/PhaseTapChangerNonLinear/schema.json> dcterms:title " Smart Data Models - PhaseTapChangerNonLinear";
    dcterms:description "Adapted from CIM data models. The non-linear phase tap changer describes the non-linear behavior of a phase tap changer. This is a base class for the symmetrical and asymmetrical phase tap changer models. The details of these models can be found in the IEC 61970-301 document.".
sdm:type dcterms:description "Property. NGSI type. It has to be PhaseTapChangerNonLinear";
    rdf:type rdf:Property;
    rdfs:label "type";
    rdfs:domain <https://smart-data-models.github.io/dataModels.CIMEnergyClasses/PhaseTapChangerNonLinear/schema.json>.
sdm:Type rdf:type skos:ConceptScheme.
sdm:type rdfs:range [
  owl:oneOf (sdm:PhaseTapChangerNonLinear)
].
sdm:PhaseTapChangerNonLinear rdf:type skos:Concept;
    skos:inScheme sdm:Type;
    rdfs:label "PhaseTapChangerNonLinear".
sdm:voltageStepIncrement dcterms:description "Property. Model:'https://schema.org/Number'. The voltage step increment on the out of phase winding specified in percent of nominal voltage of the transformer end. Default: 0.0";
    rdf:type rdf:Property;
    rdfs:label "voltageStepIncrement";
    rdfs:domain <https://smart-data-models.github.io/dataModels.CIMEnergyClasses/PhaseTapChangerNonLinear/schema.json>;
    rdfs:range xsd:decimal.
sdm:xMax dcterms:description "Property. Model:'https://schema.org/Number'. The reactance depend on the tap position according to a `u` shaped curve. The maximum reactance (xMax) appear at the low and high tap positions. Default: 0.0";
    rdf:type rdf:Property;
    rdfs:label "xMax";
    rdfs:domain <https://smart-data-models.github.io/dataModels.CIMEnergyClasses/PhaseTapChangerNonLinear/schema.json>;
    rdfs:range xsd:decimal.
sdm:xMin dcterms:description "Property. Model:'https://schema.org/Number'. The reactance depend on the tap position according to a `u` shaped curve. The minimum reactance (xMin) appear at the mid tap position. Default: 0.0";
    rdf:type rdf:Property;
    rdfs:label "xMin";
    rdfs:domain <https://smart-data-models.github.io/dataModels.CIMEnergyClasses/PhaseTapChangerNonLinear/schema.json>;
    rdfs:range xsd:decimal.
