@prefix schema: <https://schema.org/>.
@prefix skos: <http://www.w3.org/2004/02/skos/core#>.
@prefix rdf: <http://www.w3.org/1999/02/22-rdf-syntax-ns#>.
@prefix rdfs: <http://www.w3.org/2000/01/rdf-schema#>.
@prefix foaf: <http://xmlns.com/foaf/0.1/>.
@prefix xsd: <http://www.w3.org/2001/XMLSchema#>.
@prefix dcterms: <http://purl.org/dc/terms/>.
@prefix owl: <http://www.w3.org/2002/07/owl#>.
@prefix jsonsc: <https://www.w3.org/2019/wot/json-schema#>.
@prefix jsonsc-ld: <http://w3id.org/jsonsc-ld/>.
@prefix api: <http://purl.org/linked-data/api/vocab>.
@prefix geo: <http://www.w3.org/2003/01/geo/wgs84_pos#>.
@prefix mobivoc: <http://schema.mobivoc.org/#>.
@prefix geosparql: <http://www.opengis.net/ont/geosparql#>.
@prefix sdm: <https://w3id.org/sdm#>.

<https://smart-data-models.github.io/data-model.WaterNetworkManagementEPANET/Simulation/schema.json> dcterms:title "WaterNetwork - SimulationScenario";
    dcterms:description "This entity contains a harmonised description of a generic simulation scenario made for the Water Network Management domain. This entity is primarily associated with the water network management vertical and related IoT applications.".
sdm:type dcterms:description "Property. NGSI-LD Entity Type. It has to be SimulationScenario";
    rdf:type rdf:Property;
    rdfs:label "type";
    rdfs:domain <https://smart-data-models.github.io/data-model.WaterNetworkManagementEPANET/Simulation/schema.json>.
sdm:Type rdf:type skos:ConceptScheme.
sdm:type rdfs:range [
  owl:oneOf (sdm:SimulationScenario)
].
sdm:SimulationScenario rdf:type skos:Concept;
    skos:inScheme sdm:Type;
    rdfs:label "SimulationScenario".
sdm:createdBy dcterms:description "Relationship. The ID of who created/triggered the simulation. Reference to an entity of type 'User'. Model:'https://schema.org/URL'";
    rdf:type rdf:Property;
    rdfs:label "createdBy";
    rdfs:domain <https://smart-data-models.github.io/data-model.WaterNetworkManagementEPANET/Simulation/schema.json>.
sdm:hasInputNetwork dcterms:description "Relationship. The ID of the network used in the simulation. Model:'https://schema.org/URL'";
    rdf:type rdf:Property;
    rdfs:label "hasInputNetwork";
    rdfs:domain <https://smart-data-models.github.io/data-model.WaterNetworkManagementEPANET/Simulation/schema.json>.
sdm:hasSimulationResult dcterms:description "Relationship. The ID of the related simulation result. Reference to an entity of type 'SimulationResult'. Model:'https://schema.org/URL'";
    rdf:type rdf:Property;
    rdfs:label "hasSimulationResult";
    rdfs:domain <https://smart-data-models.github.io/data-model.WaterNetworkManagementEPANET/Simulation/schema.json>.
sdm:qualityTimeStep dcterms:description "Property. Model:'https://schema.org/Number'. The timestep used to track changes in water quality in the network. Given in seconds. Units:'seconds'";
    rdf:type rdf:Property;
    rdfs:label "qualityTimeStep";
    rdfs:domain <https://smart-data-models.github.io/data-model.WaterNetworkManagementEPANET/Simulation/schema.json>;
    rdfs:range xsd:decimal.
sdm:duration dcterms:description "Property. Model:'https://schema.org/Number'. Duration of the simulation, given in seconds. Units:'seconds'";
    rdf:type rdf:Property;
    rdfs:label "duration";
    rdfs:domain <https://smart-data-models.github.io/data-model.WaterNetworkManagementEPANET/Simulation/schema.json>;
    rdfs:range xsd:decimal.
sdm:hydraulicTimeStep dcterms:description "Property. Model:'https://schema.org/Number'. Determines how often the hydraulic state of the network is calculated. Given in seconds. Units:'seconds'";
    rdf:type rdf:Property;
    rdfs:label "hydraulicTimeStep";
    rdfs:domain <https://smart-data-models.github.io/data-model.WaterNetworkManagementEPANET/Simulation/schema.json>;
    rdfs:range xsd:decimal.
sdm:patternStep dcterms:description "Property. Model:'https://schema.org/Number'. Pattern step of the simulation.";
    rdf:type rdf:Property;
    rdfs:label "patternStep";
    rdfs:domain <https://smart-data-models.github.io/data-model.WaterNetworkManagementEPANET/Simulation/schema.json>;
    rdfs:range xsd:decimal.
sdm:patternStart dcterms:description "Property. Model:'https://schema.org/DateTime'. Start time of the  the simulation.";
    rdf:type rdf:Property;
    rdfs:label "patternStart";
    rdfs:domain <https://smart-data-models.github.io/data-model.WaterNetworkManagementEPANET/Simulation/schema.json>;
    rdfs:range xsd:dateTime.
sdm:reportStep dcterms:description "Property. Model:'https://schema.org/Number'. Interval at which output results are reported. given in seconds. Units:'seconds'";
    rdf:type rdf:Property;
    rdfs:label "reportStep";
    rdfs:domain <https://smart-data-models.github.io/data-model.WaterNetworkManagementEPANET/Simulation/schema.json>;
    rdfs:range xsd:decimal.
sdm:reportStart dcterms:description "Property. Model:'https://schema.org/Number'. Simulation time at which results start to be reported. Given in seconds from start of simulation. Units:'seconds'";
    rdf:type rdf:Property;
    rdfs:label "reportStart";
    rdfs:domain <https://smart-data-models.github.io/data-model.WaterNetworkManagementEPANET/Simulation/schema.json>;
    rdfs:range xsd:decimal.
sdm:ruleTimeStep dcterms:description "Property. Model:'https://schema.org/Number'. Time step used to check for changes in system status due to rule-based controls. Given in seconds. Units:'seconds'";
    rdf:type rdf:Property;
    rdfs:label "ruleTimeStep";
    rdfs:domain <https://smart-data-models.github.io/data-model.WaterNetworkManagementEPANET/Simulation/schema.json>;
    rdfs:range xsd:decimal.
sdm:startClockTime dcterms:description "Property. Model:'https://schema.org/Number'. Time of day at which the simulation begins. Given as seconds from start of day. Units:'seconds'";
    rdf:type rdf:Property;
    rdfs:label "startClockTime";
    rdfs:domain <https://smart-data-models.github.io/data-model.WaterNetworkManagementEPANET/Simulation/schema.json>;
    rdfs:range xsd:decimal.
sdm:statistic dcterms:description "Property. Model:'https://schema.org/string'. The type of statistical post-processing that is done on the time series of simulation results generated. Options are AVERAGED (report time-averaged results), MINIMUM (report only minimum values), MAXIMUM (report only maximum values), RANGE (report difference between minimum and maximum values) and NONE (report full time series). Enum:'averaged, minimum, maximum, range, none'";
    rdf:type rdf:Property;
    rdfs:label "statistic";
    rdfs:domain <https://smart-data-models.github.io/data-model.WaterNetworkManagementEPANET/Simulation/schema.json>.
sdm:Statistic rdf:type skos:ConceptScheme.
sdm:statistic rdfs:range [
  owl:oneOf (sdm:averaged sdm:maximum sdm:minimum sdm:none sdm:range)
].
sdm:averaged rdf:type skos:Concept;
    skos:inScheme sdm:Statistic;
    rdfs:label "averaged".
sdm:maximum rdf:type skos:Concept;
    skos:inScheme sdm:Statistic;
    rdfs:label "maximum".
sdm:minimum rdf:type skos:Concept;
    skos:inScheme sdm:Statistic;
    rdfs:label "minimum".
sdm:none rdf:type skos:Concept;
    skos:inScheme sdm:Statistic;
    rdfs:label "none".
sdm:range rdf:type skos:Concept;
    skos:inScheme sdm:Statistic;
    rdfs:label "range".
sdm:trials dcterms:description "Property. Model:'https://schema.org/Number'. The maximum number of trials used to solve network hydraulics at each hydraulic time step of a simulation";
    rdf:type rdf:Property;
    rdfs:label "trials";
    rdfs:domain <https://smart-data-models.github.io/data-model.WaterNetworkManagementEPANET/Simulation/schema.json>;
    rdfs:range xsd:decimal.
sdm:accuracy dcterms:description "Property. Model:'https://schema.org/Number'. Total normalized flow change convergence criterion for determining when a hydraulic solution has been reached.";
    rdf:type rdf:Property;
    rdfs:label "accuracy";
    rdfs:domain <https://smart-data-models.github.io/data-model.WaterNetworkManagementEPANET/Simulation/schema.json>;
    rdfs:range xsd:decimal.
sdm:tolerance dcterms:description "Property. Model:'https://schema.org/Number'. Water quality tolerance";
    rdf:type rdf:Property;
    rdfs:label "tolerance";
    rdfs:domain <https://smart-data-models.github.io/data-model.WaterNetworkManagementEPANET/Simulation/schema.json>;
    rdfs:range xsd:decimal.
sdm:emitterExponent dcterms:description "Property. Model:'https://schema.org/Number'. Power to which pressure at a junction is raised when computing from an emitter.";
    rdf:type rdf:Property;
    rdfs:label "emitterExponent";
    rdfs:domain <https://smart-data-models.github.io/data-model.WaterNetworkManagementEPANET/Simulation/schema.json>;
    rdfs:range xsd:decimal.
sdm:headError dcterms:description "Property. Model:'https://schema.org/Number'. Maximum headloss convergence criterion for determining when a hydraulic solution has been reached.";
    rdf:type rdf:Property;
    rdfs:label "headError";
    rdfs:domain <https://smart-data-models.github.io/data-model.WaterNetworkManagementEPANET/Simulation/schema.json>;
    rdfs:range xsd:decimal.
sdm:flowChange dcterms:description "Property. Model:'https://schema.org/Number'. Maximum flow change convergence criterion for determining when a hydraulic solution has been reached.";
    rdf:type rdf:Property;
    rdfs:label "flowChange";
    rdfs:domain <https://smart-data-models.github.io/data-model.WaterNetworkManagementEPANET/Simulation/schema.json>;
    rdfs:range xsd:decimal.
sdm:demandCharge dcterms:description "Property. Model:'https://schema.org/Number'. Energy charge per maximum kW usage.";
    rdf:type rdf:Property;
    rdfs:label "demandCharge";
    rdfs:domain <https://smart-data-models.github.io/data-model.WaterNetworkManagementEPANET/Simulation/schema.json>;
    rdfs:range xsd:decimal.
sdm:specificGravity dcterms:description "Property. Model:'https://schema.org/Number'. The ratio of the density of the fluid being modeled to that of water at 4 deg. C";
    rdf:type rdf:Property;
    rdfs:label "specificGravity";
    rdfs:domain <https://smart-data-models.github.io/data-model.WaterNetworkManagementEPANET/Simulation/schema.json>;
    rdfs:range xsd:decimal.
sdm:requiredPressure dcterms:description "Property. Model:'https://schema.org/Number'. Pressure required to supply a node's full demand under a pressure driven analysis. Only used if demandModel is 'PDA'";
    rdf:type rdf:Property;
    rdfs:label "requiredPressure";
    rdfs:domain <https://smart-data-models.github.io/data-model.WaterNetworkManagementEPANET/Simulation/schema.json>;
    rdfs:range xsd:decimal.
sdm:pressureExponent dcterms:description "Property. Model:'https://schema.org/Number'. Power to which pressure is raised when calculating the demand delivered under a pressure driven analysis. Only used if demandModel is 'PDA'";
    rdf:type rdf:Property;
    rdfs:label "pressureExponent";
    rdfs:domain <https://smart-data-models.github.io/data-model.WaterNetworkManagementEPANET/Simulation/schema.json>;
    rdfs:range xsd:decimal.
sdm:viscosity dcterms:description "Property. Model:'https://schema.org/Number'. The kinematic viscosity of the fluid being modeled relative to that of water at 20 deg. C";
    rdf:type rdf:Property;
    rdfs:label "viscosity";
    rdfs:domain <https://smart-data-models.github.io/data-model.WaterNetworkManagementEPANET/Simulation/schema.json>;
    rdfs:range xsd:decimal.
sdm:unbalanced dcterms:description "Property. Model:'https://schema.org/Text'. Determines what happens if a hydraulic solution cannot be reached within the allowed number of trials. Allowable options are STOP (halt analysis), CONTINUE (continue analysis but with a warning message) and CONTINUE_N (continue for another N trials, where the value of N is given by 'unbalancedN'). Enum:'stop, continue, continue_N'";
    rdf:type rdf:Property;
    rdfs:label "unbalanced";
    rdfs:domain <https://smart-data-models.github.io/data-model.WaterNetworkManagementEPANET/Simulation/schema.json>.
sdm:Unbalanced rdf:type skos:ConceptScheme.
sdm:unbalanced rdfs:range [
  owl:oneOf (sdm:stop sdm:continue sdm:continue_N)
].
sdm:stop rdf:type skos:Concept;
    skos:inScheme sdm:Unbalanced;
    rdfs:label "stop".
sdm:continue rdf:type skos:Concept;
    skos:inScheme sdm:Unbalanced;
    rdfs:label "continue".
sdm:continue_N rdf:type skos:Concept;
    skos:inScheme sdm:Unbalanced;
    rdfs:label "continue_N".
sdm:unbalancedN dcterms:description "Property. Model:'https://schema.org/Number'. Number of additional trials allowed if 'unbalanced' is set to continue_N. Mandatory if 'unbalanced' is set to continue_N, else not required.";
    rdf:type rdf:Property;
    rdfs:label "unbalancedN";
    rdfs:domain <https://smart-data-models.github.io/data-model.WaterNetworkManagementEPANET/Simulation/schema.json>;
    rdfs:range xsd:decimal.
sdm:checkFrequency dcterms:description "Property. Model:'https://schema.org/Number'. Frequency of hydraulic status checks";
    rdf:type rdf:Property;
    rdfs:label "checkFrequency";
    rdfs:domain <https://smart-data-models.github.io/data-model.WaterNetworkManagementEPANET/Simulation/schema.json>;
    rdfs:range xsd:decimal.
sdm:maxCheck dcterms:description "Property. Model:'https://schema.org/Number'. Number of trials after which status checks are discontinued";
    rdf:type rdf:Property;
    rdfs:label "maxCheck";
    rdfs:domain <https://smart-data-models.github.io/data-model.WaterNetworkManagementEPANET/Simulation/schema.json>;
    rdfs:range xsd:decimal.
sdm:dampLimit dcterms:description "Property. Model:'https://schema.org/Number'. Accuracy value at which solution damping and status checks begin for PRVs and PSVs.";
    rdf:type rdf:Property;
    rdfs:label "dampLimit";
    rdfs:domain <https://smart-data-models.github.io/data-model.WaterNetworkManagementEPANET/Simulation/schema.json>;
    rdfs:range xsd:decimal.
sdm:diffusivity dcterms:description "Property. Model:'https://schema.org/Number'. Molecular diffusivity of the chemical analysed in a quality analysis, relative to diffusivity of chlorine in water.";
    rdf:type rdf:Property;
    rdfs:label "diffusivity";
    rdfs:domain <https://smart-data-models.github.io/data-model.WaterNetworkManagementEPANET/Simulation/schema.json>;
    rdfs:range xsd:decimal.
sdm:bulkOrder dcterms:description "Property. Model:'https://schema.org/Number'. Bulk water reaction order for pipes";
    rdf:type rdf:Property;
    rdfs:label "bulkOrder";
    rdfs:domain <https://smart-data-models.github.io/data-model.WaterNetworkManagementEPANET/Simulation/schema.json>;
    rdfs:range xsd:decimal.
sdm:wallOrder dcterms:description "Property. Model:'https://schema.org/Number'. Wall reaction order for pipes";
    rdf:type rdf:Property;
    rdfs:label "wallOrder";
    rdfs:domain <https://smart-data-models.github.io/data-model.WaterNetworkManagementEPANET/Simulation/schema.json>;
    rdfs:range xsd:decimal.
sdm:tankOrder dcterms:description "Property. Model:'https://schema.org/Number'. Bulk water reaction order for tanks";
    rdf:type rdf:Property;
    rdfs:label "tankOrder";
    rdfs:domain <https://smart-data-models.github.io/data-model.WaterNetworkManagementEPANET/Simulation/schema.json>;
    rdfs:range xsd:decimal.
sdm:concentrationLimit dcterms:description "Property. Model:'https://schema.org/Number'. Limiting concentration for growth reactions";
    rdf:type rdf:Property;
    rdfs:label "concentrationLimit";
    rdfs:domain <https://smart-data-models.github.io/data-model.WaterNetworkManagementEPANET/Simulation/schema.json>;
    rdfs:range xsd:decimal.
sdm:qualityType dcterms:description "Property. Model:'https://schema.org/Text'. Type of water quality analysis. Enum:'chem, age, trace, none'";
    rdf:type rdf:Property;
    rdfs:label "qualityType";
    rdfs:domain <https://smart-data-models.github.io/data-model.WaterNetworkManagementEPANET/Simulation/schema.json>.
sdm:QualityType rdf:type skos:ConceptScheme.
sdm:qualityType rdfs:range [
  owl:oneOf (sdm:age sdm:chem sdm:none sdm:trace)
].
sdm:age rdf:type skos:Concept;
    skos:inScheme sdm:QualityType;
    rdfs:label "age".
sdm:chem rdf:type skos:Concept;
    skos:inScheme sdm:QualityType;
    rdfs:label "chem".
sdm:none rdf:type skos:Concept;
    skos:inScheme sdm:QualityType;
    rdfs:label "none".
sdm:trace rdf:type skos:Concept;
    skos:inScheme sdm:QualityType;
    rdfs:label "trace".
sdm:chemicalName dcterms:description "Property. Model:'https://schema.org/Text'. Name of the chemical modelled. Only used if 'qualityType' is CHEM";
    rdf:type rdf:Property;
    rdfs:label "chemicalName";
    rdfs:domain <https://smart-data-models.github.io/data-model.WaterNetworkManagementEPANET/Simulation/schema.json>;
    rdfs:range xsd:string.
sdm:chemicalUnits dcterms:description "Property. Model:'https://schema.org/Text'. Units of the chemical modelled. Only used if 'qualityType' is CHEM";
    rdf:type rdf:Property;
    rdfs:label "chemicalUnits";
    rdfs:domain <https://smart-data-models.github.io/data-model.WaterNetworkManagementEPANET/Simulation/schema.json>;
    rdfs:range xsd:string.
sdm:traceNodeID dcterms:description "Relationship. URI of node being traced in the quality analysis. Mandatory if 'qualityType' is TRACE, otherwise not required. Model:'https://schema.org/URL'";
    rdf:type rdf:Property;
    rdfs:label "traceNodeID";
    rdfs:domain <https://smart-data-models.github.io/data-model.WaterNetworkManagementEPANET/Simulation/schema.json>.
sdm:flowUnits dcterms:description "Property. Model:'https://schema.org/Text'. Units in which flow rates are expressed in the simulation. Allowable options are CFS (cubic feet per second), GPM (gallons per minute), MGD (million gallons per day), IMGD (imperial MGD), AFD (acre-feet per day), LPS (litres pre second), LPM (litres per minute), MLD (million litres per day), CMH (cubic metres per hour) and CMD (cubic metres per day). Enum:'AFD, CFS, CMD, CMH, GPM, IMGD, LPS, LPM, MLD, MGD'";
    rdf:type rdf:Property;
    rdfs:label "flowUnits";
    rdfs:domain <https://smart-data-models.github.io/data-model.WaterNetworkManagementEPANET/Simulation/schema.json>.
sdm:FlowUnits rdf:type skos:ConceptScheme.
sdm:flowUnits rdfs:range [
  owl:oneOf (sdm:AFD sdm:CFS sdm:CMD sdm:CMH sdm:GPM sdm:IMGD sdm:LPS sdm:LPM sdm:MLD sdm:MGD)
].
sdm:AFD rdf:type skos:Concept;
    skos:inScheme sdm:FlowUnits;
    rdfs:label "AFD".
sdm:CFS rdf:type skos:Concept;
    skos:inScheme sdm:FlowUnits;
    rdfs:label "CFS".
sdm:CMD rdf:type skos:Concept;
    skos:inScheme sdm:FlowUnits;
    rdfs:label "CMD".
sdm:CMH rdf:type skos:Concept;
    skos:inScheme sdm:FlowUnits;
    rdfs:label "CMH".
sdm:GPM rdf:type skos:Concept;
    skos:inScheme sdm:FlowUnits;
    rdfs:label "GPM".
sdm:IMGD rdf:type skos:Concept;
    skos:inScheme sdm:FlowUnits;
    rdfs:label "IMGD".
sdm:LPS rdf:type skos:Concept;
    skos:inScheme sdm:FlowUnits;
    rdfs:label "LPS".
sdm:LPM rdf:type skos:Concept;
    skos:inScheme sdm:FlowUnits;
    rdfs:label "LPM".
sdm:MLD rdf:type skos:Concept;
    skos:inScheme sdm:FlowUnits;
    rdfs:label "MLD".
sdm:MGD rdf:type skos:Concept;
    skos:inScheme sdm:FlowUnits;
    rdfs:label "MGD".
sdm:headlossFormula dcterms:description "Property. Model:'https://schema.org/Text'. Formula used for computing head loss for flow through a pipe. The choices are the Hazen-Williams (H-W), Darcy-Weisbach (D-W) or Chezy-Manning (C-M) formulas. Allowable options are 'H-W', 'D-W', 'C-M'. Enum:'C-M, D-W, H-W'";
    rdf:type rdf:Property;
    rdfs:label "headlossFormula";
    rdfs:domain <https://smart-data-models.github.io/data-model.WaterNetworkManagementEPANET/Simulation/schema.json>.
sdm:HeadlossFormula rdf:type skos:ConceptScheme.
sdm:headlossFormula rdfs:range [
  owl:oneOf (sdm:H-W sdm:D-W sdm:C-M)
].
sdm:H-W rdf:type skos:Concept;
    skos:inScheme sdm:HeadlossFormula;
    rdfs:label "H-W".
sdm:D-W rdf:type skos:Concept;
    skos:inScheme sdm:HeadlossFormula;
    rdfs:label "D-W".
sdm:C-M rdf:type skos:Concept;
    skos:inScheme sdm:HeadlossFormula;
    rdfs:label "C-M".
sdm:demandModel dcterms:description "Property. Model:'https://schema.org/Text'. Specifies whether the analysis is pressure driven (PDA) or demand driven (DDA). Enum:'DDA, PDA'";
    rdf:type rdf:Property;
    rdfs:label "demandModel";
    rdfs:domain <https://smart-data-models.github.io/data-model.WaterNetworkManagementEPANET/Simulation/schema.json>.
sdm:DemandModel rdf:type skos:ConceptScheme.
sdm:demandModel rdfs:range [
  owl:oneOf (sdm:DDA sdm:PDA)
].
sdm:DDA rdf:type skos:Concept;
    skos:inScheme sdm:DemandModel;
    rdfs:label "DDA".
sdm:PDA rdf:type skos:Concept;
    skos:inScheme sdm:DemandModel;
    rdfs:label "PDA".
sdm:minimumPressure dcterms:description "Property. Model:'https://schema.org/Number'. Pressure below which no demand can be delivered under a pressure dirven analysis. Only used if demandModel is 'PDA'";
    rdf:type rdf:Property;
    rdfs:label "minimumPressure";
    rdfs:domain <https://smart-data-models.github.io/data-model.WaterNetworkManagementEPANET/Simulation/schema.json>;
    rdfs:range xsd:decimal.
sdm:operationalControl dcterms:description "Property. The operational control of de item";
    rdf:type rdf:Property;
    rdfs:label "operationalControl";
    rdfs:domain <https://smart-data-models.github.io/data-model.WaterNetworkManagementEPANET/Simulation/schema.json>;
    rdfs:range sdm:OperationalControl.
sdm:OperationalControl rdf:type rdfs:Class;
    rdfs:label "OperationalControl".
sdm:type dcterms:description "Property. Model:'https://schema.org/Text'. Description of a control applied to the network for the simulation. Enum:'controlledLink, controlType, monitoredNode, setting, triggerLevel'";
    rdf:type rdf:Property;
    rdfs:label "type";
    rdfs:domain sdm:OperationalControl;
    rdfs:range xsd:string.
sdm:triggerLevel dcterms:description "Property. Model:'https://schema.org/Number'. Level at which control is activated. A sub-property of the Property 'control'";
    rdf:type rdf:Property;
    rdfs:label "triggerLevel";
    rdfs:domain sdm:OperationalControl;
    rdfs:range xsd:decimal.
sdm:setting dcterms:description "Property. Model:'https://schema.org/Number'. Setting applied in the to the controlled link when trigger level is reached. A sub-property of the Property 'control'";
    rdf:type rdf:Property;
    rdfs:label "setting";
    rdfs:domain sdm:OperationalControl;
    rdfs:range xsd:decimal.
sdm:controlType dcterms:description "Property. Model:'https://schema.org/Text'. Type of trigger for the control. A sub-property of the Property 'control'. Enum:'HILEVEL, LOWLEVEL, TIMEOFDAY, TIMER'";
    rdf:type rdf:Property;
    rdfs:label "controlType";
    rdfs:domain sdm:OperationalControl.
sdm:ControlType rdf:type skos:ConceptScheme.
sdm:controlType rdfs:range [
  owl:oneOf (sdm:HILEVEL sdm:LOWLEVEL sdm:TIMEOFDAY sdm:TIMER)
].
sdm:HILEVEL rdf:type skos:Concept;
    skos:inScheme sdm:ControlType;
    rdfs:label "HILEVEL".
sdm:LOWLEVEL rdf:type skos:Concept;
    skos:inScheme sdm:ControlType;
    rdfs:label "LOWLEVEL".
sdm:TIMEOFDAY rdf:type skos:Concept;
    skos:inScheme sdm:ControlType;
    rdfs:label "TIMEOFDAY".
sdm:TIMER rdf:type skos:Concept;
    skos:inScheme sdm:ControlType;
    rdfs:label "TIMER".
sdm:controlledLink dcterms:description "Relationship. Model:'https://schema.org/URL'. Link controlled. A sub-relationship of the Property 'control'. Reference to an entity of type 'Pipe', 'Pump' or 'Valve'";
    rdf:type rdf:Property;
    rdfs:label "controlledLink";
    rdfs:domain sdm:OperationalControl.
sdm:monitoredNode dcterms:description "Relationship. Model:'https://schema.org/URL'. Node which is monitored for control trigger level. A sub-relationship of the Property 'control'.  Reference to an entity of type 'Junction', 'Tank' or 'Reservoir'";
    rdf:type rdf:Property;
    rdfs:label "monitoredNode";
    rdfs:domain sdm:OperationalControl.
sdm:inputParameter dcterms:description "Property. Model:'https://Text'. Description of the set of modifications to be applied to the network for the simulation";
    rdf:type rdf:Property;
    rdfs:label "inputParameter";
    rdfs:domain <https://smart-data-models.github.io/data-model.WaterNetworkManagementEPANET/Simulation/schema.json>;
    rdfs:range sdm:InputParameter.
sdm:InputParameter rdf:type rdfs:Class;
    rdfs:label "InputParameter".
sdm:parameterName rdf:type rdf:Property;
    rdfs:label "parameterName";
    rdfs:domain sdm:InputParameter;
    rdfs:range xsd:string.
sdm:value rdf:type rdf:Property;
    rdfs:label "value";
    rdfs:domain sdm:InputParameter.
sdm:targetURI dcterms:description "Relationship. Model:'https://schema.org/URL'. URI of network component with property modified in simulation. A sub-relationship of the Property water attribute.";
    rdf:type rdf:Property;
    rdfs:label "targetURI";
    rdfs:domain sdm:InputParameter.
