@prefix schema: <https://schema.org/>.
@prefix skos: <http://www.w3.org/2004/02/skos/core#>.
@prefix rdf: <http://www.w3.org/1999/02/22-rdf-syntax-ns#>.
@prefix rdfs: <http://www.w3.org/2000/01/rdf-schema#>.
@prefix foaf: <http://xmlns.com/foaf/0.1/>.
@prefix xsd: <http://www.w3.org/2001/XMLSchema#>.
@prefix dcterms: <http://purl.org/dc/terms/>.
@prefix owl: <http://www.w3.org/2002/07/owl#>.
@prefix jsonsc: <https://www.w3.org/2019/wot/json-schema#>.
@prefix jsonsc-ld: <http://w3id.org/jsonsc-ld/>.
@prefix api: <http://purl.org/linked-data/api/vocab>.
@prefix geo: <http://www.w3.org/2003/01/geo/wgs84_pos#>.
@prefix mobivoc: <http://schema.mobivoc.org/#>.
@prefix geosparql: <http://www.opengis.net/ont/geosparql#>.
@prefix sdm: <https://w3id.org/sdm#>.

<https://smart-data-models.github.io/dataModels.CIMEnergyClasses/PhaseTapChangerAsymmetrical/schema.json> dcterms:title " Smart Data Models - PhaseTapChangerAsymmetrical";
    dcterms:description "Adapted from CIM data models. Describes the tap model for an asymmetrical phase shifting transformer in which the difference voltage vector adds to the primary side voltage. The angle between the primary side voltage and the difference voltage is named the winding connection angle. The phase shift depends on both the difference voltage magnitude and the winding connection angle.".
sdm:type dcterms:description "Property. NGSI type. It has to be PhaseTapChangerAsymmetrical";
    rdf:type rdf:Property;
    rdfs:label "type";
    rdfs:domain <https://smart-data-models.github.io/dataModels.CIMEnergyClasses/PhaseTapChangerAsymmetrical/schema.json>.
sdm:Type rdf:type skos:ConceptScheme.
sdm:type rdfs:range [
  owl:oneOf (sdm:PhaseTapChangerAsymmetrical)
].
sdm:PhaseTapChangerAsymmetrical rdf:type skos:Concept;
    skos:inScheme sdm:Type;
    rdfs:label "PhaseTapChangerAsymmetrical".
sdm:windingConnectionAngle dcterms:description "Property. Model:'https://schema.org/Number'. The phase angle between the in-phase winding and the out-of -phase winding used for creating phase shift. The out-of-phase winding produces what is known as the difference voltage.  Setting this angle to 90 degrees is not the same as a symmemtrical transformer. Default: 0.0";
    rdf:type rdf:Property;
    rdfs:label "windingConnectionAngle";
    rdfs:domain <https://smart-data-models.github.io/dataModels.CIMEnergyClasses/PhaseTapChangerAsymmetrical/schema.json>;
    rdfs:range xsd:decimal.
