@prefix schema: <https://schema.org/>.
@prefix skos: <http://www.w3.org/2004/02/skos/core#>.
@prefix rdf: <http://www.w3.org/1999/02/22-rdf-syntax-ns#>.
@prefix rdfs: <http://www.w3.org/2000/01/rdf-schema#>.
@prefix foaf: <http://xmlns.com/foaf/0.1/>.
@prefix xsd: <http://www.w3.org/2001/XMLSchema#>.
@prefix dcterms: <http://purl.org/dc/terms/>.
@prefix owl: <http://www.w3.org/2002/07/owl#>.
@prefix jsonsc: <https://www.w3.org/2019/wot/json-schema#>.
@prefix jsonsc-ld: <http://w3id.org/jsonsc-ld/>.
@prefix api: <http://purl.org/linked-data/api/vocab>.
@prefix geo: <http://www.w3.org/2003/01/geo/wgs84_pos#>.
@prefix mobivoc: <http://schema.mobivoc.org/#>.
@prefix geosparql: <http://www.opengis.net/ont/geosparql#>.
@prefix sdm: <https://w3id.org/sdm#>.

<https://smart-data-models.github.io/dataModel.Environment/MosquitoDensity/schema.json> dcterms:title "Smart Data Models - Mosquito Density data Model";
    dcterms:description "A Data Model for density of mosquitoes in cities.".
sdm:type dcterms:description "Property. NGSI Entity type. It has to be MosquitoDensity";
    rdf:type rdf:Property;
    rdfs:label "type";
    rdfs:domain <https://smart-data-models.github.io/dataModel.Environment/MosquitoDensity/schema.json>.
sdm:Type rdf:type skos:ConceptScheme.
sdm:type rdfs:range [
  owl:oneOf (sdm:MosquitoDensity)
].
sdm:MosquitoDensity rdf:type skos:Concept;
    skos:inScheme sdm:Type;
    rdfs:label "MosquitoDensity".
sdm:dataDescriptor dcterms:description "Relationship. URI pointing to the data-descriptor entity";
    rdf:type rdf:Property;
    rdfs:label "dataDescriptor";
    rdfs:domain <https://smart-data-models.github.io/dataModel.Environment/MosquitoDensity/schema.json>;
    rdfs:range xsd:anyURI.
sdm:mosquitoDensity dcterms:description "Property. The binomial (or) zoological nomenclature of the mosquito species and its count as identified by the device corresponding to this observation..";
    rdf:type rdf:Property;
    rdfs:label "mosquitoDensity";
    rdfs:domain <https://smart-data-models.github.io/dataModel.Environment/MosquitoDensity/schema.json>;
    rdfs:range sdm:MosquitoDensity.
sdm:MosquitoDensity rdf:type rdfs:Class;
    rdfs:label "MosquitoDensity".
sdm:maleSpeciesCount dcterms:description "Property. The total count of the male mosquitoes of the species identified by the device..";
    rdf:type rdf:Property;
    rdfs:label "maleSpeciesCount";
    rdfs:domain sdm:MosquitoDensity;
    rdfs:range xsd:decimal.
sdm:totalSpeciesCount dcterms:description "Property. The total count of a particular species detected by the device..";
    rdf:type rdf:Property;
    rdfs:label "totalSpeciesCount";
    rdfs:domain sdm:MosquitoDensity;
    rdfs:range xsd:decimal.
sdm:mosquitoSpecies dcterms:description "Property. The binomial/ zoological nomenclature of the mosquito species as identified by the device.";
    rdf:type rdf:Property;
    rdfs:label "mosquitoSpecies";
    rdfs:domain sdm:MosquitoDensity;
    rdfs:range xsd:string.
sdm:femaleSpeciesCount dcterms:description "Property. The total count of the female mosquitoes of the species identified by the device..";
    rdf:type rdf:Property;
    rdfs:label "femaleSpeciesCount";
    rdfs:domain sdm:MosquitoDensity;
    rdfs:range xsd:decimal.
sdm:deviceInfo dcterms:description "Property. Model:'https://schema.org/Text. Information about the device associated with the observations.";
    rdf:type rdf:Property;
    rdfs:label "deviceInfo";
    rdfs:domain <https://smart-data-models.github.io/dataModel.Environment/MosquitoDensity/schema.json>;
    rdfs:range sdm:DeviceInfo.
sdm:DeviceInfo rdf:type rdfs:Class;
    rdfs:label "DeviceInfo".
sdm:rfID dcterms:description "Property. Model:'https://schema.org/Text'. Gives the ID of the RFID reader.";
    rdf:type rdf:Property;
    rdfs:label "rfID";
    rdfs:domain sdm:DeviceInfo;
    rdfs:range xsd:string.
sdm:deviceBatteryStatus dcterms:description "Property. Model:'https://schema.org/Text'. Gives the Battery charging status of the reporting device(Connected, Disconnected).";
    rdf:type rdf:Property;
    rdfs:label "deviceBatteryStatus";
    rdfs:domain sdm:DeviceInfo;
    rdfs:range xsd:string.
sdm:deviceName dcterms:description "Property. Model:'https://schema.org/Text'. Device Name or Station name of the sensor device/station corresponding to this observation.";
    rdf:type rdf:Property;
    rdfs:label "deviceName";
    rdfs:domain sdm:DeviceInfo;
    rdfs:range xsd:string.
sdm:deviceId dcterms:description "Property. Model:'https://schema.org/Text'. Device ID of the physical sensor/ measurement station corresponding to this observation.";
    rdf:type rdf:Property;
    rdfs:label "deviceId";
    rdfs:domain sdm:DeviceInfo;
    rdfs:range xsd:string.
sdm:measurand dcterms:description "Property. Model:'https://schema.org/Text'. Property/properties sensed/observed/measured by the device.";
    rdf:type rdf:Property;
    rdfs:label "measurand";
    rdfs:domain sdm:DeviceInfo;
    rdfs:range xsd:string.
sdm:deviceSimNumber dcterms:description "Property. Model:'https://schema.org/Text'. Gives the sim number of the device in the waste management vehicle.";
    rdf:type rdf:Property;
    rdfs:label "deviceSimNumber";
    rdfs:domain sdm:DeviceInfo;
    rdfs:range xsd:string.
sdm:deviceModel dcterms:description "Property. Model:'https://schema.org/Text'. Describes the information of the device, sensor or system in consideration.";
    rdf:type rdf:Property;
    rdfs:label "deviceModel";
    rdfs:domain sdm:DeviceInfo;
    rdfs:range sdm:DeviceModel.
sdm:DeviceModel rdf:type rdfs:Class;
    rdfs:label "DeviceModel".
sdm:brandName dcterms:description "Property. Model:'https://schema.org/Text'. Name of the brand associated with an entity, e.g., sensor, device etc.";
    rdf:type rdf:Property;
    rdfs:label "brandName";
    rdfs:domain sdm:DeviceModel;
    rdfs:range xsd:string.
sdm:manufacturerName dcterms:description "Property. Model:'https://schema.org/Text'. Name of the manufacturer associated with an entity, e.g., sensor, device etc.";
    rdf:type rdf:Property;
    rdfs:label "manufacturerName";
    rdfs:domain sdm:DeviceModel;
    rdfs:range xsd:string.
sdm:modelName dcterms:description "Property. Model:'https://schema.org/Text'. Name of a specific model associated with an entity, e.g., sensor, device etc.";
    rdf:type rdf:Property;
    rdfs:label "modelName";
    rdfs:domain sdm:DeviceModel;
    rdfs:range xsd:string.
sdm:modelURL dcterms:description "Property. Model:'https://schema.org/Text'. URL providing further information of a specific model associated with an entity, e.g., sensor, device etc.";
    rdf:type rdf:Property;
    rdfs:label "modelURL";
    rdfs:domain sdm:DeviceModel;
    rdfs:range xsd:string.
sdm:observationDateTime dcterms:description "Property. Last reported time of observation.";
    rdf:type rdf:Property;
    rdfs:label "observationDateTime";
    rdfs:domain sdm:DeviceInfo;
    rdfs:range xsd:dateTime.
sdm:airTemperature dcterms:description "Property. Observed value of air temperature. Value is an object containing attributes representing statistical aggregates derived from past data.";
    rdf:type rdf:Property;
    rdfs:label "airTemperature";
    rdfs:domain sdm:DeviceInfo;
    rdfs:range sdm:AirTemperature.
sdm:AirTemperature rdf:type rdfs:Class;
    rdfs:label "AirTemperature".
sdm:precipitation dcterms:description "Property. Observed precipitation/rainfall level over a given duration.";
    rdf:type rdf:Property;
    rdfs:label "precipitation";
    rdfs:domain sdm:DeviceInfo;
    rdfs:range xsd:decimal.
