@prefix schema: <https://schema.org/>.
@prefix skos: <http://www.w3.org/2004/02/skos/core#>.
@prefix rdf: <http://www.w3.org/1999/02/22-rdf-syntax-ns#>.
@prefix rdfs: <http://www.w3.org/2000/01/rdf-schema#>.
@prefix foaf: <http://xmlns.com/foaf/0.1/>.
@prefix xsd: <http://www.w3.org/2001/XMLSchema#>.
@prefix dcterms: <http://purl.org/dc/terms/>.
@prefix owl: <http://www.w3.org/2002/07/owl#>.
@prefix jsonsc: <https://www.w3.org/2019/wot/json-schema#>.
@prefix jsonsc-ld: <http://w3id.org/jsonsc-ld/>.
@prefix api: <http://purl.org/linked-data/api/vocab>.
@prefix geo: <http://www.w3.org/2003/01/geo/wgs84_pos#>.
@prefix mobivoc: <http://schema.mobivoc.org/#>.
@prefix geosparql: <http://www.opengis.net/ont/geosparql#>.
@prefix sdm: <https://w3id.org/sdm#>.

<https://smart-data-models.github.io/dataModel.Aeronautics/AircraftModel/schema.json> dcterms:title "Smart Data models - Aircraft schema";
    dcterms:description "A description of a generic aircraft model".
sdm:type dcterms:description "Property. NGSI Entity type. It has to be AircraftModel";
    rdf:type rdf:Property;
    rdfs:label "type";
    rdfs:domain <https://smart-data-models.github.io/dataModel.Aeronautics/AircraftModel/schema.json>.
sdm:Type rdf:type skos:ConceptScheme.
sdm:type rdfs:range [
  owl:oneOf (sdm:AircraftModel)
].
sdm:AircraftModel rdf:type skos:Concept;
    skos:inScheme sdm:Type;
    rdfs:label "AircraftModel".
sdm:codeIATA dcterms:description "Property. Model:'http://schema.org/Text'. IATA aircraft type";
    rdf:type rdf:Property;
    rdfs:label "codeIATA";
    rdfs:domain <https://smart-data-models.github.io/dataModel.Aeronautics/AircraftModel/schema.json>;
    rdfs:range xsd:string.
sdm:codeICAO dcterms:description "Property. Model:'http://schema.org/Text'. ICAO aircraft type";
    rdf:type rdf:Property;
    rdfs:label "codeICAO";
    rdfs:domain <https://smart-data-models.github.io/dataModel.Aeronautics/AircraftModel/schema.json>;
    rdfs:range xsd:string.
sdm:length dcterms:description "Property. Model:'http://schema.org/Number'. Aircraft model length in metres. Units:'metres'";
    rdf:type rdf:Property;
    rdfs:label "length";
    rdfs:domain <https://smart-data-models.github.io/dataModel.Aeronautics/AircraftModel/schema.json>;
    rdfs:range xsd:decimal.
sdm:wingSpan dcterms:description "Property. Model:'http://schema.org/Number'. Aircraft model wingspan in metres. Units:'metres'";
    rdf:type rdf:Property;
    rdfs:label "wingSpan";
    rdfs:domain <https://smart-data-models.github.io/dataModel.Aeronautics/AircraftModel/schema.json>;
    rdfs:range xsd:decimal.
sdm:height dcterms:description "Property. Model:'http://schema.org/Number'. Aircraft model height in metres. Units:'metres'";
    rdf:type rdf:Property;
    rdfs:label "height";
    rdfs:domain <https://smart-data-models.github.io/dataModel.Aeronautics/AircraftModel/schema.json>;
    rdfs:range xsd:decimal.
sdm:mtow dcterms:description "Property. Model:'http://schema.org/Number'.  Aircraft maximum takeoff weight in kilograms. Units:'kilograms'";
    rdf:type rdf:Property;
    rdfs:label "mtow";
    rdfs:domain <https://smart-data-models.github.io/dataModel.Aeronautics/AircraftModel/schema.json>;
    rdfs:range xsd:decimal.
sdm:maximumAllowedSpeed dcterms:description "Property. Model:'http://schema.org/Number'.  Aircraft maximum speed in kilometers per hour. Units:'kilometers per hour'";
    rdf:type rdf:Property;
    rdfs:label "maximumAllowedSpeed";
    rdfs:domain <https://smart-data-models.github.io/dataModel.Aeronautics/AircraftModel/schema.json>;
    rdfs:range xsd:decimal.
sdm:maximumAllowedFuel dcterms:description "Property. Model:'http://schema.org/Number'. Aircraft maximum fuel in kilograms. Units:'kilograms'";
    rdf:type rdf:Property;
    rdfs:label "maximumAllowedFuel";
    rdfs:domain <https://smart-data-models.github.io/dataModel.Aeronautics/AircraftModel/schema.json>;
    rdfs:range xsd:decimal.
sdm:ceiling dcterms:description "Property. Model:'http://schema.org/Number'. Maximum altitude the aircraft model can reach in metres. Units:'metres'";
    rdf:type rdf:Property;
    rdfs:label "ceiling";
    rdfs:domain <https://smart-data-models.github.io/dataModel.Aeronautics/AircraftModel/schema.json>;
    rdfs:range xsd:decimal.
sdm:numberOfEngines dcterms:description "Property. Model:'http://schema.org/Integer'. Number of engines";
    rdf:type rdf:Property;
    rdfs:label "numberOfEngines";
    rdfs:domain <https://smart-data-models.github.io/dataModel.Aeronautics/AircraftModel/schema.json>;
    rdfs:range xsd:integer.
sdm:capacity dcterms:description "Property. Model:'http://schema.org/Integer'. Number of seatings";
    rdf:type rdf:Property;
    rdfs:label "capacity";
    rdfs:domain <https://smart-data-models.github.io/dataModel.Aeronautics/AircraftModel/schema.json>;
    rdfs:range xsd:integer.
