@prefix schema: <https://schema.org/>.
@prefix skos: <http://www.w3.org/2004/02/skos/core#>.
@prefix rdf: <http://www.w3.org/1999/02/22-rdf-syntax-ns#>.
@prefix rdfs: <http://www.w3.org/2000/01/rdf-schema#>.
@prefix foaf: <http://xmlns.com/foaf/0.1/>.
@prefix xsd: <http://www.w3.org/2001/XMLSchema#>.
@prefix dcterms: <http://purl.org/dc/terms/>.
@prefix owl: <http://www.w3.org/2002/07/owl#>.
@prefix jsonsc: <https://www.w3.org/2019/wot/json-schema#>.
@prefix jsonsc-ld: <http://w3id.org/jsonsc-ld/>.
@prefix api: <http://purl.org/linked-data/api/vocab>.
@prefix geo: <http://www.w3.org/2003/01/geo/wgs84_pos#>.
@prefix mobivoc: <http://schema.mobivoc.org/#>.
@prefix geosparql: <http://www.opengis.net/ont/geosparql#>.
@prefix sdm: <https://w3id.org/sdm#>.

<https://smart-data-models.github.io/dataModel.WaterDistributionManagementEPANET/Pump/schema.json> dcterms:title "Smart Data Models. WaterNetworkManagementEPANET - Pump";
    dcterms:description "This entity contains a harmonised description of a generic pump made for the Water Network Management domain. This entity is primarily associated with the water management vertical and related IoT applications.".
sdm:type dcterms:description "Property. NGSI-LD Entity Type. It must be equal to Pump.";
    rdf:type rdf:Property;
    rdfs:label "type";
    rdfs:domain <https://smart-data-models.github.io/dataModel.WaterDistributionManagementEPANET/Pump/schema.json>.
sdm:Type rdf:type skos:ConceptScheme.
sdm:type rdfs:range [
  owl:oneOf (sdm:Pump)
].
sdm:Pump rdf:type skos:Concept;
    skos:inScheme sdm:Type;
    rdfs:label "Pump".
sdm:power dcterms:description "Property. Model:'https://schema.org/Number'. Units:'KiloWatt'. The power supplied by the pump. All units are accepted in [CEFACT](https://www.unece.org/cefact.html) code.";
    rdf:type rdf:Property;
    rdfs:label "power";
    rdfs:domain <https://smart-data-models.github.io/dataModel.WaterDistributionManagementEPANET/Pump/schema.json>;
    rdfs:range xsd:decimal.
sdm:speed dcterms:description "Property. Model:'https://schema.org/Number'. Units:'Metre per Second'. The relative speed setting of the Pump. All units are accepted in [CEFACT](https://www.unece.org/cefact.html) code.";
    rdf:type rdf:Property;
    rdfs:label "speed";
    rdfs:domain <https://smart-data-models.github.io/dataModel.WaterDistributionManagementEPANET/Pump/schema.json>;
    rdfs:range xsd:decimal.
sdm:startsAt dcterms:description "Relationship. The ID of the node on the suction side of the pump";
    rdf:type rdf:Property;
    rdfs:label "startsAt";
    rdfs:domain <https://smart-data-models.github.io/dataModel.WaterDistributionManagementEPANET/Pump/schema.json>.
sdm:endsAt dcterms:description "Relationship. The ID of the node on the discharge side of the pump";
    rdf:type rdf:Property;
    rdfs:label "endsAt";
    rdfs:domain <https://smart-data-models.github.io/dataModel.WaterDistributionManagementEPANET/Pump/schema.json>.
sdm:vertices dcterms:description "Geoproperty. Coordinates of all vertices in the pump, ordered from the startsAt node to the endsAt node and encoded as a GeoJSON ";
    rdf:type rdf:Property;
    rdfs:label "vertices";
    rdfs:domain <https://smart-data-models.github.io/dataModel.WaterDistributionManagementEPANET/Pump/schema.json>.
sdm:headCurve dcterms:description "Relationship. The ID label of the pump curve used to describe the relationship between the head delivered by the pump and the flow through the Pump.";
    rdf:type rdf:Property;
    rdfs:label "headCurve";
    rdfs:domain <https://smart-data-models.github.io/dataModel.WaterDistributionManagementEPANET/Pump/schema.json>;
    rdfs:range xsd:anyURI.
sdm:pumpPattern dcterms:description "Relationship. The ID label of a time pattern used to control the pump's operation. The multipliers of the pattern are equivalent to speed settings. A multiplier of zero implies that the pump will be shut off during the corresponding time period";
    rdf:type rdf:Property;
    rdfs:label "pumpPattern";
    rdfs:domain <https://smart-data-models.github.io/dataModel.WaterDistributionManagementEPANET/Pump/schema.json>.
sdm:efficCurve dcterms:description "Relationship. The ID label of the curve that represents the pump's wire-to-water efficiency as a function of flow rate.";
    rdf:type rdf:Property;
    rdfs:label "efficCurve";
    rdfs:domain <https://smart-data-models.github.io/dataModel.WaterDistributionManagementEPANET/Pump/schema.json>.
sdm:energyPrice dcterms:description "Property. Units:'No unit'. The average or nominal price of energy in monetary units. All units are accepted in [CEFACT](https://www.unece.org/cefact.html) code.";
    rdf:type rdf:Property;
    rdfs:label "energyPrice";
    rdfs:domain <https://smart-data-models.github.io/dataModel.WaterDistributionManagementEPANET/Pump/schema.json>;
    rdfs:range xsd:decimal.
sdm:energyPattern dcterms:description "Relationship. The ID label of the time pattern used to describe the variation in energy price throughout the day.";
    rdf:type rdf:Property;
    rdfs:label "energyPattern";
    rdfs:domain <https://smart-data-models.github.io/dataModel.WaterDistributionManagementEPANET/Pump/schema.json>.
