@prefix schema: <https://schema.org/>.
@prefix skos: <http://www.w3.org/2004/02/skos/core#>.
@prefix rdf: <http://www.w3.org/1999/02/22-rdf-syntax-ns#>.
@prefix rdfs: <http://www.w3.org/2000/01/rdf-schema#>.
@prefix foaf: <http://xmlns.com/foaf/0.1/>.
@prefix xsd: <http://www.w3.org/2001/XMLSchema#>.
@prefix dcterms: <http://purl.org/dc/terms/>.
@prefix owl: <http://www.w3.org/2002/07/owl#>.
@prefix jsonsc: <https://www.w3.org/2019/wot/json-schema#>.
@prefix jsonsc-ld: <http://w3id.org/jsonsc-ld/>.
@prefix api: <http://purl.org/linked-data/api/vocab>.
@prefix geo: <http://www.w3.org/2003/01/geo/wgs84_pos#>.
@prefix mobivoc: <http://schema.mobivoc.org/#>.
@prefix geosparql: <http://www.opengis.net/ont/geosparql#>.
@prefix sdm: <https://w3id.org/sdm#>.

<https://smart-data-models.github.io/data-models/specs/WasteWaterTreatment/WasteWaterSimulationResults/schema.json> dcterms:title "Smart Data Models - WasteWaterSimulationResults";
    dcterms:description "This entity contains an harmonised description of a WasteWaterSimulationResults made for the Wastewater treatment domain. The entity contains properties that are parameters which have been predicted or forecasted by models through a simulation.".
sdm:type dcterms:description "Property. NGSI-LD Entity Type. It has to be a WasteWaterSimulationResults.";
    rdf:type rdf:Property;
    rdfs:label "type";
    rdfs:domain <https://smart-data-models.github.io/data-models/specs/WasteWaterTreatment/WasteWaterSimulationResults/schema.json>.
sdm:Type rdf:type skos:ConceptScheme.
sdm:type rdfs:range [
  owl:oneOf (sdm:WasteWaterSimulationResult)
].
sdm:WasteWaterSimulationResult rdf:type skos:Concept;
    skos:inScheme sdm:Type;
    rdfs:label "WasteWaterSimulationResult".
sdm:airflow dcterms:description "Property. Model: https://schema.org/Number. Units: 'm/s'. Estimation of airflow from a blower generated through aeration of a given wastewater entity, by a simulation/data-driven model.";
    rdf:type rdf:Property;
    rdfs:label "airflow";
    rdfs:domain <https://smart-data-models.github.io/data-models/specs/WasteWaterTreatment/WasteWaterSimulationResults/schema.json>;
    rdfs:range xsd:decimal.
sdm:power dcterms:description "Property. Model: https://schema.org/Number. Units: 'kW'. Estimation of power consumed by a blower for the aeration process to a given wastewater entity, by a simulation/data-driven model.";
    rdf:type rdf:Property;
    rdfs:label "power";
    rdfs:domain <https://smart-data-models.github.io/data-models/specs/WasteWaterTreatment/WasteWaterSimulationResults/schema.json>;
    rdfs:range xsd:decimal.
sdm:nh4 dcterms:description "Property. Model: https://schema.org/Number. Units: 'mg/L'. Estimation of ammonia concentration at a given wastewater entity, by a simulation/data-driven model.";
    rdf:type rdf:Property;
    rdfs:label "nh4";
    rdfs:domain <https://smart-data-models.github.io/data-models/specs/WasteWaterTreatment/WasteWaterSimulationResults/schema.json>;
    rdfs:range xsd:decimal.
sdm:no3 dcterms:description "Property. Model: https://schema.org/Number. Units: 'mg/L'. Estimation of nitrate concentration at a given wastewater entity, by a simulation/data-driven model.";
    rdf:type rdf:Property;
    rdfs:label "no3";
    rdfs:domain <https://smart-data-models.github.io/data-models/specs/WasteWaterTreatment/WasteWaterSimulationResults/schema.json>;
    rdfs:range xsd:decimal.
