@prefix schema: <https://schema.org/>.
@prefix skos: <http://www.w3.org/2004/02/skos/core#>.
@prefix rdf: <http://www.w3.org/1999/02/22-rdf-syntax-ns#>.
@prefix rdfs: <http://www.w3.org/2000/01/rdf-schema#>.
@prefix foaf: <http://xmlns.com/foaf/0.1/>.
@prefix xsd: <http://www.w3.org/2001/XMLSchema#>.
@prefix dcterms: <http://purl.org/dc/terms/>.
@prefix owl: <http://www.w3.org/2002/07/owl#>.
@prefix jsonsc: <https://www.w3.org/2019/wot/json-schema#>.
@prefix jsonsc-ld: <http://w3id.org/jsonsc-ld/>.
@prefix api: <http://purl.org/linked-data/api/vocab>.
@prefix geo: <http://www.w3.org/2003/01/geo/wgs84_pos#>.
@prefix mobivoc: <http://schema.mobivoc.org/#>.
@prefix geosparql: <http://www.opengis.net/ont/geosparql#>.
@prefix sdm: <https://w3id.org/sdm#>.

<https://smart-data-models.github.io/dataModels.CIMEnergyClasses/AsynchronousMachineEquivalentCircuit/schema.json> dcterms:title " Smart Data Models - AsynchronousMachineEquivalentCircuit";
    dcterms:description "Adapted from CIM data models. The electrical equations of all variations of the asynchronous model are based on the AsynchronousEquivalentCircuit diagram for the direct and quadrature axes, with two equivalent rotor windings in each axis.      =  +   =  +  *  / ( + )  =  +  * *  / ( *  +  *  +  * )  = ( + ) / ( * )  = ( *  +  *  +  * ) / ( *  * (+ ) Same equations using CIM attributes from AsynchronousMachineTimeConstantReactance class on left of = sign and AsynchronousMachineEquivalentCircuit class on right (except as noted): xs = xm + RotatingMachineDynamics.statorLeakageReactance xp = RotatingMachineDynamics.statorLeakageReactance + xm * xlr1 / (xm + xlr1) xpp = RotatingMachineDynamics.statorLeakageReactance + xm * xlr1* xlr2 / (xm * xlr1 + xm * xlr2 + xlr1 * xlr2) tpo = (xm + xlr1) / (2*pi*nominal frequency * rr1) tppo = (xm * xlr1 + xm * xlr2 + xlr1 * xlr2) / (2*pi*nominal frequency * rr2 * (xm + xlr1).".
sdm:type dcterms:description "Property. NGSI type. It has to be AsynchronousMachineEquivalentCircuit";
    rdf:type rdf:Property;
    rdfs:label "type";
    rdfs:domain <https://smart-data-models.github.io/dataModels.CIMEnergyClasses/AsynchronousMachineEquivalentCircuit/schema.json>.
sdm:Type rdf:type skos:ConceptScheme.
sdm:type rdfs:range [
  owl:oneOf (sdm:AsynchronousMachineEquivalentCircuit)
].
sdm:AsynchronousMachineEquivalentCircuit rdf:type skos:Concept;
    skos:inScheme sdm:Type;
    rdfs:label "AsynchronousMachineEquivalentCircuit".
sdm:rr1 dcterms:description "Property. Model:'https://schema.org/Number'. Damper 1 winding resistance. Default: 0.0";
    rdf:type rdf:Property;
    rdfs:label "rr1";
    rdfs:domain <https://smart-data-models.github.io/dataModels.CIMEnergyClasses/AsynchronousMachineEquivalentCircuit/schema.json>;
    rdfs:range xsd:decimal.
sdm:rr2 dcterms:description "Property. Model:'https://schema.org/Number'. Damper 2 winding resistance. Default: 0.0";
    rdf:type rdf:Property;
    rdfs:label "rr2";
    rdfs:domain <https://smart-data-models.github.io/dataModels.CIMEnergyClasses/AsynchronousMachineEquivalentCircuit/schema.json>;
    rdfs:range xsd:decimal.
sdm:xlr1 dcterms:description "Property. Model:'https://schema.org/Number'. Damper 1 winding leakage reactance. Default: 0.0";
    rdf:type rdf:Property;
    rdfs:label "xlr1";
    rdfs:domain <https://smart-data-models.github.io/dataModels.CIMEnergyClasses/AsynchronousMachineEquivalentCircuit/schema.json>;
    rdfs:range xsd:decimal.
sdm:xlr2 dcterms:description "Property. Model:'https://schema.org/Number'. Damper 2 winding leakage reactance. Default: 0.0";
    rdf:type rdf:Property;
    rdfs:label "xlr2";
    rdfs:domain <https://smart-data-models.github.io/dataModels.CIMEnergyClasses/AsynchronousMachineEquivalentCircuit/schema.json>;
    rdfs:range xsd:decimal.
sdm:xm dcterms:description "Property. Model:'https://schema.org/Number'. Magnetizing reactance. Default: 0.0";
    rdf:type rdf:Property;
    rdfs:label "xm";
    rdfs:domain <https://smart-data-models.github.io/dataModels.CIMEnergyClasses/AsynchronousMachineEquivalentCircuit/schema.json>;
    rdfs:range xsd:decimal.
