@prefix schema: <https://schema.org/>.
@prefix skos: <http://www.w3.org/2004/02/skos/core#>.
@prefix rdf: <http://www.w3.org/1999/02/22-rdf-syntax-ns#>.
@prefix rdfs: <http://www.w3.org/2000/01/rdf-schema#>.
@prefix foaf: <http://xmlns.com/foaf/0.1/>.
@prefix xsd: <http://www.w3.org/2001/XMLSchema#>.
@prefix dcterms: <http://purl.org/dc/terms/>.
@prefix owl: <http://www.w3.org/2002/07/owl#>.
@prefix jsonsc: <https://www.w3.org/2019/wot/json-schema#>.
@prefix jsonsc-ld: <http://w3id.org/jsonsc-ld/>.
@prefix api: <http://purl.org/linked-data/api/vocab>.
@prefix geo: <http://www.w3.org/2003/01/geo/wgs84_pos#>.
@prefix mobivoc: <http://schema.mobivoc.org/#>.
@prefix geosparql: <http://www.opengis.net/ont/geosparql#>.
@prefix sdm: <https://w3id.org/sdm#>.

<https://smart-data-models.github.io/dataModel.Environment/SeaConditions/schema.json> dcterms:title "Sea Conditions schema";
    dcterms:description "This entity contains a harmonised geographic description of sea conditions".
sdm:type dcterms:description "Property. NGSI-LD Entity Type. It has to be SeaConditions";
    rdf:type rdf:Property;
    rdfs:label "type";
    rdfs:domain <https://smart-data-models.github.io/dataModel.Environment/SeaConditions/schema.json>.
sdm:Type rdf:type skos:ConceptScheme.
sdm:type rdfs:range [
  owl:oneOf (sdm:SeaConditions)
].
sdm:SeaConditions rdf:type skos:Concept;
    skos:inScheme sdm:Type;
    rdfs:label "SeaConditions".
sdm:waveLevel dcterms:description "Property. Model:'https://schema.org/Number'. Units:'Douglas sea scale'. It indicates the height of the waves and also measures the swell of the sea.";
    rdf:type rdf:Property;
    rdfs:label "waveLevel";
    rdfs:domain <https://smart-data-models.github.io/dataModel.Environment/SeaConditions/schema.json>;
    rdfs:range xsd:decimal.
sdm:surfaceTemperature dcterms:description "Property. Model:'https://schema.org/Number'. Units:'Celsius degrees'. Sea surface temperature.";
    rdf:type rdf:Property;
    rdfs:label "surfaceTemperature";
    rdfs:domain <https://smart-data-models.github.io/dataModel.Environment/SeaConditions/schema.json>;
    rdfs:range xsd:decimal.
sdm:waveHeight dcterms:description "Property. Model:'https://schema.org/Number'. Units:'Meters'. Height of the waves.";
    rdf:type rdf:Property;
    rdfs:label "waveHeight";
    rdfs:domain <https://smart-data-models.github.io/dataModel.Environment/SeaConditions/schema.json>;
    rdfs:range xsd:decimal.
sdm:wavePeriod dcterms:description "Property. Model:'https://schema.org/Number'. Units:'Seconds'. Indicates the time between the crests of a wave.";
    rdf:type rdf:Property;
    rdfs:label "wavePeriod";
    rdfs:domain <https://smart-data-models.github.io/dataModel.Environment/SeaConditions/schema.json>;
    rdfs:range xsd:decimal.
sdm:pH dcterms:description "Property. Model:'https://schema.org/Number'. Acidity or basicity of an aqueous solution.";
    rdf:type rdf:Property;
    rdfs:label "pH";
    rdfs:domain <https://smart-data-models.github.io/dataModel.Environment/SeaConditions/schema.json>;
    rdfs:range xsd:decimal.
sdm:salinity dcterms:description "Property. Model:'https://schema.org/Number'. Units:'Parts per thousand'. Amount of salts dissolved in water.";
    rdf:type rdf:Property;
    rdfs:label "salinity";
    rdfs:domain <https://smart-data-models.github.io/dataModel.Environment/SeaConditions/schema.json>;
    rdfs:range xsd:decimal.
sdm:dateObserved dcterms:description "Property. Model:'https://schema.org/DateTime'. The date and time of this observation in ISO8601 UTC format.";
    rdf:type rdf:Property;
    rdfs:label "dateObserved";
    rdfs:domain <https://smart-data-models.github.io/dataModel.Environment/SeaConditions/schema.json>;
    rdfs:range xsd:dateTime.
