@prefix schema: <https://schema.org/>.
@prefix skos: <http://www.w3.org/2004/02/skos/core#>.
@prefix rdf: <http://www.w3.org/1999/02/22-rdf-syntax-ns#>.
@prefix rdfs: <http://www.w3.org/2000/01/rdf-schema#>.
@prefix foaf: <http://xmlns.com/foaf/0.1/>.
@prefix xsd: <http://www.w3.org/2001/XMLSchema#>.
@prefix dcterms: <http://purl.org/dc/terms/>.
@prefix owl: <http://www.w3.org/2002/07/owl#>.
@prefix jsonsc: <https://www.w3.org/2019/wot/json-schema#>.
@prefix jsonsc-ld: <http://w3id.org/jsonsc-ld/>.
@prefix api: <http://purl.org/linked-data/api/vocab>.
@prefix geo: <http://www.w3.org/2003/01/geo/wgs84_pos#>.
@prefix mobivoc: <http://schema.mobivoc.org/#>.
@prefix geosparql: <http://www.opengis.net/ont/geosparql#>.
@prefix sdm: <https://w3id.org/sdm#>.

<https://smart-data-models.github.io/data-models.OpenChannelManagement/RegulationStructureSimulation/schema.json> dcterms:title "Smart Data Models - RegulationStructureSimulation";
    dcterms:description "This entity contains a harmonised description of a data model for regulation structure simulation, for Raw-Water (Open Channels) System Management domain.".
sdm:type dcterms:description "Property. NGSI-LD Entity Type. It has to be RegulationStructureSimulation.";
    rdf:type rdf:Property;
    rdfs:label "type";
    rdfs:domain <https://smart-data-models.github.io/data-models.OpenChannelManagement/RegulationStructureSimulation/schema.json>.
sdm:Type rdf:type skos:ConceptScheme.
sdm:type rdfs:range [
  owl:oneOf (sdm:RegulationStructureSimulation)
].
sdm:RegulationStructureSimulation rdf:type skos:Concept;
    skos:inScheme sdm:Type;
    rdfs:label "RegulationStructureSimulation".
sdm:startSimulationTime dcterms:description "Property. Time of day in ISO8601 UTC format at which the simulation begins.";
    rdf:type rdf:Property;
    rdfs:label "startSimulationTime";
    rdfs:domain <https://smart-data-models.github.io/data-models.OpenChannelManagement/RegulationStructureSimulation/schema.json>;
    rdfs:range xsd:dateTime.
sdm:endSimulationTime dcterms:description "Property. Time of day in ISO8601 UTC format at which the simulation ends.";
    rdf:type rdf:Property;
    rdfs:label "endSimulationTime";
    rdfs:domain <https://smart-data-models.github.io/data-models.OpenChannelManagement/RegulationStructureSimulation/schema.json>;
    rdfs:range xsd:dateTime.
sdm:modelError dcterms:description "Property. Percentage error between observed and simulated discharge.";
    rdf:type rdf:Property;
    rdfs:label "modelError";
    rdfs:domain <https://smart-data-models.github.io/data-models.OpenChannelManagement/RegulationStructureSimulation/schema.json>;
    rdfs:range xsd:decimal.
sdm:targetDischarge dcterms:description "Property. Desirable discharge to be established in the channel, defined by the utilityâ€™s operators.";
    rdf:type rdf:Property;
    rdfs:label "targetDischarge";
    rdfs:domain <https://smart-data-models.github.io/data-models.OpenChannelManagement/RegulationStructureSimulation/schema.json>;
    rdfs:range xsd:decimal.
sdm:modelledDischarge dcterms:description "Property. Discharge estimated from the simulation model.";
    rdf:type rdf:Property;
    rdfs:label "modelledDischarge";
    rdfs:domain <https://smart-data-models.github.io/data-models.OpenChannelManagement/RegulationStructureSimulation/schema.json>;
    rdfs:range xsd:decimal.
sdm:spillwayFlow dcterms:description "Property. Ratio of the spillway discharge to the new total discharge";
    rdf:type rdf:Property;
    rdfs:label "spillwayFlow";
    rdfs:domain <https://smart-data-models.github.io/data-models.OpenChannelManagement/RegulationStructureSimulation/schema.json>;
    rdfs:range xsd:decimal.
sdm:estimatedGateDischargeCoefficient dcterms:description "Property. Calibrated discharge coefficient of the sluice gate.";
    rdf:type rdf:Property;
    rdfs:label "estimatedGateDischargeCoefficient";
    rdfs:domain <https://smart-data-models.github.io/data-models.OpenChannelManagement/RegulationStructureSimulation/schema.json>;
    rdfs:range xsd:decimal.
sdm:equivalentSluiceOpening dcterms:description "Property. Equivalent sluice gate opening in the case of multiple sluice gates, estimated as the mean value of the different openings.";
    rdf:type rdf:Property;
    rdfs:label "equivalentSluiceOpening";
    rdfs:domain <https://smart-data-models.github.io/data-models.OpenChannelManagement/RegulationStructureSimulation/schema.json>;
    rdfs:range xsd:decimal.
sdm:simulationOutput dcterms:description "Property. Description of the set of results of simulation of the regulation structure.";
    rdf:type rdf:Property;
    rdfs:label "simulationOutput";
    rdfs:domain <https://smart-data-models.github.io/data-models.OpenChannelManagement/RegulationStructureSimulation/schema.json>;
    rdfs:range sdm:SimulationOutput.
sdm:SimulationOutput rdf:type rdfs:Class;
    rdfs:label "SimulationOutput".
sdm:waterAttribute dcterms:description "Property: An attribute issued from the data models for Open Channel Management. It follows fully this data model and it could be a property or a relationship. It contains the values for specified properties, as derive from the simulation.";
    rdf:type rdf:Property;
    rdfs:label "waterAttribute";
    rdfs:domain sdm:SimulationOutput.
sdm:WaterAttribute rdf:type skos:ConceptScheme.
sdm:waterAttribute rdfs:range [
  owl:oneOf (sdm:gateOpening sdm:waterDischarge sdm:headDifference sdm:gateDischargeCoefficient sdm:waterFlow sdm:waterVelocity sdm:celerity sdm:travelDuration sdm:waterLevel)
].
sdm:gateOpening rdf:type skos:Concept;
    skos:inScheme sdm:WaterAttribute;
    rdfs:label "gateOpening".
sdm:waterDischarge rdf:type skos:Concept;
    skos:inScheme sdm:WaterAttribute;
    rdfs:label "waterDischarge".
sdm:headDifference rdf:type skos:Concept;
    skos:inScheme sdm:WaterAttribute;
    rdfs:label "headDifference".
sdm:gateDischargeCoefficient rdf:type skos:Concept;
    skos:inScheme sdm:WaterAttribute;
    rdfs:label "gateDischargeCoefficient".
sdm:waterFlow rdf:type skos:Concept;
    skos:inScheme sdm:WaterAttribute;
    rdfs:label "waterFlow".
sdm:waterVelocity rdf:type skos:Concept;
    skos:inScheme sdm:WaterAttribute;
    rdfs:label "waterVelocity".
sdm:celerity rdf:type skos:Concept;
    skos:inScheme sdm:WaterAttribute;
    rdfs:label "celerity".
sdm:travelDuration rdf:type skos:Concept;
    skos:inScheme sdm:WaterAttribute;
    rdfs:label "travelDuration".
sdm:waterLevel rdf:type skos:Concept;
    skos:inScheme sdm:WaterAttribute;
    rdfs:label "waterLevel".
sdm:value rdf:type rdf:Property;
    rdfs:label "value";
    rdfs:domain sdm:SimulationOutput.
sdm:targetURI dcterms:description "Relationship. A relationship indicating the network component with a simulated property value.";
    rdf:type rdf:Property;
    rdfs:label "targetURI";
    rdfs:domain sdm:SimulationOutput.
sdm:inputParameters dcterms:description "Property. Description of the set of the modifications to be applied to the Regulation Structure for the simulation.";
    rdf:type rdf:Property;
    rdfs:label "inputParameters";
    rdfs:domain <https://smart-data-models.github.io/data-models.OpenChannelManagement/RegulationStructureSimulation/schema.json>;
    rdfs:range sdm:InputParameter.
sdm:InputParameter rdf:type rdfs:Class;
    rdfs:label "InputParameter".
sdm:waterAttribute dcterms:description "Property: An attribute issued from the data models for Open Channel Management. It follows fully this data model and it could be a property or a relationship. It contains the values for specified properties, as derive from the simulation.";
    rdf:type rdf:Property;
    rdfs:label "waterAttribute";
    rdfs:domain sdm:InputParameter;
    rdfs:range xsd:string.
sdm:value rdf:type rdf:Property;
    rdfs:label "value";
    rdfs:domain sdm:InputParameter.
sdm:targetURI dcterms:description "Relationship. A relationship indicating the network component with a simulated property value.";
    rdf:type rdf:Property;
    rdfs:label "targetURI";
    rdfs:domain sdm:InputParameter.
sdm:initialConditions dcterms:description "Property. Description of the set of the modifications to be applied to the Regulation Structure for the simulation.";
    rdf:type rdf:Property;
    rdfs:label "initialConditions";
    rdfs:domain <https://smart-data-models.github.io/data-models.OpenChannelManagement/RegulationStructureSimulation/schema.json>;
    rdfs:range sdm:InitialCondition.
sdm:InitialCondition rdf:type rdfs:Class;
    rdfs:label "InitialCondition".
sdm:waterAttribute dcterms:description "Property: An attribute issued from the data models for Open Channel Management. It follows fully this data model and it could be a property or a relationship. It contains the values for specified properties, as derive from the simulation.";
    rdf:type rdf:Property;
    rdfs:label "waterAttribute";
    rdfs:domain sdm:InitialCondition;
    rdfs:range xsd:string.
sdm:value rdf:type rdf:Property;
    rdfs:label "value";
    rdfs:domain sdm:InitialCondition.
sdm:targetURI dcterms:description "Relationship. A relationship indicating the network component with a simulated property value.";
    rdf:type rdf:Property;
    rdfs:label "targetURI";
    rdfs:domain sdm:InitialCondition.
