@prefix schema: <https://schema.org/>.
@prefix skos: <http://www.w3.org/2004/02/skos/core#>.
@prefix rdf: <http://www.w3.org/1999/02/22-rdf-syntax-ns#>.
@prefix rdfs: <http://www.w3.org/2000/01/rdf-schema#>.
@prefix foaf: <http://xmlns.com/foaf/0.1/>.
@prefix xsd: <http://www.w3.org/2001/XMLSchema#>.
@prefix dcterms: <http://purl.org/dc/terms/>.
@prefix owl: <http://www.w3.org/2002/07/owl#>.
@prefix jsonsc: <https://www.w3.org/2019/wot/json-schema#>.
@prefix jsonsc-ld: <http://w3id.org/jsonsc-ld/>.
@prefix api: <http://purl.org/linked-data/api/vocab>.
@prefix geo: <http://www.w3.org/2003/01/geo/wgs84_pos#>.
@prefix mobivoc: <http://schema.mobivoc.org/#>.
@prefix geosparql: <http://www.opengis.net/ont/geosparql#>.
@prefix sdm: <https://w3id.org/sdm#>.

<https://smart-data-models.github.io/dataModel.WaterDistributionManagementEPANET/Pipe/schema.json> dcterms:title "Smart Data Models. WaterNetworkManagementEPANET - Pipe";
    dcterms:description "This entity contains a harmonised description of a generic pipe made for the Water Network Management domain. This entity is primarily associated with the water management vertical and related IoT applications.".
sdm:type dcterms:description "Property. NGSI-LD Entity Type. It has to be Pipe";
    rdf:type rdf:Property;
    rdfs:label "type";
    rdfs:domain <https://smart-data-models.github.io/dataModel.WaterDistributionManagementEPANET/Pipe/schema.json>.
sdm:Type rdf:type skos:ConceptScheme.
sdm:type rdfs:range [
  owl:oneOf (sdm:Pipe)
].
sdm:Pipe rdf:type skos:Concept;
    skos:inScheme sdm:Type;
    rdfs:label "Pipe".
sdm:length dcterms:description "Property. Model:'https://schema.org/Number'. Units:'Metre'. The actual length of the pipe. All units are accepted in [CEFACT](https://www.unece.org/cefact.html) code.";
    rdf:type rdf:Property;
    rdfs:label "length";
    rdfs:domain <https://smart-data-models.github.io/dataModel.WaterDistributionManagementEPANET/Pipe/schema.json>;
    rdfs:range xsd:decimal.
sdm:diameter dcterms:description "Property. Model:'https://schema.org/Number'. Units:'Millimetre'. The pipe diameter";
    rdf:type rdf:Property;
    rdfs:label "diameter";
    rdfs:domain <https://smart-data-models.github.io/dataModel.WaterDistributionManagementEPANET/Pipe/schema.json>;
    rdfs:range xsd:decimal.
sdm:roughness dcterms:description "Property. Model:'https://schema.org/Number'. Units:'No unit'. The roughness coefficient of the Pipe.";
    rdf:type rdf:Property;
    rdfs:label "roughness";
    rdfs:domain <https://smart-data-models.github.io/dataModel.WaterDistributionManagementEPANET/Pipe/schema.json>;
    rdfs:range xsd:decimal.
sdm:minorLoss dcterms:description "Property. Model:'https://schema.org/Number'. Units:'No unit'. Unitless minor loss coefficient associated with bends, fittings, etc";
    rdf:type rdf:Property;
    rdfs:label "minorLoss";
    rdfs:domain <https://smart-data-models.github.io/dataModel.WaterDistributionManagementEPANET/Pipe/schema.json>;
    rdfs:range xsd:decimal.
sdm:startsAt dcterms:description "Relationship. The ID of the node where the pipe begins";
    rdf:type rdf:Property;
    rdfs:label "startsAt";
    rdfs:domain <https://smart-data-models.github.io/dataModel.WaterDistributionManagementEPANET/Pipe/schema.json>;
    rdfs:range xsd:anyURI.
sdm:endsAt dcterms:description "Relationship. The ID of the node where the pipe ends";
    rdf:type rdf:Property;
    rdfs:label "endsAt";
    rdfs:domain <https://smart-data-models.github.io/dataModel.WaterDistributionManagementEPANET/Pipe/schema.json>;
    rdfs:range xsd:anyURI.
sdm:wallCoeff dcterms:description "Property. Model:'https://schema.org/Number'. Units:'mg/mÂ²/day'. The wall reaction coefficient for the pipe. Use a positive value for growth and a negative value for decay. All units are accepted in [CEFACT](https://www.unece.org/cefact.html) code.";
    rdf:type rdf:Property;
    rdfs:label "wallCoeff";
    rdfs:domain <https://smart-data-models.github.io/dataModel.WaterDistributionManagementEPANET/Pipe/schema.json>;
    rdfs:range xsd:decimal.
sdm:bulkCoeff dcterms:description "Property. Model:'https://schema.org/Number'. Units:'reciprocal day' The bulk reaction coefficient for the pipe. Use a positive value for growth and a negative value for decay. All units are accepted in [CEFACT](https://www.unece.org/cefact.html) code.";
    rdf:type rdf:Property;
    rdfs:label "bulkCoeff";
    rdfs:domain <https://smart-data-models.github.io/dataModel.WaterDistributionManagementEPANET/Pipe/schema.json>;
    rdfs:range xsd:decimal.
sdm:vertices dcterms:description "Geoproperty. Coordinates of all vertices in the pipe, ordered from the startsAt node to the endsAt node and encoded as a GeoJSON ";
    rdf:type rdf:Property;
    rdfs:label "vertices";
    rdfs:domain <https://smart-data-models.github.io/dataModel.WaterDistributionManagementEPANET/Pipe/schema.json>.
