@prefix schema: <https://schema.org/>.
@prefix skos: <http://www.w3.org/2004/02/skos/core#>.
@prefix rdf: <http://www.w3.org/1999/02/22-rdf-syntax-ns#>.
@prefix rdfs: <http://www.w3.org/2000/01/rdf-schema#>.
@prefix foaf: <http://xmlns.com/foaf/0.1/>.
@prefix xsd: <http://www.w3.org/2001/XMLSchema#>.
@prefix dcterms: <http://purl.org/dc/terms/>.
@prefix owl: <http://www.w3.org/2002/07/owl#>.
@prefix jsonsc: <https://www.w3.org/2019/wot/json-schema#>.
@prefix jsonsc-ld: <http://w3id.org/jsonsc-ld/>.
@prefix api: <http://purl.org/linked-data/api/vocab>.
@prefix geo: <http://www.w3.org/2003/01/geo/wgs84_pos#>.
@prefix mobivoc: <http://schema.mobivoc.org/#>.
@prefix geosparql: <http://www.opengis.net/ont/geosparql#>.
@prefix sdm: <https://w3id.org/sdm#>.

<https://smart-data-models.github.io/dataModel.Agrifood/AnimalDisease/schema.json> dcterms:title "Animal Disease FarmData4All i4Trust";
    dcterms:description "Object modelling an animal disease for a livestock farm.".
sdm:type dcterms:description "Property. NGSI entity type. It has to be AnimalDisease";
    rdf:type rdf:Property;
    rdfs:label "type";
    rdfs:domain <https://smart-data-models.github.io/dataModel.Agrifood/AnimalDisease/schema.json>.
sdm:Type rdf:type skos:ConceptScheme.
sdm:type rdfs:range [
  owl:oneOf (sdm:AnimalDisease)
].
sdm:AnimalDisease rdf:type skos:Concept;
    skos:inScheme sdm:Type;
    rdfs:label "AnimalDisease".
sdm:disease dcterms:description "Property. Animal disease. Indicates the disease the animal has as diagnosed by a veterinarian. Spanish source of diseases https://www.mapa.gob.es/es/ganaderia/temas/sanidad-animal-higiene-ganadera/sanidad-animal/enfermedades/";
    rdf:type rdf:Property;
    rdfs:label "disease";
    rdfs:domain <https://smart-data-models.github.io/dataModel.Agrifood/AnimalDisease/schema.json>;
    rdfs:range xsd:string.
sdm:diagnosticTest dcterms:description "Property. Diagnostic test performed in the animals for the determination of the disease by a veterinarian.";
    rdf:type rdf:Property;
    rdfs:label "diagnosticTest";
    rdfs:domain <https://smart-data-models.github.io/dataModel.Agrifood/AnimalDisease/schema.json>;
    rdfs:range xsd:string.
sdm:date dcterms:description "Property. Date of diagnosis of the disease by a veterinarian.";
    rdf:type rdf:Property;
    rdfs:label "date";
    rdfs:domain <https://smart-data-models.github.io/dataModel.Agrifood/AnimalDisease/schema.json>;
    rdfs:range xsd:dateTime.
sdm:veterinarianTreatment dcterms:description "Relationship. Medical treatment diagnosed by the veterinarian to treat the disease. https://github.com/smart-data-models/dataModel.Agrifood/blob/master/VeterinarianTreatment/schema.json";
    rdf:type rdf:Property;
    rdfs:label "veterinarianTreatment";
    rdfs:domain <https://smart-data-models.github.io/dataModel.Agrifood/AnimalDisease/schema.json>;
    rdfs:range xsd:anyURI.
sdm:animals rdf:type rdf:Property;
    rdfs:label "animals";
    rdfs:domain <https://smart-data-models.github.io/dataModel.Agrifood/AnimalDisease/schema.json>;
    rdfs:range xsd:anyURI.
sdm:veterinarian dcterms:description "Relationship. Diagnostic veterinarian. Relationship to the prescribing veterinarian";
    rdf:type rdf:Property;
    rdfs:label "veterinarian";
    rdfs:domain <https://smart-data-models.github.io/dataModel.Agrifood/AnimalDisease/schema.json>;
    rdfs:range xsd:anyURI.
