@prefix schema: <https://schema.org/>.
@prefix skos: <http://www.w3.org/2004/02/skos/core#>.
@prefix rdf: <http://www.w3.org/1999/02/22-rdf-syntax-ns#>.
@prefix rdfs: <http://www.w3.org/2000/01/rdf-schema#>.
@prefix foaf: <http://xmlns.com/foaf/0.1/>.
@prefix xsd: <http://www.w3.org/2001/XMLSchema#>.
@prefix dcterms: <http://purl.org/dc/terms/>.
@prefix owl: <http://www.w3.org/2002/07/owl#>.
@prefix jsonsc: <https://www.w3.org/2019/wot/json-schema#>.
@prefix jsonsc-ld: <http://w3id.org/jsonsc-ld/>.
@prefix api: <http://purl.org/linked-data/api/vocab>.
@prefix geo: <http://www.w3.org/2003/01/geo/wgs84_pos#>.
@prefix mobivoc: <http://schema.mobivoc.org/#>.
@prefix geosparql: <http://www.opengis.net/ont/geosparql#>.
@prefix sdm: <https://w3id.org/sdm#>.

<https://smart-data-models.github.io/data-models/specs/WasteWaterTreatment/OffGasStack/schema.json> dcterms:title "WasteWaterTreatment - Off-gas Stack";
    dcterms:description "This entity contains a harmonised description of a generic Off-gas Stack made for the Wastewater treatment domain. This entity represents stacks that are present in some wastewater treatment plants where the emissions, greenhouse gases included, are emitted.".
sdm:type dcterms:description "Property. NGSI-LD Entity Type. it has to be OffGasStack";
    rdf:type rdf:Property;
    rdfs:label "type";
    rdfs:domain <https://smart-data-models.github.io/data-models/specs/WasteWaterTreatment/OffGasStack/schema.json>.
sdm:Type rdf:type skos:ConceptScheme.
sdm:type rdfs:range [
  owl:oneOf (sdm:OffGasStack)
].
sdm:OffGasStack rdf:type skos:Concept;
    skos:inScheme sdm:Type;
    rdfs:label "OffGasStack".
sdm:n2o dcterms:description "Property. Model: https://schema.org/Number. Units: 'ppm'. N2O gas emissions from an off-gas stack entity.";
    rdf:type rdf:Property;
    rdfs:label "n2o";
    rdfs:domain <https://smart-data-models.github.io/data-models/specs/WasteWaterTreatment/OffGasStack/schema.json>;
    rdfs:range xsd:decimal.
sdm:co2 dcterms:description "Property. Model: https://schema.org/Number. Units: 'ppm'. CO2 gas emissions from an off-gas stack entity.";
    rdf:type rdf:Property;
    rdfs:label "co2";
    rdfs:domain <https://smart-data-models.github.io/data-models/specs/WasteWaterTreatment/OffGasStack/schema.json>;
    rdfs:range xsd:decimal.
sdm:ch4 dcterms:description "Property. Model: https://schema.org/Number. Units: 'ppm'. CH4 gas emissions from an off-gas stack entity.";
    rdf:type rdf:Property;
    rdfs:label "ch4";
    rdfs:domain <https://smart-data-models.github.io/data-models/specs/WasteWaterTreatment/OffGasStack/schema.json>;
    rdfs:range xsd:decimal.
sdm:o2 dcterms:description "Property. Model: https://schema.org/Number. Units: 'ppm'. O2 gas emissions from an off-gas stack entity.";
    rdf:type rdf:Property;
    rdfs:label "o2";
    rdfs:domain <https://smart-data-models.github.io/data-models/specs/WasteWaterTreatment/OffGasStack/schema.json>;
    rdfs:range xsd:decimal.
sdm:startsAt dcterms:description "Relationship. A relationship indicating the entity the Off Gas Stack is connected to in the upstream point.";
    rdf:type rdf:Property;
    rdfs:label "startsAt";
    rdfs:domain <https://smart-data-models.github.io/data-models/specs/WasteWaterTreatment/OffGasStack/schema.json>;
    rdfs:range xsd:anyURI.
sdm:endsAt dcterms:description "Relationship. A relationship indicating the entity the Off Gas Stack is connected to in the downstream point.";
    rdf:type rdf:Property;
    rdfs:label "endsAt";
    rdfs:domain <https://smart-data-models.github.io/data-models/specs/WasteWaterTreatment/OffGasStack/schema.json>;
    rdfs:range xsd:anyURI.
