@prefix schema: <https://schema.org/>.
@prefix skos: <http://www.w3.org/2004/02/skos/core#>.
@prefix rdf: <http://www.w3.org/1999/02/22-rdf-syntax-ns#>.
@prefix rdfs: <http://www.w3.org/2000/01/rdf-schema#>.
@prefix foaf: <http://xmlns.com/foaf/0.1/>.
@prefix xsd: <http://www.w3.org/2001/XMLSchema#>.
@prefix dcterms: <http://purl.org/dc/terms/>.
@prefix owl: <http://www.w3.org/2002/07/owl#>.
@prefix jsonsc: <https://www.w3.org/2019/wot/json-schema#>.
@prefix jsonsc-ld: <http://w3id.org/jsonsc-ld/>.
@prefix api: <http://purl.org/linked-data/api/vocab>.
@prefix geo: <http://www.w3.org/2003/01/geo/wgs84_pos#>.
@prefix mobivoc: <http://schema.mobivoc.org/#>.
@prefix geosparql: <http://www.opengis.net/ont/geosparql#>.
@prefix sdm: <https://w3id.org/sdm#>.

<https://smart-data-models.github.io/dataModel.Parking/ParkingAccess/schema.json> dcterms:title " - Parking / Parking Access";
    dcterms:description "Parking Access - TODO: Provide a complete Schema".
sdm:type dcterms:description "Property. NGSI Entity type. It has to be ParkingAccess";
    rdf:type rdf:Property;
    rdfs:label "type";
    rdfs:domain <https://smart-data-models.github.io/dataModel.Parking/ParkingAccess/schema.json>.
sdm:Type rdf:type skos:ConceptScheme.
sdm:type rdfs:range [
  owl:oneOf (sdm:ParkingAccess)
].
sdm:ParkingAccess rdf:type skos:Concept;
    skos:inScheme sdm:Type;
    rdfs:label "ParkingAccess".
sdm:category rdf:type rdf:Property;
    rdfs:label "category";
    rdfs:domain <https://smart-data-models.github.io/dataModel.Parking/ParkingAccess/schema.json>;
    rdfs:range xsd:string.
sdm:refOffStreetParking dcterms:description "Relationship. The offstreet parking site this access point gives access to.";
    rdf:type rdf:Property;
    rdfs:label "refOffStreetParking";
    rdfs:domain <https://smart-data-models.github.io/dataModel.Parking/ParkingAccess/schema.json>.
sdm:features rdf:type rdf:Property;
    rdfs:label "features";
    rdfs:domain <https://smart-data-models.github.io/dataModel.Parking/ParkingAccess/schema.json>;
    rdfs:range xsd:string.
sdm:width dcterms:description "Property. Width of the access point. Model:'https://schema.org/width'";
    rdf:type rdf:Property;
    rdfs:label "width";
    rdfs:domain <https://smart-data-models.github.io/dataModel.Parking/ParkingAccess/schema.json>;
    rdfs:range xsd:decimal.
sdm:height dcterms:description "Property. Height of the access point. Model:'https://schema.org/height'";
    rdf:type rdf:Property;
    rdfs:label "height";
    rdfs:domain <https://smart-data-models.github.io/dataModel.Parking/ParkingAccess/schema.json>;
    rdfs:range xsd:decimal.
sdm:slope dcterms:description "Property. Slope of the access point (in relative terms). Model:'https://schema.org/Number'";
    rdf:type rdf:Property;
    rdfs:label "slope";
    rdfs:domain <https://smart-data-models.github.io/dataModel.Parking/ParkingAccess/schema.json>;
    rdfs:range xsd:decimal.
