@prefix schema: <https://schema.org/>.
@prefix skos: <http://www.w3.org/2004/02/skos/core#>.
@prefix rdf: <http://www.w3.org/1999/02/22-rdf-syntax-ns#>.
@prefix rdfs: <http://www.w3.org/2000/01/rdf-schema#>.
@prefix foaf: <http://xmlns.com/foaf/0.1/>.
@prefix xsd: <http://www.w3.org/2001/XMLSchema#>.
@prefix dcterms: <http://purl.org/dc/terms/>.
@prefix owl: <http://www.w3.org/2002/07/owl#>.
@prefix jsonsc: <https://www.w3.org/2019/wot/json-schema#>.
@prefix jsonsc-ld: <http://w3id.org/jsonsc-ld/>.
@prefix api: <http://purl.org/linked-data/api/vocab>.
@prefix geo: <http://www.w3.org/2003/01/geo/wgs84_pos#>.
@prefix mobivoc: <http://schema.mobivoc.org/#>.
@prefix geosparql: <http://www.opengis.net/ont/geosparql#>.
@prefix sdm: <https://w3id.org/sdm#>.

<https://smart-data-models.github.io/dataModel.DCAT_AP/DistributionDCAT-AP/schema.json> dcterms:title "Smart Data models -DCAT-AP distribution of a Dataset,";
    dcterms:description "this is a distribution belonging ot a dataset according to the DCAT-AP standard 2.0.1".
sdm:type dcterms:description "Property. NGSI entity type. It has to be DistributionDCAT-AP";
    rdf:type rdf:Property;
    rdfs:label "type";
    rdfs:domain <https://smart-data-models.github.io/dataModel.DCAT_AP/DistributionDCAT-AP/schema.json>.
sdm:Type rdf:type skos:ConceptScheme.
sdm:type rdfs:range [
  owl:oneOf (sdm:DistributionDCAT-AP)
].
sdm:DistributionDCAT-AP rdf:type skos:Concept;
    skos:inScheme sdm:Type;
    rdfs:label "DistributionDCAT-AP".
sdm:accessUrl rdf:type rdf:Property;
    rdfs:label "accessUrl";
    rdfs:domain <https://smart-data-models.github.io/dataModel.DCAT_AP/DistributionDCAT-AP/schema.json>;
    rdfs:range xsd:string.
sdm:availability dcterms:description "Property. Model:'https://schema.org/Text'. This property indicates how long it is planned to keep the Distribution of the Dataset available.";
    rdf:type rdf:Property;
    rdfs:label "availability";
    rdfs:domain <https://smart-data-models.github.io/dataModel.DCAT_AP/DistributionDCAT-AP/schema.json>;
    rdfs:range xsd:string.
sdm:format dcterms:description "Property. Model:'https://schema.org/Text'. This property refers to the file format of the Distribution.";
    rdf:type rdf:Property;
    rdfs:label "format";
    rdfs:domain <https://smart-data-models.github.io/dataModel.DCAT_AP/DistributionDCAT-AP/schema.json>;
    rdfs:range xsd:string.
sdm:license dcterms:description "Property. Model:'https://schema.org/Text'. This property refers to a data service that gives access to the distribution of the dataset";
    rdf:type rdf:Property;
    rdfs:label "license";
    rdfs:domain <https://smart-data-models.github.io/dataModel.DCAT_AP/DistributionDCAT-AP/schema.json>;
    rdfs:range xsd:string.
sdm:accessService rdf:type rdf:Property;
    rdfs:label "accessService";
    rdfs:domain <https://smart-data-models.github.io/dataModel.DCAT_AP/DistributionDCAT-AP/schema.json>;
    rdfs:range xsd:string.
sdm:byteSize dcterms:description "Property. Model:'https://schema.org/Number'. This property contains the size of a Distribution in bytes.";
    rdf:type rdf:Property;
    rdfs:label "byteSize";
    rdfs:domain <https://smart-data-models.github.io/dataModel.DCAT_AP/DistributionDCAT-AP/schema.json>;
    rdfs:range xsd:decimal.
sdm:checksum dcterms:description "Property. Model:'https://schema.org/Text'. This property provides a mechanism that can be used to verify that the contents of a distribution have not changed. The checksum is related to the downloadURL.";
    rdf:type rdf:Property;
    rdfs:label "checksum";
    rdfs:domain <https://smart-data-models.github.io/dataModel.DCAT_AP/DistributionDCAT-AP/schema.json>;
    rdfs:range xsd:string.
sdm:compressionFormat dcterms:description "Property. Model:'https://schema.org/Text'. This property refers to the format of the file in which the data is contained in a compressed form, e.g. to reduce the size of the downloadable file. It SHOULD be expressed using a media type as defined in the official register of media types managed by IANA";
    rdf:type rdf:Property;
    rdfs:label "compressionFormat";
    rdfs:domain <https://smart-data-models.github.io/dataModel.DCAT_AP/DistributionDCAT-AP/schema.json>;
    rdfs:range xsd:string.
sdm:documentation rdf:type rdf:Property;
    rdfs:label "documentation";
    rdfs:domain <https://smart-data-models.github.io/dataModel.DCAT_AP/DistributionDCAT-AP/schema.json>;
    rdfs:range xsd:string.
sdm:downloadURL rdf:type rdf:Property;
    rdfs:label "downloadURL";
    rdfs:domain <https://smart-data-models.github.io/dataModel.DCAT_AP/DistributionDCAT-AP/schema.json>;
    rdfs:range xsd:anyURI.
sdm:hasPolicy dcterms:description "Property. Model:'https://schema.org/Text'. This property refers to the policy expressing the rights associated with the distribution if using the ODRL vocabulary";
    rdf:type rdf:Property;
    rdfs:label "hasPolicy";
    rdfs:domain <https://smart-data-models.github.io/dataModel.DCAT_AP/DistributionDCAT-AP/schema.json>;
    rdfs:range xsd:string.
sdm:language rdf:type rdf:Property;
    rdfs:label "language";
    rdfs:domain <https://smart-data-models.github.io/dataModel.DCAT_AP/DistributionDCAT-AP/schema.json>;
    rdfs:range xsd:string.
sdm:linkedSchemas rdf:type rdf:Property;
    rdfs:label "linkedSchemas";
    rdfs:domain <https://smart-data-models.github.io/dataModel.DCAT_AP/DistributionDCAT-AP/schema.json>;
    rdfs:range xsd:string.
sdm:mediaType dcterms:description "Property. Model:'https://schema.org/Text'. This property refers to the media type of the Distribution as defined in the official register of media types managed by IANA";
    rdf:type rdf:Property;
    rdfs:label "mediaType";
    rdfs:domain <https://smart-data-models.github.io/dataModel.DCAT_AP/DistributionDCAT-AP/schema.json>;
    rdfs:range xsd:string.
sdm:packagingFormat dcterms:description "Property. Model:'https://schema.org/Text'. This property refers to the format of the file in which one or more data files are grouped together, e.g. to enable a set of related files to be downloaded together. It SHOULD be expressed using a media type as defined in the official register of media types managed by IANA";
    rdf:type rdf:Property;
    rdfs:label "packagingFormat";
    rdfs:domain <https://smart-data-models.github.io/dataModel.DCAT_AP/DistributionDCAT-AP/schema.json>;
    rdfs:range xsd:string.
sdm:releaseDate dcterms:description "Property. Model:'https://schema.org/DateTime'. This property contains the date of formal issuance (e.g., publication) of the Distribution.";
    rdf:type rdf:Property;
    rdfs:label "releaseDate";
    rdfs:domain <https://smart-data-models.github.io/dataModel.DCAT_AP/DistributionDCAT-AP/schema.json>;
    rdfs:range xsd:dateTime.
sdm:rights dcterms:description "Property. Model:'https://schema.org/Text'. This property refers to a statement that specifies rights associated with the Distribution.";
    rdf:type rdf:Property;
    rdfs:label "rights";
    rdfs:domain <https://smart-data-models.github.io/dataModel.DCAT_AP/DistributionDCAT-AP/schema.json>;
    rdfs:range xsd:string.
sdm:spatialResolution rdf:type rdf:Property;
    rdfs:label "spatialResolution";
    rdfs:domain <https://smart-data-models.github.io/dataModel.DCAT_AP/DistributionDCAT-AP/schema.json>;
    rdfs:range xsd:decimal.
sdm:status dcterms:description "Property. Model:'https://schema.org/Text'. This property refers to the maturity of the Distribution. It MUST take one of the values Completed, Deprecated, Under Development, Withdrawn";
    rdf:type rdf:Property;
    rdfs:label "status";
    rdfs:domain <https://smart-data-models.github.io/dataModel.DCAT_AP/DistributionDCAT-AP/schema.json>.
sdm:Status rdf:type skos:ConceptScheme.
sdm:status rdfs:range [
  owl:oneOf (sdm:Completed sdm:Deprecated sdm:Under Development sdm:Withdrawn)
].
sdm:Completed rdf:type skos:Concept;
    skos:inScheme sdm:Status;
    rdfs:label "Completed".
sdm:Deprecated rdf:type skos:Concept;
    skos:inScheme sdm:Status;
    rdfs:label "Deprecated".
sdm:Under Development rdf:type skos:Concept;
    skos:inScheme sdm:Status;
    rdfs:label "Under Development".
sdm:Withdrawn rdf:type skos:Concept;
    skos:inScheme sdm:Status;
    rdfs:label "Withdrawn".
sdm:temporalResolution rdf:type rdf:Property;
    rdfs:label "temporalResolution";
    rdfs:domain <https://smart-data-models.github.io/dataModel.DCAT_AP/DistributionDCAT-AP/schema.json>;
    rdfs:range xsd:decimal.
sdm:title rdf:type rdf:Property;
    rdfs:label "title";
    rdfs:domain <https://smart-data-models.github.io/dataModel.DCAT_AP/DistributionDCAT-AP/schema.json>;
    rdfs:range xsd:string.
sdm:modifiedDate dcterms:description "Property. Model:'https://schema.org/DateTime'. This property contains the most recent date on which the Distribution was changed or modified.";
    rdf:type rdf:Property;
    rdfs:label "modifiedDate";
    rdfs:domain <https://smart-data-models.github.io/dataModel.DCAT_AP/DistributionDCAT-AP/schema.json>;
    rdfs:range xsd:dateTime.
