@prefix schema: <https://schema.org/>.
@prefix skos: <http://www.w3.org/2004/02/skos/core#>.
@prefix rdf: <http://www.w3.org/1999/02/22-rdf-syntax-ns#>.
@prefix rdfs: <http://www.w3.org/2000/01/rdf-schema#>.
@prefix foaf: <http://xmlns.com/foaf/0.1/>.
@prefix xsd: <http://www.w3.org/2001/XMLSchema#>.
@prefix dcterms: <http://purl.org/dc/terms/>.
@prefix owl: <http://www.w3.org/2002/07/owl#>.
@prefix jsonsc: <https://www.w3.org/2019/wot/json-schema#>.
@prefix jsonsc-ld: <http://w3id.org/jsonsc-ld/>.
@prefix api: <http://purl.org/linked-data/api/vocab>.
@prefix geo: <http://www.w3.org/2003/01/geo/wgs84_pos#>.
@prefix mobivoc: <http://schema.mobivoc.org/#>.
@prefix geosparql: <http://www.opengis.net/ont/geosparql#>.
@prefix sdm: <https://w3id.org/sdm#>.

<https://smart-data-models.github.io/dataModel.Battery/Battery/schema.json> dcterms:title "Smart Data Models - Battery";
    dcterms:description "Represent a physical battery with its hardware specifications".
sdm:type dcterms:description "Property. NGSI Entity type. It has to be Battery";
    rdf:type rdf:Property;
    rdfs:label "type";
    rdfs:domain <https://smart-data-models.github.io/dataModel.Battery/Battery/schema.json>.
sdm:Type rdf:type skos:ConceptScheme.
sdm:type rdfs:range [
  owl:oneOf (sdm:Battery)
].
sdm:Battery rdf:type skos:Concept;
    skos:inScheme sdm:Type;
    rdfs:label "Battery".
sdm:refDevice dcterms:description "Relationship. Model:'http://schema.org/URL'. Device providing the measured data about the battery";
    rdf:type rdf:Property;
    rdfs:label "refDevice";
    rdfs:domain <https://smart-data-models.github.io/dataModel.Battery/Battery/schema.json>.
sdm:status rdf:type rdf:Property;
    rdfs:label "status";
    rdfs:domain <https://smart-data-models.github.io/dataModel.Battery/Battery/schema.json>.
sdm:Status rdf:type skos:ConceptScheme.
sdm:status rdfs:range [
  owl:oneOf (sdm:outOfService sdm:withIncidence sdm:working)
].
sdm:outOfService rdf:type skos:Concept;
    skos:inScheme sdm:Status;
    rdfs:label "outOfService".
sdm:withIncidence rdf:type skos:Concept;
    skos:inScheme sdm:Status;
    rdfs:label "withIncidence".
sdm:working rdf:type skos:Concept;
    skos:inScheme sdm:Status;
    rdfs:label "working".
sdm:cycleLife dcterms:description "Property. Model:'http://schema.org/Number'. Numeric value of the load/unload operation cycles for the item'";
    rdf:type rdf:Property;
    rdfs:label "cycleLife";
    rdfs:domain <https://smart-data-models.github.io/dataModel.Battery/Battery/schema.json>;
    rdfs:range xsd:integer.
sdm:autonomyTime dcterms:description "Property. Model:'http://schema.org/Number'. Autonomy of operations of the item without further charge.";
    rdf:type rdf:Property;
    rdfs:label "autonomyTime";
    rdfs:domain <https://smart-data-models.github.io/dataModel.Battery/Battery/schema.json>;
    rdfs:range xsd:string.
sdm:rechargeTime dcterms:description "Property. Model:'http://schema.org/Number'. Time for the full charge of the battery.";
    rdf:type rdf:Property;
    rdfs:label "rechargeTime";
    rdfs:domain <https://smart-data-models.github.io/dataModel.Battery/Battery/schema.json>;
    rdfs:range xsd:string.
sdm:acPowerInput dcterms:description "Property. Model:'http://schema.org/Number'. Numeric value in volts for the alternate current charge. Units:'volts'";
    rdf:type rdf:Property;
    rdfs:label "acPowerInput";
    rdfs:domain <https://smart-data-models.github.io/dataModel.Battery/Battery/schema.json>;
    rdfs:range xsd:decimal.
sdm:acPowerOutput dcterms:description "Property. Model:'http://schema.org/Number'. Numeric value in volts for the alternate output. Units:'volts'";
    rdf:type rdf:Property;
    rdfs:label "acPowerOutput";
    rdfs:domain <https://smart-data-models.github.io/dataModel.Battery/Battery/schema.json>;
    rdfs:range xsd:decimal.
sdm:dcPowerInput dcterms:description "Property. Model:'http://schema.org/Number'. Numeric value in volts for the continuous current charge. Units:'volts'";
    rdf:type rdf:Property;
    rdfs:label "dcPowerInput";
    rdfs:domain <https://smart-data-models.github.io/dataModel.Battery/Battery/schema.json>;
    rdfs:range xsd:decimal.
sdm:dcPowerOutput dcterms:description "Property. Model:'http://schema.org/Number'. Numeric value in volts for the continuous current charge. Units:'volts'";
    rdf:type rdf:Property;
    rdfs:label "dcPowerOutput";
    rdfs:domain <https://smart-data-models.github.io/dataModel.Battery/Battery/schema.json>;
    rdfs:range xsd:decimal.
