@prefix schema: <https://schema.org/>.
@prefix skos: <http://www.w3.org/2004/02/skos/core#>.
@prefix rdf: <http://www.w3.org/1999/02/22-rdf-syntax-ns#>.
@prefix rdfs: <http://www.w3.org/2000/01/rdf-schema#>.
@prefix foaf: <http://xmlns.com/foaf/0.1/>.
@prefix xsd: <http://www.w3.org/2001/XMLSchema#>.
@prefix dcterms: <http://purl.org/dc/terms/>.
@prefix owl: <http://www.w3.org/2002/07/owl#>.
@prefix jsonsc: <https://www.w3.org/2019/wot/json-schema#>.
@prefix jsonsc-ld: <http://w3id.org/jsonsc-ld/>.
@prefix api: <http://purl.org/linked-data/api/vocab>.
@prefix geo: <http://www.w3.org/2003/01/geo/wgs84_pos#>.
@prefix mobivoc: <http://schema.mobivoc.org/#>.
@prefix geosparql: <http://www.opengis.net/ont/geosparql#>.
@prefix sdm: <https://w3id.org/sdm#>.

<https://smart-data-models.github.io/dataModel.Environment/EnvironmentObserved/schema.json> dcterms:title "Smart Data models - Environment-Observed schema";
    dcterms:description "This entity contains a harmonised description of the environmental conditions observed at a particular location and time. This entity is primarily associated with the vertical segment of the environment and agriculture but may also be used in smart home, smart cities, industry and related IoT applications.".
sdm:type dcterms:description "Property. NGSI Entity identifier. It has to be EnvironmentObserved";
    rdf:type rdf:Property;
    rdfs:label "type";
    rdfs:domain <https://smart-data-models.github.io/dataModel.Environment/EnvironmentObserved/schema.json>.
sdm:Type rdf:type skos:ConceptScheme.
sdm:type rdfs:range [
  owl:oneOf (sdm:EnvironmentObserved)
].
sdm:EnvironmentObserved rdf:type skos:Concept;
    skos:inScheme sdm:Type;
    rdfs:label "EnvironmentObserved".
sdm:pointOfInterest dcterms:description "Relationship. A reference to associated Points of Interest (e.g. monitoring stations) that the associated observations are related to.";
    rdf:type rdf:Property;
    rdfs:label "pointOfInterest";
    rdfs:domain <https://smart-data-models.github.io/dataModel.Environment/EnvironmentObserved/schema.json>.
sdm:weatherObserved rdf:type rdf:Property;
    rdfs:label "weatherObserved";
    rdfs:domain <https://smart-data-models.github.io/dataModel.Environment/EnvironmentObserved/schema.json>.
sdm:airQualityObserved dcterms:description "Relationship. A reference to associated AirQualityObserved entities.";
    rdf:type rdf:Property;
    rdfs:label "airQualityObserved";
    rdfs:domain <https://smart-data-models.github.io/dataModel.Environment/EnvironmentObserved/schema.json>.
sdm:waterQualityObserved rdf:type rdf:Property;
    rdfs:label "waterQualityObserved";
    rdfs:domain <https://smart-data-models.github.io/dataModel.Environment/EnvironmentObserved/schema.json>.
