@prefix schema: <https://schema.org/>.
@prefix skos: <http://www.w3.org/2004/02/skos/core#>.
@prefix rdf: <http://www.w3.org/1999/02/22-rdf-syntax-ns#>.
@prefix rdfs: <http://www.w3.org/2000/01/rdf-schema#>.
@prefix foaf: <http://xmlns.com/foaf/0.1/>.
@prefix xsd: <http://www.w3.org/2001/XMLSchema#>.
@prefix dcterms: <http://purl.org/dc/terms/>.
@prefix owl: <http://www.w3.org/2002/07/owl#>.
@prefix jsonsc: <https://www.w3.org/2019/wot/json-schema#>.
@prefix jsonsc-ld: <http://w3id.org/jsonsc-ld/>.
@prefix api: <http://purl.org/linked-data/api/vocab>.
@prefix geo: <http://www.w3.org/2003/01/geo/wgs84_pos#>.
@prefix mobivoc: <http://schema.mobivoc.org/#>.
@prefix geosparql: <http://www.opengis.net/ont/geosparql#>.
@prefix sdm: <https://w3id.org/sdm#>.

<https://smart-data-models.github.io/dataModels.CIMEnergyClasses/SynchronousMachineDetailed/schema.json> dcterms:title " Smart Data Models - SynchronousMachineDetailed";
    dcterms:description "Adapted from CIM data models. All synchronous machine detailed types use a subset of the same data parameters and input/output variables.   The several variations differ in the following ways:   It is not necessary for each simulation tool to have separate models for each of the model types.  The same model can often be used for several types by alternative logic within the model.  Also, differences in saturation representation may not result in significant model performance differences so model substitutions are often acceptable.".
sdm:type dcterms:description "Property. NGSI type. It has to be SynchronousMachineDetailed";
    rdf:type rdf:Property;
    rdfs:label "type";
    rdfs:domain <https://smart-data-models.github.io/dataModels.CIMEnergyClasses/SynchronousMachineDetailed/schema.json>.
sdm:Type rdf:type skos:ConceptScheme.
sdm:type rdfs:range [
  owl:oneOf (sdm:SynchronousMachineDetailed)
].
sdm:SynchronousMachineDetailed rdf:type skos:Concept;
    skos:inScheme sdm:Type;
    rdfs:label "SynchronousMachineDetailed".
sdm:efdBaseRatio dcterms:description "Property. Model:'https://schema.org/Number'. Ratio of Efd bases of exciter and generator models.  Typical Value = 1. Default: 0.0";
    rdf:type rdf:Property;
    rdfs:label "efdBaseRatio";
    rdfs:domain <https://smart-data-models.github.io/dataModels.CIMEnergyClasses/SynchronousMachineDetailed/schema.json>;
    rdfs:range xsd:decimal.
sdm:ifdBaseType dcterms:description "Property. Model:'https://schema.org/Number'. Excitation base system mode.  Typical Value = ifag. Default: None";
    rdf:type rdf:Property;
    rdfs:label "ifdBaseType";
    rdfs:domain <https://smart-data-models.github.io/dataModels.CIMEnergyClasses/SynchronousMachineDetailed/schema.json>;
    rdfs:range xsd:decimal.
sdm:ifdBaseValue dcterms:description "Property. Model:'https://schema.org/Number'. Ifd base current if .ifdBaseType = other. Not needed if .ifdBaseType not = other.   Unit = A.  Typical Value = 0. Default: 0.0";
    rdf:type rdf:Property;
    rdfs:label "ifdBaseValue";
    rdfs:domain <https://smart-data-models.github.io/dataModels.CIMEnergyClasses/SynchronousMachineDetailed/schema.json>;
    rdfs:range xsd:decimal.
sdm:saturationFactor120QAxis dcterms:description "Property. Model:'https://schema.org/Number'. Q-axis saturation factor at 120% of rated terminal voltage (S12q) (>=S1q).  Typical Value = 0.12. Default: 0.0";
    rdf:type rdf:Property;
    rdfs:label "saturationFactor120QAxis";
    rdfs:domain <https://smart-data-models.github.io/dataModels.CIMEnergyClasses/SynchronousMachineDetailed/schema.json>;
    rdfs:range xsd:decimal.
sdm:saturationFactorQAxis dcterms:description "Property. Model:'https://schema.org/Number'. Q-axis saturation factor at rated terminal voltage (S1q) (>= 0). Typical Value = 0.02. Default: 0.0";
    rdf:type rdf:Property;
    rdfs:label "saturationFactorQAxis";
    rdfs:domain <https://smart-data-models.github.io/dataModels.CIMEnergyClasses/SynchronousMachineDetailed/schema.json>;
    rdfs:range xsd:decimal.
