@prefix schema: <https://schema.org/>.
@prefix skos: <http://www.w3.org/2004/02/skos/core#>.
@prefix rdf: <http://www.w3.org/1999/02/22-rdf-syntax-ns#>.
@prefix rdfs: <http://www.w3.org/2000/01/rdf-schema#>.
@prefix foaf: <http://xmlns.com/foaf/0.1/>.
@prefix xsd: <http://www.w3.org/2001/XMLSchema#>.
@prefix dcterms: <http://purl.org/dc/terms/>.
@prefix owl: <http://www.w3.org/2002/07/owl#>.
@prefix jsonsc: <https://www.w3.org/2019/wot/json-schema#>.
@prefix jsonsc-ld: <http://w3id.org/jsonsc-ld/>.
@prefix api: <http://purl.org/linked-data/api/vocab>.
@prefix geo: <http://www.w3.org/2003/01/geo/wgs84_pos#>.
@prefix mobivoc: <http://schema.mobivoc.org/#>.
@prefix geosparql: <http://www.opengis.net/ont/geosparql#>.
@prefix sdm: <https://w3id.org/sdm#>.

<https://smart-data-models.github.io/dataModel.Streetlighting/StreetlightControlCabinet/schema.json> dcterms:title " - Street Lighting / Streetlight Control Cabinet";
    dcterms:description "A Streetlight control cabinet".
sdm:type dcterms:description "Property. NGSI Entity type. It has to be StreetlightControlCabinet";
    rdf:type rdf:Property;
    rdfs:label "type";
    rdfs:domain <https://smart-data-models.github.io/dataModel.Streetlighting/StreetlightControlCabinet/schema.json>.
sdm:Type rdf:type skos:ConceptScheme.
sdm:type rdfs:range [
  owl:oneOf (sdm:StreetlightControlCabinet)
].
sdm:StreetlightControlCabinet rdf:type skos:Concept;
    skos:inScheme sdm:Type;
    rdfs:label "StreetlightControlCabinet".
sdm:serialNumber dcterms:description "Property. Model:'https://schema.org/serialNumber'. Serial number of the container.";
    rdf:type rdf:Property;
    rdfs:label "serialNumber";
    rdfs:domain <https://smart-data-models.github.io/dataModel.Streetlighting/StreetlightControlCabinet/schema.json>;
    rdfs:range xsd:string.
sdm:refStreetlightGroup rdf:type rdf:Property;
    rdfs:label "refStreetlightGroup";
    rdfs:domain <https://smart-data-models.github.io/dataModel.Streetlighting/StreetlightControlCabinet/schema.json>.
sdm:brandName dcterms:description "Property. Name of the cabinet's brand. Model:'https://schema.org/brand'";
    rdf:type rdf:Property;
    rdfs:label "brandName";
    rdfs:domain <https://smart-data-models.github.io/dataModel.Streetlighting/StreetlightControlCabinet/schema.json>;
    rdfs:range xsd:string.
sdm:modelName dcterms:description "Property. Name of the cabinet's model. Model:'https://schema.org/model'";
    rdf:type rdf:Property;
    rdfs:label "modelName";
    rdfs:domain <https://smart-data-models.github.io/dataModel.Streetlighting/StreetlightControlCabinet/schema.json>;
    rdfs:range xsd:string.
sdm:manufacturerName dcterms:description "Property. Name of the cabinet's manufacturer. Model:'https://schema.org/manufacturer'";
    rdf:type rdf:Property;
    rdfs:label "manufacturerName";
    rdfs:domain <https://smart-data-models.github.io/dataModel.Streetlighting/StreetlightControlCabinet/schema.json>;
    rdfs:range xsd:string.
sdm:cupboardMadeOf dcterms:description "Property. Material the cabinet's cupboard is made of. Enum:'concrete, metal, other, plastic'";
    rdf:type rdf:Property;
    rdfs:label "cupboardMadeOf";
    rdfs:domain <https://smart-data-models.github.io/dataModel.Streetlighting/StreetlightControlCabinet/schema.json>.
sdm:CupboardMadeOf rdf:type skos:ConceptScheme.
sdm:cupboardMadeOf rdfs:range [
  owl:oneOf (sdm:concrete sdm:metal sdm:other sdm:plastic)
].
sdm:concrete rdf:type skos:Concept;
    skos:inScheme sdm:CupboardMadeOf;
    rdfs:label "concrete".
sdm:metal rdf:type skos:Concept;
    skos:inScheme sdm:CupboardMadeOf;
    rdfs:label "metal".
sdm:other rdf:type skos:Concept;
    skos:inScheme sdm:CupboardMadeOf;
    rdfs:label "other".
sdm:plastic rdf:type skos:Concept;
    skos:inScheme sdm:CupboardMadeOf;
    rdfs:label "plastic".
sdm:features rdf:type rdf:Property;
    rdfs:label "features";
    rdfs:domain <https://smart-data-models.github.io/dataModel.Streetlighting/StreetlightControlCabinet/schema.json>.
sdm:Features rdf:type skos:ConceptScheme.
sdm:features rdfs:range [
  owl:oneOf (sdm:astronomicalClock sdm:individualControl)
].
sdm:astronomicalClock rdf:type skos:Concept;
    skos:inScheme sdm:Features;
    rdfs:label "astronomicalClock".
sdm:individualControl rdf:type skos:Concept;
    skos:inScheme sdm:Features;
    rdfs:label "individualControl".
sdm:compliantWith rdf:type rdf:Property;
    rdfs:label "compliantWith";
    rdfs:domain <https://smart-data-models.github.io/dataModel.Streetlighting/StreetlightControlCabinet/schema.json>;
    rdfs:range xsd:string.
sdm:annotations rdf:type rdf:Property;
    rdfs:label "annotations";
    rdfs:domain <https://smart-data-models.github.io/dataModel.Streetlighting/StreetlightControlCabinet/schema.json>;
    rdfs:range xsd:string.
sdm:refDevice rdf:type rdf:Property;
    rdfs:label "refDevice";
    rdfs:domain <https://smart-data-models.github.io/dataModel.Streetlighting/StreetlightControlCabinet/schema.json>.
sdm:dateServiceStarted dcterms:description "Property. Date at which the cabinet controller started giving service. Model:'https://schema.org/DateTime'";
    rdf:type rdf:Property;
    rdfs:label "dateServiceStarted";
    rdfs:domain <https://smart-data-models.github.io/dataModel.Streetlighting/StreetlightControlCabinet/schema.json>;
    rdfs:range xsd:dateTime.
sdm:dateLastProgramming dcterms:description "Property. Date at which there was a programming operation over the cabinet. Model:'https://schema.org/DateTime'";
    rdf:type rdf:Property;
    rdfs:label "dateLastProgramming";
    rdfs:domain <https://smart-data-models.github.io/dataModel.Streetlighting/StreetlightControlCabinet/schema.json>;
    rdfs:range xsd:dateTime.
sdm:nextActuationDeadline dcterms:description "Property. Deadline for next actuation to be performed (programming, testing, etc.). Model:'https://schema.org/DateTime'";
    rdf:type rdf:Property;
    rdfs:label "nextActuationDeadline";
    rdfs:domain <https://smart-data-models.github.io/dataModel.Streetlighting/StreetlightControlCabinet/schema.json>;
    rdfs:range xsd:dateTime.
sdm:responsible dcterms:description "Property. Responsible for the cabinet controller, i.e. entity in charge of actuating (programming, etc.).";
    rdf:type rdf:Property;
    rdfs:label "responsible";
    rdfs:domain <https://smart-data-models.github.io/dataModel.Streetlighting/StreetlightControlCabinet/schema.json>;
    rdfs:range xsd:string.
sdm:workingMode dcterms:description "Property. Working mode for this cabinet controller.  `automatic` : The cabinet controller decides automatically when light groups are switched on and off. Manual operation is not allowed. `manual` : Human intervention is required for switching on and off. `semiautomatic` : The same as `automatic` but in this case manual intervention is allowed.";
    rdf:type rdf:Property;
    rdfs:label "workingMode";
    rdfs:domain <https://smart-data-models.github.io/dataModel.Streetlighting/StreetlightControlCabinet/schema.json>.
sdm:WorkingMode rdf:type skos:ConceptScheme.
sdm:workingMode rdfs:range [
  owl:oneOf (sdm:automatic sdm:manual sdm:semiautomatic)
].
sdm:automatic rdf:type skos:Concept;
    skos:inScheme sdm:WorkingMode;
    rdfs:label "automatic".
sdm:manual rdf:type skos:Concept;
    skos:inScheme sdm:WorkingMode;
    rdfs:label "manual".
sdm:semiautomatic rdf:type skos:Concept;
    skos:inScheme sdm:WorkingMode;
    rdfs:label "semiautomatic".
sdm:description dcterms:description "Property. Timestamp of the last change of lamp made";
    rdf:type rdf:Property;
    rdfs:label "description";
    rdfs:domain <https://smart-data-models.github.io/dataModel.Streetlighting/StreetlightControlCabinet/schema.json>;
    rdfs:range xsd:string.
sdm:maximumPowerAvailable dcterms:description "Property. The maximum power available (by contract) for the circuits controlled by this cabinet. Units:'Kilowatts (kW)'";
    rdf:type rdf:Property;
    rdfs:label "maximumPowerAvailable";
    rdfs:domain <https://smart-data-models.github.io/dataModel.Streetlighting/StreetlightControlCabinet/schema.json>;
    rdfs:range xsd:decimal.
sdm:energyConsumed dcterms:description "Property. Energy consumed by the circuits controlled since metering started (since dateMeteringStarted). Units:'Kilowatts per hour (kWh)'. Model:'https://schema.org/Number'";
    rdf:type rdf:Property;
    rdfs:label "energyConsumed";
    rdfs:domain <https://smart-data-models.github.io/dataModel.Streetlighting/StreetlightControlCabinet/schema.json>;
    rdfs:range xsd:decimal.
sdm:energyCost dcterms:description "Property. Cost of the energy consumed by the circuits controlled since the metering start date. Model:'https://schema.org/Number'";
    rdf:type rdf:Property;
    rdfs:label "energyCost";
    rdfs:domain <https://smart-data-models.github.io/dataModel.Streetlighting/StreetlightControlCabinet/schema.json>;
    rdfs:range xsd:decimal.
sdm:reactiveEnergyConsumed dcterms:description "Property. Energy consumed (with regards to reactive power) by circuits since the metering start date. Model:'https://schema.org/Number'. Units:'KiloVolts-Ampere-Reactive per hour (kVArh)'";
    rdf:type rdf:Property;
    rdfs:label "reactiveEnergyConsumed";
    rdfs:domain <https://smart-data-models.github.io/dataModel.Streetlighting/StreetlightControlCabinet/schema.json>;
    rdfs:range xsd:decimal.
sdm:dateMeteringStarted dcterms:description "Property. The starting date for metering energy consumed. Model:'https://schema.org/DateTime'";
    rdf:type rdf:Property;
    rdfs:label "dateMeteringStarted";
    rdfs:domain <https://smart-data-models.github.io/dataModel.Streetlighting/StreetlightControlCabinet/schema.json>;
    rdfs:range xsd:dateTime.
sdm:lastMeterReading dcterms:description "Property. Value of the last reading obtained from the energy consumed metering system. Model:'https://schema.org/DateTime'. Units:'Kilowatts per hour (kWh)'";
    rdf:type rdf:Property;
    rdfs:label "lastMeterReading";
    rdfs:domain <https://smart-data-models.github.io/dataModel.Streetlighting/StreetlightControlCabinet/schema.json>;
    rdfs:range xsd:decimal.
sdm:meterReadingPeriod dcterms:description "Property. The periodicity of energy consumed meter readings in days. Model:'http://schema.org/Number'";
    rdf:type rdf:Property;
    rdfs:label "meterReadingPeriod";
    rdfs:domain <https://smart-data-models.github.io/dataModel.Streetlighting/StreetlightControlCabinet/schema.json>;
    rdfs:range xsd:decimal.
sdm:frequency dcterms:description "Property. The working frequency of the circuit. Units:'Hertz (Hz)'";
    rdf:type rdf:Property;
    rdfs:label "frequency";
    rdfs:domain <https://smart-data-models.github.io/dataModel.Streetlighting/StreetlightControlCabinet/schema.json>;
    rdfs:range xsd:decimal.
sdm:totalActivePower dcterms:description "Property. Active power currently consumed (counting all phases). Units:'KiloWatts (kW)'";
    rdf:type rdf:Property;
    rdfs:label "totalActivePower";
    rdfs:domain <https://smart-data-models.github.io/dataModel.Streetlighting/StreetlightControlCabinet/schema.json>;
    rdfs:range xsd:decimal.
sdm:totalReactivePower dcterms:description "Property. Reactive power currently consumed (counting all phases). Units:'KiloVolts-Ampere-Reactive (kVArh)'";
    rdf:type rdf:Property;
    rdfs:label "totalReactivePower";
    rdfs:domain <https://smart-data-models.github.io/dataModel.Streetlighting/StreetlightControlCabinet/schema.json>;
    rdfs:range xsd:decimal.
sdm:activePowerR dcterms:description "Property. Active power consumed in R phase. Units:'Kilowatts (kW)'. Model:'http://schema.org/Number'";
    rdf:type rdf:Property;
    rdfs:label "activePowerR";
    rdfs:domain <https://smart-data-models.github.io/dataModel.Streetlighting/StreetlightControlCabinet/schema.json>;
    rdfs:range xsd:decimal.
sdm:activePowerS dcterms:description "Property. Active power consumed in S phase. Units:'Kilowatts (kW)'. Model:'http://schema.org/Number'";
    rdf:type rdf:Property;
    rdfs:label "activePowerS";
    rdfs:domain <https://smart-data-models.github.io/dataModel.Streetlighting/StreetlightControlCabinet/schema.json>;
    rdfs:range xsd:decimal.
sdm:activePowerT dcterms:description "Property. Active power consumed in T phase. Units:'Kilowatts (kW)'. Model:'http://schema.org/Number'";
    rdf:type rdf:Property;
    rdfs:label "activePowerT";
    rdfs:domain <https://smart-data-models.github.io/dataModel.Streetlighting/StreetlightControlCabinet/schema.json>;
    rdfs:range xsd:decimal.
sdm:reactivePowerR dcterms:description "Property. Reactive power in R phase. Units:'KiloVolts-Ampere-Reactive (kVArh)'. Model:'http://schema.org/Number'";
    rdf:type rdf:Property;
    rdfs:label "reactivePowerR";
    rdfs:domain <https://smart-data-models.github.io/dataModel.Streetlighting/StreetlightControlCabinet/schema.json>;
    rdfs:range xsd:decimal.
sdm:reactivePowerS dcterms:description "Property. Reactive power in S phase. Units:'KiloVolts-Ampere-Reactive (kVArh)'. Model:'http://schema.org/Number'";
    rdf:type rdf:Property;
    rdfs:label "reactivePowerS";
    rdfs:domain <https://smart-data-models.github.io/dataModel.Streetlighting/StreetlightControlCabinet/schema.json>;
    rdfs:range xsd:decimal.
sdm:reactivePowerT dcterms:description "Property. Reactive power in T phase. Units:'KiloVolts-Ampere-Reactive (kVArh)'. Model:'http://schema.org/Number'";
    rdf:type rdf:Property;
    rdfs:label "reactivePowerT";
    rdfs:domain <https://smart-data-models.github.io/dataModel.Streetlighting/StreetlightControlCabinet/schema.json>;
    rdfs:range xsd:decimal.
sdm:powerFactorR dcterms:description "Property. Power factor for phase R. Allowed values: A number between -1 and 1. Model:'http://schema.org/Number'";
    rdf:type rdf:Property;
    rdfs:label "powerFactorR";
    rdfs:domain <https://smart-data-models.github.io/dataModel.Streetlighting/StreetlightControlCabinet/schema.json>;
    rdfs:range xsd:decimal.
sdm:powerFactorS dcterms:description "Property. Power factor for phase S. Allowed values: A number between -1 and 1. Model:'http://schema.org/Number'";
    rdf:type rdf:Property;
    rdfs:label "powerFactorS";
    rdfs:domain <https://smart-data-models.github.io/dataModel.Streetlighting/StreetlightControlCabinet/schema.json>;
    rdfs:range xsd:decimal.
sdm:powerFactorT dcterms:description "Property. Power factor for phase T. Allowed values: A number between -1 and 1. Model:'http://schema.org/Number'";
    rdf:type rdf:Property;
    rdfs:label "powerFactorT";
    rdfs:domain <https://smart-data-models.github.io/dataModel.Streetlighting/StreetlightControlCabinet/schema.json>;
    rdfs:range xsd:decimal.
sdm:cosPhi dcterms:description "Property. Cosine of phi parameter. Model:'https://schema.org/Number'";
    rdf:type rdf:Property;
    rdfs:label "cosPhi";
    rdfs:domain <https://smart-data-models.github.io/dataModel.Streetlighting/StreetlightControlCabinet/schema.json>;
    rdfs:range xsd:decimal.
sdm:intensityR dcterms:description "Property. Electric intensity in R phase. Units:'Ampers (A)'. Model:'http://schema.org/Number'";
    rdf:type rdf:Property;
    rdfs:label "intensityR";
    rdfs:domain <https://smart-data-models.github.io/dataModel.Streetlighting/StreetlightControlCabinet/schema.json>;
    rdfs:range xsd:decimal.
sdm:intensityS dcterms:description "Property. Electric intensity in S phase. Units:'Ampers (A)'. Model:'http://schema.org/Number'";
    rdf:type rdf:Property;
    rdfs:label "intensityS";
    rdfs:domain <https://smart-data-models.github.io/dataModel.Streetlighting/StreetlightControlCabinet/schema.json>;
    rdfs:range xsd:decimal.
sdm:intensityT dcterms:description "Property.  Electric intensity in T phase. Units:'Ampers (A)'. Model:'http://schema.org/Number'";
    rdf:type rdf:Property;
    rdfs:label "intensityT";
    rdfs:domain <https://smart-data-models.github.io/dataModel.Streetlighting/StreetlightControlCabinet/schema.json>;
    rdfs:range xsd:decimal.
sdm:voltageR dcterms:description "Property. Electric tension in phase R. Units:'Volts (V)'. Model:'http://schema.org/Number'";
    rdf:type rdf:Property;
    rdfs:label "voltageR";
    rdfs:domain <https://smart-data-models.github.io/dataModel.Streetlighting/StreetlightControlCabinet/schema.json>;
    rdfs:range xsd:decimal.
sdm:voltageS dcterms:description "Property. Electric tension in phase S. Units:'Volts (V)'. Model:'http://schema.org/Number'";
    rdf:type rdf:Property;
    rdfs:label "voltageS";
    rdfs:domain <https://smart-data-models.github.io/dataModel.Streetlighting/StreetlightControlCabinet/schema.json>;
    rdfs:range xsd:decimal.
sdm:voltageT dcterms:description "Property. Electric tension in phase T. Units:'Volts (V)'. Model:'http://schema.org/Number'";
    rdf:type rdf:Property;
    rdfs:label "voltageT";
    rdfs:domain <https://smart-data-models.github.io/dataModel.Streetlighting/StreetlightControlCabinet/schema.json>;
    rdfs:range xsd:decimal.
sdm:thdrVoltageR dcterms:description "Property. Total harmonic distortion (R) of voltage in phase R. Allowed values: A number between 0 and 1. Model:'http://schema.org/Number'";
    rdf:type rdf:Property;
    rdfs:label "thdrVoltageR";
    rdfs:domain <https://smart-data-models.github.io/dataModel.Streetlighting/StreetlightControlCabinet/schema.json>;
    rdfs:range xsd:decimal.
sdm:thdrVoltageS dcterms:description "Property. Total harmonic distortion (S) of voltage in phase S. Allowed values: A number between 0 and 1. Model:'http://schema.org/Number'";
    rdf:type rdf:Property;
    rdfs:label "thdrVoltageS";
    rdfs:domain <https://smart-data-models.github.io/dataModel.Streetlighting/StreetlightControlCabinet/schema.json>;
    rdfs:range xsd:decimal.
sdm:thdrVoltageT dcterms:description "Property. Total harmonic distortion (T) of voltage in phase T. Allowed values: A number between 0 and 1. Model:'http://schema.org/Number'";
    rdf:type rdf:Property;
    rdfs:label "thdrVoltageT";
    rdfs:domain <https://smart-data-models.github.io/dataModel.Streetlighting/StreetlightControlCabinet/schema.json>;
    rdfs:range xsd:decimal.
sdm:thdrIntensityR dcterms:description "Property. Total harmonic distortion (R) of intensity in phase R. Allowed values: A number between 0 and 1. Model:'http://schema.org/Number'";
    rdf:type rdf:Property;
    rdfs:label "thdrIntensityR";
    rdfs:domain <https://smart-data-models.github.io/dataModel.Streetlighting/StreetlightControlCabinet/schema.json>;
    rdfs:range xsd:decimal.
sdm:thdrIntensityS dcterms:description "Property. Total harmonic distortion (S) of intensity in phase S. Allowed values: A number between 0 and 1. Model:'http://schema.org/Number'";
    rdf:type rdf:Property;
    rdfs:label "thdrIntensityS";
    rdfs:domain <https://smart-data-models.github.io/dataModel.Streetlighting/StreetlightControlCabinet/schema.json>;
    rdfs:range xsd:decimal.
sdm:thdrIntensityT dcterms:description "Property. Total harmonic distortion (T) of intensity in phase T. Allowed values: A number between 0 and 1. Model:'http://schema.org/Number'";
    rdf:type rdf:Property;
    rdfs:label "thdrIntensityT";
    rdfs:domain <https://smart-data-models.github.io/dataModel.Streetlighting/StreetlightControlCabinet/schema.json>;
    rdfs:range xsd:decimal.
