@prefix schema: <https://schema.org/>.
@prefix skos: <http://www.w3.org/2004/02/skos/core#>.
@prefix rdf: <http://www.w3.org/1999/02/22-rdf-syntax-ns#>.
@prefix rdfs: <http://www.w3.org/2000/01/rdf-schema#>.
@prefix foaf: <http://xmlns.com/foaf/0.1/>.
@prefix xsd: <http://www.w3.org/2001/XMLSchema#>.
@prefix dcterms: <http://purl.org/dc/terms/>.
@prefix owl: <http://www.w3.org/2002/07/owl#>.
@prefix jsonsc: <https://www.w3.org/2019/wot/json-schema#>.
@prefix jsonsc-ld: <http://w3id.org/jsonsc-ld/>.
@prefix api: <http://purl.org/linked-data/api/vocab>.
@prefix geo: <http://www.w3.org/2003/01/geo/wgs84_pos#>.
@prefix mobivoc: <http://schema.mobivoc.org/#>.
@prefix geosparql: <http://www.opengis.net/ont/geosparql#>.
@prefix sdm: <https://w3id.org/sdm#>.

<https://smart-data-models.github.io/dataModel.UnmannedAerialVehicle/UnmannedAerialVehicleTMS/schema.json> dcterms:title "Smart Data models - UAV-Traffic Management Software schema";
    dcterms:description "This entity contains a harmonized description of a specific Unmanned Aerial Vehicle (UAV) Traffic Management Software Application that is designed to listen to and monitor the information transmitted by UAVâ€™s, typically this software application would be operated at a ground station. This entity is primarily associated with UAV command and control applications.".
sdm:type dcterms:description "Property. NGSI Entity identifier. It has to be UnmannedAerialVehicleTMS";
    rdf:type rdf:Property;
    rdfs:label "type";
    rdfs:domain <https://smart-data-models.github.io/dataModel.UnmannedAerialVehicle/UnmannedAerialVehicleTMS/schema.json>.
sdm:Type rdf:type skos:ConceptScheme.
sdm:type rdfs:range [
  owl:oneOf (sdm:UnmannedAerialVehicleTMS)
].
sdm:UnmannedAerialVehicleTMS rdf:type skos:Concept;
    skos:inScheme sdm:Type;
    rdfs:label "UnmannedAerialVehicleTMS".
sdm:softwareApplication dcterms:description "Property. Details about the software application using the Schema.org definition Model:'https://schema.org/SoftwareApplication'. ";
    rdf:type rdf:Property;
    rdfs:label "softwareApplication";
    rdfs:domain <https://smart-data-models.github.io/dataModel.UnmannedAerialVehicle/UnmannedAerialVehicleTMS/schema.json>;
    rdfs:range sdm:SoftwareApplication.
sdm:SoftwareApplication rdf:type rdfs:Class;
    rdfs:label "SoftwareApplication".
sdm:operatingSystem rdf:type rdf:Property;
    rdfs:label "operatingSystem";
    rdfs:domain sdm:SoftwareApplication;
    rdfs:range xsd:string.
sdm:softwareVersion rdf:type rdf:Property;
    rdfs:label "softwareVersion";
    rdfs:domain sdm:SoftwareApplication;
    rdfs:range xsd:string.
sdm:applicationCategory rdf:type rdf:Property;
    rdfs:label "applicationCategory";
    rdfs:domain sdm:SoftwareApplication;
    rdfs:range xsd:string.
sdm:operationalInstance dcterms:description "Property. URL linking to an operational instance (assumed to be web based) for the UAV Traffic Management Software.";
    rdf:type rdf:Property;
    rdfs:label "operationalInstance";
    rdfs:domain <https://smart-data-models.github.io/dataModel.UnmannedAerialVehicle/UnmannedAerialVehicleTMS/schema.json>;
    rdfs:range xsd:anyURI.
