@prefix schema: <https://schema.org/>.
@prefix skos: <http://www.w3.org/2004/02/skos/core#>.
@prefix rdf: <http://www.w3.org/1999/02/22-rdf-syntax-ns#>.
@prefix rdfs: <http://www.w3.org/2000/01/rdf-schema#>.
@prefix foaf: <http://xmlns.com/foaf/0.1/>.
@prefix xsd: <http://www.w3.org/2001/XMLSchema#>.
@prefix dcterms: <http://purl.org/dc/terms/>.
@prefix owl: <http://www.w3.org/2002/07/owl#>.
@prefix jsonsc: <https://www.w3.org/2019/wot/json-schema#>.
@prefix jsonsc-ld: <http://w3id.org/jsonsc-ld/>.
@prefix api: <http://purl.org/linked-data/api/vocab>.
@prefix geo: <http://www.w3.org/2003/01/geo/wgs84_pos#>.
@prefix mobivoc: <http://schema.mobivoc.org/#>.
@prefix geosparql: <http://www.opengis.net/ont/geosparql#>.
@prefix sdm: <https://w3id.org/sdm#>.

<https://smart-data-models.github.io/dataModel.ManufacturingMachine/ManufacturingMachine/schema.json> dcterms:title "Smart Data models - Manufacturing Machine dataModel schema,";
    dcterms:description "Description of a generic machine".
sdm:type dcterms:description "Property. NGSI entity type. It has to be ManufacturingMachine.";
    rdf:type rdf:Property;
    rdfs:label "type";
    rdfs:domain <https://smart-data-models.github.io/dataModel.ManufacturingMachine/ManufacturingMachine/schema.json>.
sdm:Type rdf:type skos:ConceptScheme.
sdm:type rdfs:range [
  owl:oneOf (sdm:ManufacturingMachine)
].
sdm:ManufacturingMachine rdf:type skos:Concept;
    skos:inScheme sdm:Type;
    rdfs:label "ManufacturingMachine".
sdm:machineModel dcterms:description "Relationship. A reference to the associated Machine Model for this machine.";
    rdf:type rdf:Property;
    rdfs:label "machineModel";
    rdfs:domain <https://smart-data-models.github.io/dataModel.ManufacturingMachine/ManufacturingMachine/schema.json>.
sdm:serialNumber dcterms:description "Property. Model:'https://schema.org/Text'. The serial number assigned by the manufacturer.";
    rdf:type rdf:Property;
    rdfs:label "serialNumber";
    rdfs:domain <https://smart-data-models.github.io/dataModel.ManufacturingMachine/ManufacturingMachine/schema.json>;
    rdfs:range xsd:string.
sdm:assetIdentifier dcterms:description "Property. Model:'https://schema.org/Text'. An asset identifier (e.g. asset tag number) assigned by the owner.";
    rdf:type rdf:Property;
    rdfs:label "assetIdentifier";
    rdfs:domain <https://smart-data-models.github.io/dataModel.ManufacturingMachine/ManufacturingMachine/schema.json>;
    rdfs:range xsd:string.
sdm:supplierName dcterms:description "Property. Model:'https://schema.org/Text'. The name of the supplier of this machine.";
    rdf:type rdf:Property;
    rdfs:label "supplierName";
    rdfs:domain <https://smart-data-models.github.io/dataModel.ManufacturingMachine/ManufacturingMachine/schema.json>;
    rdfs:range xsd:string.
sdm:countryOfManufacture dcterms:description "Property. Model:'https://schema.org/Text'. The country where this machine was manufactured.";
    rdf:type rdf:Property;
    rdfs:label "countryOfManufacture";
    rdfs:domain <https://smart-data-models.github.io/dataModel.ManufacturingMachine/ManufacturingMachine/schema.json>;
    rdfs:range xsd:string.
sdm:factory dcterms:description "Property. Model:'https://schema.org/Text'. The factory name/code manufacturing this machine.";
    rdf:type rdf:Property;
    rdfs:label "factory";
    rdfs:domain <https://smart-data-models.github.io/dataModel.ManufacturingMachine/ManufacturingMachine/schema.json>;
    rdfs:range xsd:string.
sdm:firstUsedAt dcterms:description "Property. Model:'https://schema.org/Text'. Indicates the date/time at which date and time the machine was first used (nominally in UTC).";
    rdf:type rdf:Property;
    rdfs:label "firstUsedAt";
    rdfs:domain <https://smart-data-models.github.io/dataModel.ManufacturingMachine/ManufacturingMachine/schema.json>;
    rdfs:range xsd:dateTime.
sdm:installedAt dcterms:description "Property. Model:'https://schema.org/Text'. Indicates the date/time at which date and time the machine was installed (nominally in UTC).";
    rdf:type rdf:Property;
    rdfs:label "installedAt";
    rdfs:domain <https://smart-data-models.github.io/dataModel.ManufacturingMachine/ManufacturingMachine/schema.json>;
    rdfs:range xsd:dateTime.
sdm:manufacturedAt dcterms:description "Property. Model:'https://schema.org/Text'. Indicates the date/time at which date and time the machine was manufactured (nominally in UTC).";
    rdf:type rdf:Property;
    rdfs:label "manufacturedAt";
    rdfs:domain <https://smart-data-models.github.io/dataModel.ManufacturingMachine/ManufacturingMachine/schema.json>;
    rdfs:range xsd:dateTime.
sdm:machineOwner rdf:type rdf:Property;
    rdfs:label "machineOwner";
    rdfs:domain <https://smart-data-models.github.io/dataModel.ManufacturingMachine/ManufacturingMachine/schema.json>.
sdm:hardwareVersion dcterms:description "Property. Model:'https://schema.org/Text'. The (manufacturer specific) hardware version of this machine.";
    rdf:type rdf:Property;
    rdfs:label "hardwareVersion";
    rdfs:domain <https://smart-data-models.github.io/dataModel.ManufacturingMachine/ManufacturingMachine/schema.json>;
    rdfs:range xsd:string.
sdm:firmwareVersion dcterms:description "Property. Model:'https://schema.org/Text'. The (manufacturer specific) firmware version of this machine.";
    rdf:type rdf:Property;
    rdfs:label "firmwareVersion";
    rdfs:domain <https://smart-data-models.github.io/dataModel.ManufacturingMachine/ManufacturingMachine/schema.json>;
    rdfs:range xsd:string.
sdm:softwareVersion dcterms:description "Property. Model:'https://schema.org/Text'. The (manufacturer specific) software version of this machine.";
    rdf:type rdf:Property;
    rdfs:label "softwareVersion";
    rdfs:domain <https://smart-data-models.github.io/dataModel.ManufacturingMachine/ManufacturingMachine/schema.json>;
    rdfs:range xsd:string.
sdm:osVersion dcterms:description "Property. Model:'https://schema.org/Text'. The (manufacturer specific) operating system version of this machine";
    rdf:type rdf:Property;
    rdfs:label "osVersion";
    rdfs:domain <https://smart-data-models.github.io/dataModel.ManufacturingMachine/ManufacturingMachine/schema.json>;
    rdfs:range xsd:string.
sdm:supportedProtocol rdf:type rdf:Property;
    rdfs:label "supportedProtocol";
    rdfs:domain <https://smart-data-models.github.io/dataModel.ManufacturingMachine/ManufacturingMachine/schema.json>;
    rdfs:range xsd:string.
sdm:building dcterms:description "Relationship. Reference to the building entity instance into which this machine is installed";
    rdf:type rdf:Property;
    rdfs:label "building";
    rdfs:domain <https://smart-data-models.github.io/dataModel.ManufacturingMachine/ManufacturingMachine/schema.json>.
sdm:subscriptionService rdf:type rdf:Property;
    rdfs:label "subscriptionService";
    rdfs:domain <https://smart-data-models.github.io/dataModel.ManufacturingMachine/ManufacturingMachine/schema.json>.
sdm:online dcterms:description "Property. Model:'https://schema.org/Boolean'. The communication status of this machine. A logical representation of Offline (false) or Online (true).";
    rdf:type rdf:Property;
    rdfs:label "online";
    rdfs:domain <https://smart-data-models.github.io/dataModel.ManufacturingMachine/ManufacturingMachine/schema.json>;
    rdfs:range xsd:boolean.
sdm:status dcterms:description "Property. Model:'https://schema.org/Text'. Text formatted (current) machine status code or description. Expected to be the manufacturer or machine specific status code generated by the machine.";
    rdf:type rdf:Property;
    rdfs:label "status";
    rdfs:domain <https://smart-data-models.github.io/dataModel.ManufacturingMachine/ManufacturingMachine/schema.json>;
    rdfs:range xsd:string.
sdm:batteryLevel dcterms:description "Property. Model:'https://schema.org/Number'. Battery level. It must be equal to: 1.0 When the battery charge is full. 0.0 When the battery charge empty. Null when it cannot be determined.";
    rdf:type rdf:Property;
    rdfs:label "batteryLevel";
    rdfs:domain <https://smart-data-models.github.io/dataModel.ManufacturingMachine/ManufacturingMachine/schema.json>;
    rdfs:range xsd:decimal.
sdm:installationNotes dcterms:description "Property. Model:'https://schema.org/Text'. Notes relating to this machine installation.";
    rdf:type rdf:Property;
    rdfs:label "installationNotes";
    rdfs:domain <https://smart-data-models.github.io/dataModel.ManufacturingMachine/ManufacturingMachine/schema.json>;
    rdfs:range sdm:InstallationNote.
sdm:InstallationNote rdf:type rdfs:Class;
    rdfs:label "InstallationNote".
sdm:docUri rdf:type rdf:Property;
    rdfs:label "docUri";
    rdfs:domain sdm:InstallationNote;
    rdfs:range xsd:anyURI.
sdm:value rdf:type rdf:Property;
    rdfs:label "value";
    rdfs:domain sdm:InstallationNote;
    rdfs:range xsd:string.
sdm:voltage dcterms:description "Property. Model:'https://schema.org/Number'. The nominal required supply voltage, in volts. Units:'Volts";
    rdf:type rdf:Property;
    rdfs:label "voltage";
    rdfs:domain <https://smart-data-models.github.io/dataModel.ManufacturingMachine/ManufacturingMachine/schema.json>;
    rdfs:range xsd:decimal.
sdm:current dcterms:description "Property. Model:'https://schema.org/Number'. The nominal required supply current (at the nominal supply voltage), in amps. Units:'Amps";
    rdf:type rdf:Property;
    rdfs:label "current";
    rdfs:domain <https://smart-data-models.github.io/dataModel.ManufacturingMachine/ManufacturingMachine/schema.json>;
    rdfs:range xsd:decimal.
sdm:power dcterms:description "Property. Model:'https://schema.org/Number'. The nominal rated power consumption of the machine in kW. Units:'Kw";
    rdf:type rdf:Property;
    rdfs:label "power";
    rdfs:domain <https://smart-data-models.github.io/dataModel.ManufacturingMachine/ManufacturingMachine/schema.json>;
    rdfs:range xsd:decimal.
sdm:rotationalSpeed dcterms:description "Property. Model:'https://schema.org/Number'.  \tThe maximum rotational speed in rpm (for machines such as drills, lathes). Units:'rpm";
    rdf:type rdf:Property;
    rdfs:label "rotationalSpeed";
    rdfs:domain <https://smart-data-models.github.io/dataModel.ManufacturingMachine/ManufacturingMachine/schema.json>;
    rdfs:range xsd:decimal.
