@prefix schema: <https://schema.org/>.
@prefix skos: <http://www.w3.org/2004/02/skos/core#>.
@prefix rdf: <http://www.w3.org/1999/02/22-rdf-syntax-ns#>.
@prefix rdfs: <http://www.w3.org/2000/01/rdf-schema#>.
@prefix foaf: <http://xmlns.com/foaf/0.1/>.
@prefix xsd: <http://www.w3.org/2001/XMLSchema#>.
@prefix dcterms: <http://purl.org/dc/terms/>.
@prefix owl: <http://www.w3.org/2002/07/owl#>.
@prefix jsonsc: <https://www.w3.org/2019/wot/json-schema#>.
@prefix jsonsc-ld: <http://w3id.org/jsonsc-ld/>.
@prefix api: <http://purl.org/linked-data/api/vocab>.
@prefix geo: <http://www.w3.org/2003/01/geo/wgs84_pos#>.
@prefix mobivoc: <http://schema.mobivoc.org/#>.
@prefix geosparql: <http://www.opengis.net/ont/geosparql#>.
@prefix sdm: <https://w3id.org/sdm#>.

<https://smart-data-models.github.io/dataModels.CIMEnergyClasses/SynchronousMachineDynamics/schema.json> dcterms:title " Smart Data Models - SynchronousMachineDynamics";
    dcterms:description "Adapted from CIM data models. Synchronous machine whose behaviour is described by reference to a standard model expressed in one of the following forms:".
sdm:type dcterms:description "Property. NGSI type. It has to be SynchronousMachineDynamics";
    rdf:type rdf:Property;
    rdfs:label "type";
    rdfs:domain <https://smart-data-models.github.io/dataModels.CIMEnergyClasses/SynchronousMachineDynamics/schema.json>.
sdm:Type rdf:type skos:ConceptScheme.
sdm:type rdfs:range [
  owl:oneOf (sdm:SynchronousMachineDynamics)
].
sdm:SynchronousMachineDynamics rdf:type skos:Concept;
    skos:inScheme sdm:Type;
    rdfs:label "SynchronousMachineDynamics".
sdm:ExcitationSystemDynamics dcterms:description "Property. Model:'https://schema.org/Number'. Excitation system model associated with this synchronous machine model. Default: None";
    rdf:type rdf:Property;
    rdfs:label "ExcitationSystemDynamics";
    rdfs:domain <https://smart-data-models.github.io/dataModels.CIMEnergyClasses/SynchronousMachineDynamics/schema.json>;
    rdfs:range xsd:decimal.
sdm:GenICompensationForGenJ dcterms:description "Property. Model:'https://schema.org/Number'. Compensation of voltage compensator`s generator for current flow out of this  generator. Default: 'list'";
    rdf:type rdf:Property;
    rdfs:label "GenICompensationForGenJ";
    rdfs:domain <https://smart-data-models.github.io/dataModels.CIMEnergyClasses/SynchronousMachineDynamics/schema.json>;
    rdfs:range xsd:decimal.
sdm:MechanicalLoadDynamics dcterms:description "Property. Model:'https://schema.org/Number'. Mechanical load model associated with this synchronous machine model. Default: None";
    rdf:type rdf:Property;
    rdfs:label "MechanicalLoadDynamics";
    rdfs:domain <https://smart-data-models.github.io/dataModels.CIMEnergyClasses/SynchronousMachineDynamics/schema.json>;
    rdfs:range xsd:decimal.
sdm:SynchronousMachine dcterms:description "Property. Model:'https://schema.org/Number'. Synchronous machine to which synchronous machine dynamics model applies. Default: None";
    rdf:type rdf:Property;
    rdfs:label "SynchronousMachine";
    rdfs:domain <https://smart-data-models.github.io/dataModels.CIMEnergyClasses/SynchronousMachineDynamics/schema.json>;
    rdfs:range xsd:decimal.
sdm:TurbineGovernorDynamics dcterms:description "Property. Model:'https://schema.org/Number'. Synchronous machine model with which this turbine-governor model is associated. Default: 'list'";
    rdf:type rdf:Property;
    rdfs:label "TurbineGovernorDynamics";
    rdfs:domain <https://smart-data-models.github.io/dataModels.CIMEnergyClasses/SynchronousMachineDynamics/schema.json>;
    rdfs:range xsd:decimal.
