@prefix schema: <https://schema.org/>.
@prefix skos: <http://www.w3.org/2004/02/skos/core#>.
@prefix rdf: <http://www.w3.org/1999/02/22-rdf-syntax-ns#>.
@prefix rdfs: <http://www.w3.org/2000/01/rdf-schema#>.
@prefix foaf: <http://xmlns.com/foaf/0.1/>.
@prefix xsd: <http://www.w3.org/2001/XMLSchema#>.
@prefix dcterms: <http://purl.org/dc/terms/>.
@prefix owl: <http://www.w3.org/2002/07/owl#>.
@prefix jsonsc: <https://www.w3.org/2019/wot/json-schema#>.
@prefix jsonsc-ld: <http://w3id.org/jsonsc-ld/>.
@prefix api: <http://purl.org/linked-data/api/vocab>.
@prefix geo: <http://www.w3.org/2003/01/geo/wgs84_pos#>.
@prefix mobivoc: <http://schema.mobivoc.org/#>.
@prefix geosparql: <http://www.opengis.net/ont/geosparql#>.
@prefix sdm: <https://w3id.org/sdm#>.

<https://smart-data-models.github.io/dataModel.Transportation/BikeHireDockingStation/schema.json> dcterms:title " - Transportation / Bike Hire Docking Station";
    dcterms:description "Bike Hire Docking Station".
sdm:type dcterms:description "Property. NGSI Entity type. It has to be BikeHireDockingStation";
    rdf:type rdf:Property;
    rdfs:label "type";
    rdfs:domain <https://smart-data-models.github.io/dataModel.Transportation/BikeHireDockingStation/schema.json>.
sdm:Type rdf:type skos:ConceptScheme.
sdm:type rdfs:range [
  owl:oneOf (sdm:BikeHireDockingStation)
].
sdm:BikeHireDockingStation rdf:type skos:Concept;
    skos:inScheme sdm:Type;
    rdfs:label "BikeHireDockingStation".
sdm:totalSlotNumber dcterms:description "Property. The total number of slots offered by this bike docking station. Model:'https://schema.org/Number'.";
    rdf:type rdf:Property;
    rdfs:label "totalSlotNumber";
    rdfs:domain <https://smart-data-models.github.io/dataModel.Transportation/BikeHireDockingStation/schema.json>;
    rdfs:range xsd:integer.
sdm:freeSlotNumber dcterms:description "Property. The number of slots available for returning and parking bikes. It must lower or equal than `totalSlotNumber`. Model:'https://schema.org/Number'.";
    rdf:type rdf:Property;
    rdfs:label "freeSlotNumber";
    rdfs:domain <https://smart-data-models.github.io/dataModel.Transportation/BikeHireDockingStation/schema.json>;
    rdfs:range xsd:integer.
sdm:availableBikeNumber dcterms:description "Property. The number of bikes available in the bike hire docking station to be hired by users. Model:'https://schema.org/Number'.";
    rdf:type rdf:Property;
    rdfs:label "availableBikeNumber";
    rdfs:domain <https://smart-data-models.github.io/dataModel.Transportation/BikeHireDockingStation/schema.json>;
    rdfs:range xsd:integer.
sdm:outOfServiceSlotNumber dcterms:description "Property. The number of slots that are out of order and cannot be used to hire or park a bike. It must lower or equal than `totalSlotNumber`. Model:'https://schema.org/Number'.";
    rdf:type rdf:Property;
    rdfs:label "outOfServiceSlotNumber";
    rdfs:domain <https://smart-data-models.github.io/dataModel.Transportation/BikeHireDockingStation/schema.json>;
    rdfs:range xsd:integer.
sdm:openingHours dcterms:description "Property. Opening hours of the docking station. Model:'http://schema.org/openingHours'.";
    rdf:type rdf:Property;
    rdfs:label "openingHours";
    rdfs:domain <https://smart-data-models.github.io/dataModel.Transportation/BikeHireDockingStation/schema.json>;
    rdfs:range xsd:string.
sdm:status dcterms:description "Property. Status of the bike hire docking station. Enum:'working, outOfService, withIncidence, full, almostFull, empty, almostEmpty'. Model:'https://schema.org/Number'. Or any other application specific.";
    rdf:type rdf:Property;
    rdfs:label "status";
    rdfs:domain <https://smart-data-models.github.io/dataModel.Transportation/BikeHireDockingStation/schema.json>.
sdm:Status rdf:type skos:ConceptScheme.
sdm:status rdfs:range [
  owl:oneOf (sdm:almostEmpty sdm:almostFull sdm:empty sdm:full sdm:outOfService sdm:withIncidence sdm:working)
].
sdm:almostEmpty rdf:type skos:Concept;
    skos:inScheme sdm:Status;
    rdfs:label "almostEmpty".
sdm:almostFull rdf:type skos:Concept;
    skos:inScheme sdm:Status;
    rdfs:label "almostFull".
sdm:empty rdf:type skos:Concept;
    skos:inScheme sdm:Status;
    rdfs:label "empty".
sdm:full rdf:type skos:Concept;
    skos:inScheme sdm:Status;
    rdfs:label "full".
sdm:outOfService rdf:type skos:Concept;
    skos:inScheme sdm:Status;
    rdfs:label "outOfService".
sdm:withIncidence rdf:type skos:Concept;
    skos:inScheme sdm:Status;
    rdfs:label "withIncidence".
sdm:working rdf:type skos:Concept;
    skos:inScheme sdm:Status;
    rdfs:label "working".
sdm:provider dcterms:description "Property. Bike hire service provider. Model:'https://schema.org/provider'.";
    rdf:type rdf:Property;
    rdfs:label "provider";
    rdfs:domain <https://smart-data-models.github.io/dataModel.Transportation/BikeHireDockingStation/schema.json>;
    rdfs:range xsd:string.
sdm:stationName dcterms:description "Property. Model:'https://schema.org/Text'. The name of the bike hire docking station corresponding to this observation.";
    rdf:type rdf:Property;
    rdfs:label "stationName";
    rdfs:domain <https://smart-data-models.github.io/dataModel.Transportation/BikeHireDockingStation/schema.json>;
    rdfs:range xsd:string.
sdm:mediaURL dcterms:description "Property. Model:'https://schema.org/Text'. URL providing further information of any image(s) or media of the complaint or place.";
    rdf:type rdf:Property;
    rdfs:label "mediaURL";
    rdfs:domain <https://smart-data-models.github.io/dataModel.Transportation/BikeHireDockingStation/schema.json>;
    rdfs:range xsd:anyURI.
sdm:agency_url dcterms:description "Property. Model:'https://schema.org/Text'. The agency_url field contains the URL of the transit agency. SameAs: 'agency_url' field from GTFS Static Field Definition - agency.txt (https://developers.google.com/transit/gtfs/reference#agencytxt)";
    rdf:type rdf:Property;
    rdfs:label "agency_url";
    rdfs:domain <https://smart-data-models.github.io/dataModel.Transportation/BikeHireDockingStation/schema.json>;
    rdfs:range xsd:anyURI.
sdm:agency_name dcterms:description "Property. Model:'https://schema.org/Text'. The agency_name field contains the full name of the transit agency. SameAs: 'agency_name' field from GTFS Static Field Definition - agency.txt (https://developers.google.com/transit/gtfs/reference#agencytxt)";
    rdf:type rdf:Property;
    rdfs:label "agency_name";
    rdfs:domain <https://smart-data-models.github.io/dataModel.Transportation/BikeHireDockingStation/schema.json>;
    rdfs:range xsd:string.
sdm:stationCode dcterms:description "Property. Model:'https://schema.org/Text'. The station number or station code of the bike hire docking station corresponding to the observation.";
    rdf:type rdf:Property;
    rdfs:label "stationCode";
    rdfs:domain <https://smart-data-models.github.io/dataModel.Transportation/BikeHireDockingStation/schema.json>;
    rdfs:range xsd:string.
sdm:observationDateTime dcterms:description "Property. Model:'https://schema.org/Text'. Last reported time of observation.";
    rdf:type rdf:Property;
    rdfs:label "observationDateTime";
    rdfs:domain <https://smart-data-models.github.io/dataModel.Transportation/BikeHireDockingStation/schema.json>;
    rdfs:range xsd:dateTime.
sdm:agency_fare_url dcterms:description "Property. URL of a web page that contains the details of the fares and also could allow to purchase tickets for that agency online. SameAs: 'agency_fare_url' field from GTFS Static Field Definition - agency.txt (https://developers.google.com/transit/gtfs/reference#agencytxt) ";
    rdf:type rdf:Property;
    rdfs:label "agency_fare_url";
    rdfs:domain <https://smart-data-models.github.io/dataModel.Transportation/BikeHireDockingStation/schema.json>;
    rdfs:range xsd:string.
