@prefix schema: <https://schema.org/>.
@prefix skos: <http://www.w3.org/2004/02/skos/core#>.
@prefix rdf: <http://www.w3.org/1999/02/22-rdf-syntax-ns#>.
@prefix rdfs: <http://www.w3.org/2000/01/rdf-schema#>.
@prefix foaf: <http://xmlns.com/foaf/0.1/>.
@prefix xsd: <http://www.w3.org/2001/XMLSchema#>.
@prefix dcterms: <http://purl.org/dc/terms/>.
@prefix owl: <http://www.w3.org/2002/07/owl#>.
@prefix jsonsc: <https://www.w3.org/2019/wot/json-schema#>.
@prefix jsonsc-ld: <http://w3id.org/jsonsc-ld/>.
@prefix api: <http://purl.org/linked-data/api/vocab>.
@prefix geo: <http://www.w3.org/2003/01/geo/wgs84_pos#>.
@prefix mobivoc: <http://schema.mobivoc.org/#>.
@prefix geosparql: <http://www.opengis.net/ont/geosparql#>.
@prefix sdm: <https://w3id.org/sdm#>.

<https://smart-data-models.github.io/dataModels.CIMEnergyClasses/LoadResponseCharacteristic/schema.json> dcterms:title " Smart Data Models - LoadResponseCharacteristic";
    dcterms:description "Adapted from CIM data models. Models the characteristic response of the load demand due to changes in system conditions such as voltage and frequency. This is not related to demand response.  If LoadResponseCharacteristic.exponentModel is True, the voltage exponents are specified and used as to calculate:  Active power component = Pnominal * (Voltage/cim:BaseVoltage.nominalVoltage) ** cim:LoadResponseCharacteristic.pVoltageExponent  Reactive power component = Qnominal * (Voltage/cim:BaseVoltage.nominalVoltage)** cim:LoadResponseCharacteristic.qVoltageExponent  Where  * means 'multiply' and ** is 'raised to power of'.".
sdm:type dcterms:description "Property. NGSI type. It has to be LoadResponseCharacteristic";
    rdf:type rdf:Property;
    rdfs:label "type";
    rdfs:domain <https://smart-data-models.github.io/dataModels.CIMEnergyClasses/LoadResponseCharacteristic/schema.json>.
sdm:Type rdf:type skos:ConceptScheme.
sdm:type rdfs:range [
  owl:oneOf (sdm:LoadResponseCharacteristic)
].
sdm:LoadResponseCharacteristic rdf:type skos:Concept;
    skos:inScheme sdm:Type;
    rdfs:label "LoadResponseCharacteristic".
sdm:EnergyConsumer dcterms:description "Property. Model:'https://schema.org/Number'. The set of loads that have the response characteristics. Default: 'list'";
    rdf:type rdf:Property;
    rdfs:label "EnergyConsumer";
    rdfs:domain <https://smart-data-models.github.io/dataModels.CIMEnergyClasses/LoadResponseCharacteristic/schema.json>;
    rdfs:range xsd:decimal.
sdm:exponentModel dcterms:description "Property. Model:'https://schema.org/Number'. Indicates the exponential voltage dependency model is to be used.   If false, the coefficient model is to be used. The exponential voltage dependency model consist of the attributes - pVoltageExponent - qVoltageExponent. The coefficient model consist of the attributes - pConstantImpedance - pConstantCurrent - pConstantPower - qConstantImpedance - qConstantCurrent - qConstantPower. The sum of pConstantImpedance, pConstantCurrent and pConstantPower shall equal 1. The sum of qConstantImpedance, qConstantCurrent and qConstantPower shall equal 1. Default: False";
    rdf:type rdf:Property;
    rdfs:label "exponentModel";
    rdfs:domain <https://smart-data-models.github.io/dataModels.CIMEnergyClasses/LoadResponseCharacteristic/schema.json>;
    rdfs:range xsd:decimal.
sdm:pConstantCurrent dcterms:description "Property. Model:'https://schema.org/Number'. Portion of active power load modeled as constant current. Default: 0.0";
    rdf:type rdf:Property;
    rdfs:label "pConstantCurrent";
    rdfs:domain <https://smart-data-models.github.io/dataModels.CIMEnergyClasses/LoadResponseCharacteristic/schema.json>;
    rdfs:range xsd:decimal.
sdm:pConstantImpedance dcterms:description "Property. Model:'https://schema.org/Number'. Portion of active power load modeled as constant impedance. Default: 0.0";
    rdf:type rdf:Property;
    rdfs:label "pConstantImpedance";
    rdfs:domain <https://smart-data-models.github.io/dataModels.CIMEnergyClasses/LoadResponseCharacteristic/schema.json>;
    rdfs:range xsd:decimal.
sdm:pConstantPower dcterms:description "Property. Model:'https://schema.org/Number'. Portion of active power load modeled as constant power. Default: 0.0";
    rdf:type rdf:Property;
    rdfs:label "pConstantPower";
    rdfs:domain <https://smart-data-models.github.io/dataModels.CIMEnergyClasses/LoadResponseCharacteristic/schema.json>;
    rdfs:range xsd:decimal.
sdm:pFrequencyExponent dcterms:description "Property. Model:'https://schema.org/Number'. Exponent of per unit frequency effecting active power. Default: 0.0";
    rdf:type rdf:Property;
    rdfs:label "pFrequencyExponent";
    rdfs:domain <https://smart-data-models.github.io/dataModels.CIMEnergyClasses/LoadResponseCharacteristic/schema.json>;
    rdfs:range xsd:decimal.
sdm:pVoltageExponent dcterms:description "Property. Model:'https://schema.org/Number'. Exponent of per unit voltage effecting real power. Default: 0.0";
    rdf:type rdf:Property;
    rdfs:label "pVoltageExponent";
    rdfs:domain <https://smart-data-models.github.io/dataModels.CIMEnergyClasses/LoadResponseCharacteristic/schema.json>;
    rdfs:range xsd:decimal.
sdm:qConstantCurrent dcterms:description "Property. Model:'https://schema.org/Number'. Portion of reactive power load modeled as constant current. Default: 0.0";
    rdf:type rdf:Property;
    rdfs:label "qConstantCurrent";
    rdfs:domain <https://smart-data-models.github.io/dataModels.CIMEnergyClasses/LoadResponseCharacteristic/schema.json>;
    rdfs:range xsd:decimal.
sdm:qConstantImpedance dcterms:description "Property. Model:'https://schema.org/Number'. Portion of reactive power load modeled as constant impedance. Default: 0.0";
    rdf:type rdf:Property;
    rdfs:label "qConstantImpedance";
    rdfs:domain <https://smart-data-models.github.io/dataModels.CIMEnergyClasses/LoadResponseCharacteristic/schema.json>;
    rdfs:range xsd:decimal.
sdm:qConstantPower dcterms:description "Property. Model:'https://schema.org/Number'. Portion of reactive power load modeled as constant power. Default: 0.0";
    rdf:type rdf:Property;
    rdfs:label "qConstantPower";
    rdfs:domain <https://smart-data-models.github.io/dataModels.CIMEnergyClasses/LoadResponseCharacteristic/schema.json>;
    rdfs:range xsd:decimal.
sdm:qFrequencyExponent dcterms:description "Property. Model:'https://schema.org/Number'. Exponent of per unit frequency effecting reactive power. Default: 0.0";
    rdf:type rdf:Property;
    rdfs:label "qFrequencyExponent";
    rdfs:domain <https://smart-data-models.github.io/dataModels.CIMEnergyClasses/LoadResponseCharacteristic/schema.json>;
    rdfs:range xsd:decimal.
sdm:qVoltageExponent dcterms:description "Property. Model:'https://schema.org/Number'. Exponent of per unit voltage effecting reactive power. Default: 0.0";
    rdf:type rdf:Property;
    rdfs:label "qVoltageExponent";
    rdfs:domain <https://smart-data-models.github.io/dataModels.CIMEnergyClasses/LoadResponseCharacteristic/schema.json>;
    rdfs:range xsd:decimal.
