@prefix schema: <https://schema.org/>.
@prefix skos: <http://www.w3.org/2004/02/skos/core#>.
@prefix rdf: <http://www.w3.org/1999/02/22-rdf-syntax-ns#>.
@prefix rdfs: <http://www.w3.org/2000/01/rdf-schema#>.
@prefix foaf: <http://xmlns.com/foaf/0.1/>.
@prefix xsd: <http://www.w3.org/2001/XMLSchema#>.
@prefix dcterms: <http://purl.org/dc/terms/>.
@prefix owl: <http://www.w3.org/2002/07/owl#>.
@prefix jsonsc: <https://www.w3.org/2019/wot/json-schema#>.
@prefix jsonsc-ld: <http://w3id.org/jsonsc-ld/>.
@prefix api: <http://purl.org/linked-data/api/vocab>.
@prefix geo: <http://www.w3.org/2003/01/geo/wgs84_pos#>.
@prefix mobivoc: <http://schema.mobivoc.org/#>.
@prefix geosparql: <http://www.opengis.net/ont/geosparql#>.
@prefix sdm: <https://w3id.org/sdm#>.

<https://smart-data-models.github.io/dataModel.Aeronautics/Aircraft/schema.json> dcterms:title "Smart Data models - Aircraft schema";
    dcterms:description "Represent a generic aircraft".
sdm:type dcterms:description "Property. NGSI Entity type. It has to be Aircraft";
    rdf:type rdf:Property;
    rdfs:label "type";
    rdfs:domain <https://smart-data-models.github.io/dataModel.Aeronautics/Aircraft/schema.json>.
sdm:Type rdf:type skos:ConceptScheme.
sdm:type rdfs:range [
  owl:oneOf (sdm:Aircraft)
].
sdm:Aircraft rdf:type skos:Concept;
    skos:inScheme sdm:Type;
    rdfs:label "Aircraft".
sdm:registration dcterms:description "Property. Model:'http://schema.org/Text'. Tail number or aircraft registration";
    rdf:type rdf:Property;
    rdfs:label "registration";
    rdfs:domain <https://smart-data-models.github.io/dataModel.Aeronautics/Aircraft/schema.json>;
    rdfs:range xsd:string.
sdm:speed dcterms:description "Property. Model:'http://schema.org/Number'. Current aircraft speed in kilometres per hour. Units:'kilometres per hour'";
    rdf:type rdf:Property;
    rdfs:label "speed";
    rdfs:domain <https://smart-data-models.github.io/dataModel.Aeronautics/Aircraft/schema.json>;
    rdfs:range xsd:decimal.
sdm:verticalSpeed dcterms:description "Property. Model:'http://schema.org/Number'. Current vertical aircraft speed in metres per second. Units:'metres per second'";
    rdf:type rdf:Property;
    rdfs:label "verticalSpeed";
    rdfs:domain <https://smart-data-models.github.io/dataModel.Aeronautics/Aircraft/schema.json>;
    rdfs:range xsd:decimal.
sdm:isOnGround dcterms:description "Property. Model:'http://schema.org/Boolean'. Logical indicator that determines if an aircraft is on ground";
    rdf:type rdf:Property;
    rdfs:label "isOnGround";
    rdfs:domain <https://smart-data-models.github.io/dataModel.Aeronautics/Aircraft/schema.json>;
    rdfs:range xsd:boolean.
sdm:heading dcterms:description "Property. Model:'http://schema.org/Number'. Current aircraft heading in degrees. Untis: 'degrees'";
    rdf:type rdf:Property;
    rdfs:label "heading";
    rdfs:domain <https://smart-data-models.github.io/dataModel.Aeronautics/Aircraft/schema.json>;
    rdfs:range xsd:decimal.
sdm:dateIssued dcterms:description "Property. Model:'http://schema.org/DateTime'. Date when the meassure was taken";
    rdf:type rdf:Property;
    rdfs:label "dateIssued";
    rdfs:domain <https://smart-data-models.github.io/dataModel.Aeronautics/Aircraft/schema.json>;
    rdfs:range xsd:dateTime.
sdm:belongsToAircraftModel dcterms:description "Relationship. Reference to the aircraft model entity";
    rdf:type rdf:Property;
    rdfs:label "belongsToAircraftModel";
    rdfs:domain <https://smart-data-models.github.io/dataModel.Aeronautics/Aircraft/schema.json>.
