@prefix schema: <https://schema.org/>.
@prefix skos: <http://www.w3.org/2004/02/skos/core#>.
@prefix rdf: <http://www.w3.org/1999/02/22-rdf-syntax-ns#>.
@prefix rdfs: <http://www.w3.org/2000/01/rdf-schema#>.
@prefix foaf: <http://xmlns.com/foaf/0.1/>.
@prefix xsd: <http://www.w3.org/2001/XMLSchema#>.
@prefix dcterms: <http://purl.org/dc/terms/>.
@prefix owl: <http://www.w3.org/2002/07/owl#>.
@prefix jsonsc: <https://www.w3.org/2019/wot/json-schema#>.
@prefix jsonsc-ld: <http://w3id.org/jsonsc-ld/>.
@prefix api: <http://purl.org/linked-data/api/vocab>.
@prefix geo: <http://www.w3.org/2003/01/geo/wgs84_pos#>.
@prefix mobivoc: <http://schema.mobivoc.org/#>.
@prefix geosparql: <http://www.opengis.net/ont/geosparql#>.
@prefix sdm: <https://w3id.org/sdm#>.

<https://smart-data-models.github.io/dataModel.Agrifood/Pen/schema.json> dcterms:title " Smart Data models - Pen schema";
    dcterms:description "Fenced area in a building or department or outside housing a group of animals. Animals in a pen can move and interact freely. Pens are often not completely separated from each other (half walls, iron bars, fences,â€¦), making it possible that animals from neighbouring pens can see/touch".
sdm:type dcterms:description "Property. NGSI Entity type. it has to be Pen";
    rdf:type rdf:Property;
    rdfs:label "type";
    rdfs:domain <https://smart-data-models.github.io/dataModel.Agrifood/Pen/schema.json>.
sdm:Type rdf:type skos:ConceptScheme.
sdm:type rdfs:range [
  owl:oneOf (sdm:Pen)
].
sdm:Pen rdf:type skos:Concept;
    skos:inScheme sdm:Type;
    rdfs:label "Pen".
sdm:additionalInfo dcterms:description "Property. list of all the raw values sent by the sensor/platform with all the possible extra properties that are not included in the main structure. It is a JSON structure similar to this: {'name': 'temperature', 'value' : 32}";
    rdf:type rdf:Property;
    rdfs:label "additionalInfo";
    rdfs:domain <https://smart-data-models.github.io/dataModel.Agrifood/Pen/schema.json>;
    rdfs:range sdm:AdditionalInfo.
sdm:AdditionalInfo rdf:type rdfs:Class;
    rdfs:label "AdditionalInfo".
sdm:name rdf:type rdf:Property;
    rdfs:label "name";
    rdfs:domain sdm:AdditionalInfo;
    rdfs:range xsd:string.
sdm:value rdf:type rdf:Property;
    rdfs:label "value";
    rdfs:domain sdm:AdditionalInfo.
sdm:arrivalTimestamp dcterms:description "Property. Model:'https://schema.org/DateTime'. Date and Time for the arrival of animals to the Pen";
    rdf:type rdf:Property;
    rdfs:label "arrivalTimestamp";
    rdfs:domain <https://smart-data-models.github.io/dataModel.Agrifood/Pen/schema.json>;
    rdfs:range xsd:dateTime.
sdm:avgGrowth dcterms:description "Property. Model:'https://schema.org/Number'. The average growth in weight of the animal in this pen";
    rdf:type rdf:Property;
    rdfs:label "avgGrowth";
    rdfs:domain <https://smart-data-models.github.io/dataModel.Agrifood/Pen/schema.json>;
    rdfs:range xsd:decimal.
sdm:avgWeight dcterms:description "Property. Units:'Kg'. Model:'https://schema.org/Number'. The average weight of the animal in this Pen. ";
    rdf:type rdf:Property;
    rdfs:label "avgWeight";
    rdfs:domain <https://smart-data-models.github.io/dataModel.Agrifood/Pen/schema.json>;
    rdfs:range xsd:decimal.
sdm:buildingId dcterms:description "Relationship. Unique identifier of the Building the item is located in. Model:'https://schema.org/URL'.";
    rdf:type rdf:Property;
    rdfs:label "buildingId";
    rdfs:domain <https://smart-data-models.github.io/dataModel.Agrifood/Pen/schema.json>.
sdm:co2 dcterms:description "Property. Model:'https://schema.org/Number'. The CO2 concentration in the item";
    rdf:type rdf:Property;
    rdfs:label "co2";
    rdfs:domain <https://smart-data-models.github.io/dataModel.Agrifood/Pen/schema.json>;
    rdfs:range xsd:decimal.
sdm:companyId dcterms:description "Relationship. Model:'https://schema.org/URL'. Unique identifier of a company";
    rdf:type rdf:Property;
    rdfs:label "companyId";
    rdfs:domain <https://smart-data-models.github.io/dataModel.Agrifood/Pen/schema.json>.
sdm:compartmentId dcterms:description "Relationship. Model:'https://schema.org/URL'. Unique identifier of the Compartment the Pen is located in.";
    rdf:type rdf:Property;
    rdfs:label "compartmentId";
    rdfs:domain <https://smart-data-models.github.io/dataModel.Agrifood/Pen/schema.json>.
sdm:deadAnimalsSinceDateOfArrival dcterms:description "Property. Model:'https://schema.org/Number'. Number of dead animals since the date of arrival";
    rdf:type rdf:Property;
    rdfs:label "deadAnimalsSinceDateOfArrival";
    rdfs:domain <https://smart-data-models.github.io/dataModel.Agrifood/Pen/schema.json>;
    rdfs:range xsd:decimal.
sdm:farmId dcterms:description "Relationship. Model:'https://schema.org/URL'. Unique identifier of the Farm the Pen is located in.";
    rdf:type rdf:Property;
    rdfs:label "farmId";
    rdfs:domain <https://smart-data-models.github.io/dataModel.Agrifood/Pen/schema.json>.
sdm:feedConsumption dcterms:description "Property. Model:'https://schema.org/Number'. The total amount of food that has been eaten from the feeding station(s) in the pen.It is measured through feed intakes and specific structure to let only one animal at a time to eat. Units:'Kg'";
    rdf:type rdf:Property;
    rdfs:label "feedConsumption";
    rdfs:domain <https://smart-data-models.github.io/dataModel.Agrifood/Pen/schema.json>;
    rdfs:range xsd:decimal.
sdm:humidity dcterms:description "Property. Model:'https://schema.org/Number'. Quantity representing the amount of water vapour in the atmosphere in the pen. ";
    rdf:type rdf:Property;
    rdfs:label "humidity";
    rdfs:domain <https://smart-data-models.github.io/dataModel.Agrifood/Pen/schema.json>;
    rdfs:range xsd:decimal.
sdm:lastUpdate dcterms:description "Property. Model:'https://schema.org/DateTime'. Date and time at which the measurements in the item were taken. Units:'Seconds'";
    rdf:type rdf:Property;
    rdfs:label "lastUpdate";
    rdfs:domain <https://smart-data-models.github.io/dataModel.Agrifood/Pen/schema.json>;
    rdfs:range xsd:dateTime.
sdm:luminosity dcterms:description "Property. Model:'https://schema.org/Number'. The brightness of a light source of a certain wavelength at the item. Units:'LUX'";
    rdf:type rdf:Property;
    rdfs:label "luminosity";
    rdfs:domain <https://smart-data-models.github.io/dataModel.Agrifood/Pen/schema.json>;
    rdfs:range xsd:decimal.
sdm:numAnimals dcterms:description "Property. Model:'https://schema.org/Number'. Number of animals contained in the Pen.";
    rdf:type rdf:Property;
    rdfs:label "numAnimals";
    rdfs:domain <https://smart-data-models.github.io/dataModel.Agrifood/Pen/schema.json>;
    rdfs:range xsd:decimal.
sdm:sex dcterms:description "Property. Model:'https://schema.org/Number'. The sex of the animals contained in the pen";
    rdf:type rdf:Property;
    rdfs:label "sex";
    rdfs:domain <https://smart-data-models.github.io/dataModel.Agrifood/Pen/schema.json>.
sdm:Sex rdf:type skos:ConceptScheme.
sdm:sex rdfs:range [
  owl:oneOf (sdm:M sdm:F sdm:unknown sdm:)
].
sdm:M rdf:type skos:Concept;
    skos:inScheme sdm:Sex;
    rdfs:label "M".
sdm:F rdf:type skos:Concept;
    skos:inScheme sdm:Sex;
    rdfs:label "F".
sdm:unknown rdf:type skos:Concept;
    skos:inScheme sdm:Sex;
    rdfs:label "unknown".
sdm: rdf:type skos:Concept;
    skos:inScheme sdm:Sex;
    rdfs:label "".
sdm:temperature dcterms:description "Property. Model:'https://schema.org/Number'. Temperature of the Pen.  Unirs:' Celsius degree'";
    rdf:type rdf:Property;
    rdfs:label "temperature";
    rdfs:domain <https://smart-data-models.github.io/dataModel.Agrifood/Pen/schema.json>;
    rdfs:range xsd:decimal.
sdm:waterConsumption dcterms:description "Property. Model:'https://schema.org/Number'. The total amount of water that came out from the tap or taps in the pen. It is measured through flowmeters and specific structure to let only one animal at a time drink.";
    rdf:type rdf:Property;
    rdfs:label "waterConsumption";
    rdfs:domain <https://smart-data-models.github.io/dataModel.Agrifood/Pen/schema.json>;
    rdfs:range xsd:decimal.
sdm:weightStDev dcterms:description "Property. Model:'https://schema.org/Number'. The standard deviation associated to the average weight of the animals contained in the Pen.";
    rdf:type rdf:Property;
    rdfs:label "weightStDev";
    rdfs:domain <https://smart-data-models.github.io/dataModel.Agrifood/Pen/schema.json>;
    rdfs:range xsd:decimal.
