@prefix schema: <https://schema.org/>.
@prefix skos: <http://www.w3.org/2004/02/skos/core#>.
@prefix rdf: <http://www.w3.org/1999/02/22-rdf-syntax-ns#>.
@prefix rdfs: <http://www.w3.org/2000/01/rdf-schema#>.
@prefix foaf: <http://xmlns.com/foaf/0.1/>.
@prefix xsd: <http://www.w3.org/2001/XMLSchema#>.
@prefix dcterms: <http://purl.org/dc/terms/>.
@prefix owl: <http://www.w3.org/2002/07/owl#>.
@prefix jsonsc: <https://www.w3.org/2019/wot/json-schema#>.
@prefix jsonsc-ld: <http://w3id.org/jsonsc-ld/>.
@prefix api: <http://purl.org/linked-data/api/vocab>.
@prefix geo: <http://www.w3.org/2003/01/geo/wgs84_pos#>.
@prefix mobivoc: <http://schema.mobivoc.org/#>.
@prefix geosparql: <http://www.opengis.net/ont/geosparql#>.
@prefix sdm: <https://w3id.org/sdm#>.

<https://smart-data-models.github.io/datamodel.Transportation/FleetVehicle/schema.json> dcterms:title "Smart Data models - Fleet-Vehicle schema";
    dcterms:description "This entity contains a harmonised description of a generic fleet vehicle such as a delivery vehicle, an ambulance or a postal vehicle. This entity is primarily associated with the vertical segment of the transport and logistics but may also be used many other related IoT applications.".
sdm:type dcterms:description "Property. NGSI Entity identifier. It has to be FleetVehicle";
    rdf:type rdf:Property;
    rdfs:label "type";
    rdfs:domain <https://smart-data-models.github.io/datamodel.Transportation/FleetVehicle/schema.json>.
sdm:Type rdf:type skos:ConceptScheme.
sdm:type rdfs:range [
  owl:oneOf (sdm:FleetVehicle)
].
sdm:FleetVehicle rdf:type skos:Concept;
    skos:inScheme sdm:Type;
    rdfs:label "FleetVehicle".
sdm:vehicle dcterms:description "Relationship. Reference to the related Vehicle entity instance that describes the core attributes of this Fleet Vehicle.";
    rdf:type rdf:Property;
    rdfs:label "vehicle";
    rdfs:domain <https://smart-data-models.github.io/datamodel.Transportation/FleetVehicle/schema.json>.
sdm:fleetVehicleType dcterms:description "Property. The type of the Vehicle for example (not limited to) these ones. Enum:'Taxi, Ambulance, Postal, Fire & Rescue, Delivery'";
    rdf:type rdf:Property;
    rdfs:label "fleetVehicleType";
    rdfs:domain <https://smart-data-models.github.io/datamodel.Transportation/FleetVehicle/schema.json>;
    rdfs:range xsd:string.
sdm:operatingCompany dcterms:description "Property. Details of the organization that is operating this fleet vehicle. Based on Schema.org organization. Model:'https://schema.org/Organization'";
    rdf:type rdf:Property;
    rdfs:label "operatingCompany";
    rdfs:domain <https://smart-data-models.github.io/datamodel.Transportation/FleetVehicle/schema.json>;
    rdfs:range xsd:string.
sdm:operator dcterms:description "Relationship. The usual operator/driver/keeper of this fleet vehicle encoded as a Schema.org person. Model:'https://schema.org/Person'";
    rdf:type rdf:Property;
    rdfs:label "operator";
    rdfs:domain <https://smart-data-models.github.io/datamodel.Transportation/FleetVehicle/schema.json>.
