@prefix schema: <https://schema.org/>.
@prefix skos: <http://www.w3.org/2004/02/skos/core#>.
@prefix rdf: <http://www.w3.org/1999/02/22-rdf-syntax-ns#>.
@prefix rdfs: <http://www.w3.org/2000/01/rdf-schema#>.
@prefix foaf: <http://xmlns.com/foaf/0.1/>.
@prefix xsd: <http://www.w3.org/2001/XMLSchema#>.
@prefix dcterms: <http://purl.org/dc/terms/>.
@prefix owl: <http://www.w3.org/2002/07/owl#>.
@prefix jsonsc: <https://www.w3.org/2019/wot/json-schema#>.
@prefix jsonsc-ld: <http://w3id.org/jsonsc-ld/>.
@prefix api: <http://purl.org/linked-data/api/vocab>.
@prefix geo: <http://www.w3.org/2003/01/geo/wgs84_pos#>.
@prefix mobivoc: <http://schema.mobivoc.org/#>.
@prefix geosparql: <http://www.opengis.net/ont/geosparql#>.
@prefix sdm: <https://w3id.org/sdm#>.

<https://raw.githubusercontent.com/smart-data-models/dataModel.CallComplaints/master/Complaint/schema.json> dcterms:title "Call Complaints - Complaint";
    dcterms:description "This entity contains a harmonised description of a generic Complaint made for the Call Complaints domain.".
sdm:type dcterms:description "Property. NGSI Entity Type. It must be equal to Complaint.";
    rdf:type rdf:Property;
    rdfs:label "type";
    rdfs:domain <https://raw.githubusercontent.com/smart-data-models/dataModel.CallComplaints/master/Complaint/schema.json>.
sdm:Type rdf:type skos:ConceptScheme.
sdm:type rdfs:range [
  owl:oneOf (sdm:Complaint)
].
sdm:Complaint rdf:type skos:Concept;
    skos:inScheme sdm:Type;
    rdfs:label "Complaint".
sdm:status dcterms:description "Property. Status of the Complaint. Examples: Pending, In progress.";
    rdf:type rdf:Property;
    rdfs:label "status";
    rdfs:domain <https://raw.githubusercontent.com/smart-data-models/dataModel.CallComplaints/master/Complaint/schema.json>;
    rdfs:range xsd:string.
sdm:timestamp dcterms:description "Property. Model:'https://schema.org/DateTime'. The timestamp of the Complaint.";
    rdf:type rdf:Property;
    rdfs:label "timestamp";
    rdfs:domain <https://raw.githubusercontent.com/smart-data-models/dataModel.CallComplaints/master/Complaint/schema.json>;
    rdfs:range xsd:dateTime.
sdm:category dcterms:description "Property. Model:'https://schema.org/Text'. The category of the Complaint. Examples:Brown water, Particles, Odor / Taste, Illness, Meter leak, Network leak, No water, Low pressure, High pressure, Broken switch, Water quality, Waste of water, Broken meter, Meter repositioning, Sidewalk repair, Pavement repair.";
    rdf:type rdf:Property;
    rdfs:label "category";
    rdfs:domain <https://raw.githubusercontent.com/smart-data-models/dataModel.CallComplaints/master/Complaint/schema.json>;
    rdfs:range xsd:string.
sdm:isMadeBy dcterms:description "Relationship. The Id of the User that made this Complaint.";
    rdf:type rdf:Property;
    rdfs:label "isMadeBy";
    rdfs:domain <https://raw.githubusercontent.com/smart-data-models/dataModel.CallComplaints/master/Complaint/schema.json>.
sdm:isPartOf dcterms:description "Property. Unique identifier of the entity";
    rdf:type rdf:Property;
    rdfs:label "isPartOf";
    rdfs:domain <https://raw.githubusercontent.com/smart-data-models/dataModel.CallComplaints/master/Complaint/schema.json>.
sdm:isFiledTo dcterms:description "Relationship. The ID of the Organization (e.g., Complaints Department), that this Complaint is filed to.";
    rdf:type rdf:Property;
    rdfs:label "isFiledTo";
    rdfs:domain <https://raw.githubusercontent.com/smart-data-models/dataModel.CallComplaints/master/Complaint/schema.json>.
