@prefix schema: <https://schema.org/>.
@prefix skos: <http://www.w3.org/2004/02/skos/core#>.
@prefix rdf: <http://www.w3.org/1999/02/22-rdf-syntax-ns#>.
@prefix rdfs: <http://www.w3.org/2000/01/rdf-schema#>.
@prefix foaf: <http://xmlns.com/foaf/0.1/>.
@prefix xsd: <http://www.w3.org/2001/XMLSchema#>.
@prefix dcterms: <http://purl.org/dc/terms/>.
@prefix owl: <http://www.w3.org/2002/07/owl#>.
@prefix jsonsc: <https://www.w3.org/2019/wot/json-schema#>.
@prefix jsonsc-ld: <http://w3id.org/jsonsc-ld/>.
@prefix api: <http://purl.org/linked-data/api/vocab>.
@prefix geo: <http://www.w3.org/2003/01/geo/wgs84_pos#>.
@prefix mobivoc: <http://schema.mobivoc.org/#>.
@prefix geosparql: <http://www.opengis.net/ont/geosparql#>.
@prefix sdm: <https://w3id.org/sdm#>.

<https://smart-data-models.github.io/dataModels.CIMEnergyClasses/GovSteam0/schema.json> dcterms:title " Smart Data Models - GovSteam0";
    dcterms:description "Adapted from CIM data models. A simplified steam turbine governor model.".
sdm:type dcterms:description "Property. NGSI type. It has to be GovSteam0";
    rdf:type rdf:Property;
    rdfs:label "type";
    rdfs:domain <https://smart-data-models.github.io/dataModels.CIMEnergyClasses/GovSteam0/schema.json>.
sdm:Type rdf:type skos:ConceptScheme.
sdm:type rdfs:range [
  owl:oneOf (sdm:GovSteam0)
].
sdm:GovSteam0 rdf:type skos:Concept;
    skos:inScheme sdm:Type;
    rdfs:label "GovSteam0".
sdm:dt dcterms:description "Property. Model:'https://schema.org/Number'. Turbine damping coefficient (Dt).  Unit = delta P / delta speed. Typical Value = 0. Default: 0.0";
    rdf:type rdf:Property;
    rdfs:label "dt";
    rdfs:domain <https://smart-data-models.github.io/dataModels.CIMEnergyClasses/GovSteam0/schema.json>;
    rdfs:range xsd:decimal.
sdm:mwbase dcterms:description "Property. Model:'https://schema.org/Number'. Base for power values (MWbase)  (>0).  Unit = MW. Default: 0.0";
    rdf:type rdf:Property;
    rdfs:label "mwbase";
    rdfs:domain <https://smart-data-models.github.io/dataModels.CIMEnergyClasses/GovSteam0/schema.json>;
    rdfs:range xsd:decimal.
sdm:r dcterms:description "Property. Model:'https://schema.org/Number'. Permanent droop (R).  Typical Value = 0.05. Default: 0.0";
    rdf:type rdf:Property;
    rdfs:label "r";
    rdfs:domain <https://smart-data-models.github.io/dataModels.CIMEnergyClasses/GovSteam0/schema.json>;
    rdfs:range xsd:decimal.
sdm:t1 dcterms:description "Property. Model:'https://schema.org/Number'. Steam bowl time constant (T1).  Typical Value = 0.5. Default: 0";
    rdf:type rdf:Property;
    rdfs:label "t1";
    rdfs:domain <https://smart-data-models.github.io/dataModels.CIMEnergyClasses/GovSteam0/schema.json>;
    rdfs:range xsd:decimal.
sdm:t2 dcterms:description "Property. Model:'https://schema.org/Number'. Numerator time constant of T2/T3 block (T2).  Typical Value = 3. Default: 0";
    rdf:type rdf:Property;
    rdfs:label "t2";
    rdfs:domain <https://smart-data-models.github.io/dataModels.CIMEnergyClasses/GovSteam0/schema.json>;
    rdfs:range xsd:decimal.
sdm:t3 dcterms:description "Property. Model:'https://schema.org/Number'. Reheater time constant (T3).  Typical Value = 10. Default: 0";
    rdf:type rdf:Property;
    rdfs:label "t3";
    rdfs:domain <https://smart-data-models.github.io/dataModels.CIMEnergyClasses/GovSteam0/schema.json>;
    rdfs:range xsd:decimal.
sdm:vmax dcterms:description "Property. Model:'https://schema.org/Number'. Maximum valve position, PU of mwcap (Vmax).  Typical Value = 1. Default: 0.0";
    rdf:type rdf:Property;
    rdfs:label "vmax";
    rdfs:domain <https://smart-data-models.github.io/dataModels.CIMEnergyClasses/GovSteam0/schema.json>;
    rdfs:range xsd:decimal.
sdm:vmin dcterms:description "Property. Model:'https://schema.org/Number'. Minimum valve position, PU of mwcap (Vmin).  Typical Value = 0. Default: 0.0";
    rdf:type rdf:Property;
    rdfs:label "vmin";
    rdfs:domain <https://smart-data-models.github.io/dataModels.CIMEnergyClasses/GovSteam0/schema.json>;
    rdfs:range xsd:decimal.
