@prefix schema: <https://schema.org/>.
@prefix skos: <http://www.w3.org/2004/02/skos/core#>.
@prefix rdf: <http://www.w3.org/1999/02/22-rdf-syntax-ns#>.
@prefix rdfs: <http://www.w3.org/2000/01/rdf-schema#>.
@prefix foaf: <http://xmlns.com/foaf/0.1/>.
@prefix xsd: <http://www.w3.org/2001/XMLSchema#>.
@prefix dcterms: <http://purl.org/dc/terms/>.
@prefix owl: <http://www.w3.org/2002/07/owl#>.
@prefix jsonsc: <https://www.w3.org/2019/wot/json-schema#>.
@prefix jsonsc-ld: <http://w3id.org/jsonsc-ld/>.
@prefix api: <http://purl.org/linked-data/api/vocab>.
@prefix geo: <http://www.w3.org/2003/01/geo/wgs84_pos#>.
@prefix mobivoc: <http://schema.mobivoc.org/#>.
@prefix geosparql: <http://www.opengis.net/ont/geosparql#>.
@prefix sdm: <https://w3id.org/sdm#>.

<https://raw.githubusercontent.com/smart-data-models/dataModel.SocialMedia/master/SMCollection/schema.json> dcterms:title "Social Media - SMCollection";
    dcterms:description "This entity contains a harmonised description of a generic SMCollection made for the Social Media domain. This entity is primarily associated with the process of collection of Social Media posts (primarily Twitter).".
sdm:type dcterms:description "Property. NGSI-LD Entity Type. It must be equal to SMCollection.";
    rdf:type rdf:Property;
    rdfs:label "type";
    rdfs:domain <https://raw.githubusercontent.com/smart-data-models/dataModel.SocialMedia/master/SMCollection/schema.json>.
sdm:Type rdf:type skos:ConceptScheme.
sdm:type rdfs:range [
  owl:oneOf (sdm:SMCollection)
].
sdm:SMCollection rdf:type skos:Concept;
    skos:inScheme sdm:Type;
    rdfs:label "SMCollection".
sdm:hasPosts rdf:type rdf:Property;
    rdfs:label "hasPosts";
    rdfs:domain <https://raw.githubusercontent.com/smart-data-models/dataModel.SocialMedia/master/SMCollection/schema.json>.
sdm:hasAnalysis rdf:type rdf:Property;
    rdfs:label "hasAnalysis";
    rdfs:domain <https://raw.githubusercontent.com/smart-data-models/dataModel.SocialMedia/master/SMCollection/schema.json>.
sdm:groupedAt dcterms:description "Property. The date and time of when the collection was constructed / grouped.";
    rdf:type rdf:Property;
    rdfs:label "groupedAt";
    rdfs:domain <https://raw.githubusercontent.com/smart-data-models/dataModel.SocialMedia/master/SMCollection/schema.json>;
    rdfs:range xsd:dateTime.
