@prefix schema: <https://schema.org/>.
@prefix skos: <http://www.w3.org/2004/02/skos/core#>.
@prefix rdf: <http://www.w3.org/1999/02/22-rdf-syntax-ns#>.
@prefix rdfs: <http://www.w3.org/2000/01/rdf-schema#>.
@prefix foaf: <http://xmlns.com/foaf/0.1/>.
@prefix xsd: <http://www.w3.org/2001/XMLSchema#>.
@prefix dcterms: <http://purl.org/dc/terms/>.
@prefix owl: <http://www.w3.org/2002/07/owl#>.
@prefix jsonsc: <https://www.w3.org/2019/wot/json-schema#>.
@prefix jsonsc-ld: <http://w3id.org/jsonsc-ld/>.
@prefix api: <http://purl.org/linked-data/api/vocab>.
@prefix geo: <http://www.w3.org/2003/01/geo/wgs84_pos#>.
@prefix mobivoc: <http://schema.mobivoc.org/#>.
@prefix geosparql: <http://www.opengis.net/ont/geosparql#>.
@prefix sdm: <https://w3id.org/sdm#>.

<https://smart-data-models.github.io/datamodel.COVID19/VaccinationCertificate/schema.json> dcterms:title " Smart Data Models - Vaccination Certificates";
    dcterms:description "Description of a COVID-19 Vaccination Certificate.".
sdm:type dcterms:description "Property. NSGI Entity Type. it has to be VaccinationCertificate";
    rdf:type rdf:Property;
    rdfs:label "type";
    rdfs:domain <https://smart-data-models.github.io/datamodel.COVID19/VaccinationCertificate/schema.json>.
sdm:Type rdf:type skos:ConceptScheme.
sdm:type rdfs:range [
  owl:oneOf (sdm:VaccinationCertificate)
].
sdm:VaccinationCertificate rdf:type skos:Concept;
    skos:inScheme sdm:Type;
    rdfs:label "VaccinationCertificate".
sdm:issuanceDate dcterms:description "Property. Model:'https://schema.org/DateTime'. Date and time of issuance";
    rdf:type rdf:Property;
    rdfs:label "issuanceDate";
    rdfs:domain <https://smart-data-models.github.io/datamodel.COVID19/VaccinationCertificate/schema.json>;
    rdfs:range xsd:dateTime.
sdm:expirationDate dcterms:description "Property. Model:'https://schema.org/DateTime'. Date and time of expiry";
    rdf:type rdf:Property;
    rdfs:label "expirationDate";
    rdfs:domain <https://smart-data-models.github.io/datamodel.COVID19/VaccinationCertificate/schema.json>;
    rdfs:range xsd:dateTime.
sdm:issuer dcterms:description "Relationship. Model:'http://schema.org/URL'. Identity of the issuer";
    rdf:type rdf:Property;
    rdfs:label "issuer";
    rdfs:domain <https://smart-data-models.github.io/datamodel.COVID19/VaccinationCertificate/schema.json>.
sdm:credentialSubject dcterms:description "Property. Vaccine, Vaccine Event and recipient object";
    rdf:type rdf:Property;
    rdfs:label "credentialSubject";
    rdfs:domain <https://smart-data-models.github.io/datamodel.COVID19/VaccinationCertificate/schema.json>;
    rdfs:range sdm:CredentialSubject.
sdm:CredentialSubject rdf:type rdfs:Class;
    rdfs:label "CredentialSubject".
sdm:batchNumber dcterms:description "Property. Model:'https://schema.org/Text'. A distinctive combination of numbers and/or letters which specifically identifies a batch";
    rdf:type rdf:Property;
    rdfs:label "batchNumber";
    rdfs:domain sdm:CredentialSubject;
    rdfs:range xsd:string.
sdm:administeringCentre dcterms:description "Property. Model:'https://schema.org/Text'. Name/code of administering centre or a health authority responsible for the vaccination event";
    rdf:type rdf:Property;
    rdfs:label "administeringCentre";
    rdfs:domain sdm:CredentialSubject;
    rdfs:range xsd:string.
sdm:healthProfessional dcterms:description "Property. Model:'https://schema.org/Text'. Name or health professional code responsible for administering the vaccine or prophylaxis";
    rdf:type rdf:Property;
    rdfs:label "healthProfessional";
    rdfs:domain sdm:CredentialSubject;
    rdfs:range xsd:string.
sdm:countryOfVaccination dcterms:description "Property. Model:'https://schema.org/Text'. The country in which the vaccine recipient was vaccinated";
    rdf:type rdf:Property;
    rdfs:label "countryOfVaccination";
    rdfs:domain sdm:CredentialSubject;
    rdfs:range xsd:string.
sdm:recipient dcterms:description "Property. Model:'https://schema.org/Patient'. The recipient of the vaccine";
    rdf:type rdf:Property;
    rdfs:label "recipient";
    rdfs:domain sdm:CredentialSubject;
    rdfs:range sdm:Recipient.
sdm:Recipient rdf:type rdfs:Class;
    rdfs:label "Recipient".
sdm:givenName dcterms:description "Property. Model:'https://schema.org/Text'. The non-family name with which the vaccine recipient identifies";
    rdf:type rdf:Property;
    rdfs:label "givenName";
    rdfs:domain sdm:Recipient;
    rdfs:range xsd:string.
sdm:familyName dcterms:description "Property. Model:'https://schema.org/Text'. The name of the family with which the vaccine recipient identifies";
    rdf:type rdf:Property;
    rdfs:label "familyName";
    rdfs:domain sdm:Recipient;
    rdfs:range xsd:string.
sdm:gender dcterms:description "Property. Model:'https://schema.org/Text'. Enum:'male, female, other'. The gender of the vaccine recipient";
    rdf:type rdf:Property;
    rdfs:label "gender";
    rdfs:domain sdm:Recipient.
sdm:Gender rdf:type skos:ConceptScheme.
sdm:gender rdfs:range [
  owl:oneOf (sdm:male sdm:female sdm:other)
].
sdm:male rdf:type skos:Concept;
    skos:inScheme sdm:Gender;
    rdfs:label "male".
sdm:female rdf:type skos:Concept;
    skos:inScheme sdm:Gender;
    rdfs:label "female".
sdm:other rdf:type skos:Concept;
    skos:inScheme sdm:Gender;
    rdfs:label "other".
sdm:birthDate dcterms:description "Property. Model:'https://schema.org/Date'. this rule applies to. The date on which the vaccine recipient was born";
    rdf:type rdf:Property;
    rdfs:label "birthDate";
    rdfs:domain sdm:Recipient;
    rdfs:range xsd:date.
sdm:vaccine dcterms:description "Property. Generic description of the vaccine/prophylaxis or its component(s)";
    rdf:type rdf:Property;
    rdfs:label "vaccine";
    rdfs:domain sdm:CredentialSubject;
    rdfs:range sdm:Vaccine.
sdm:Vaccine rdf:type rdfs:Class;
    rdfs:label "Vaccine".
sdm:disease dcterms:description "Property. Model:'https://schema.org/Text'. Disease or agent that the vaccination administered to the recipient provides protection against";
    rdf:type rdf:Property;
    rdfs:label "disease";
    rdfs:domain sdm:Vaccine;
    rdfs:range xsd:string.
sdm:atcCode dcterms:description "Property. Model:'https://schema.org/Text'. Anatomical Therapeutic Chemical Code";
    rdf:type rdf:Property;
    rdfs:label "atcCode";
    rdfs:domain sdm:Vaccine;
    rdfs:range xsd:string.
sdm:medicinalProductName dcterms:description "Property. Model:'https://schema.org/Text'. Medicinal product name";
    rdf:type rdf:Property;
    rdfs:label "medicinalProductName";
    rdfs:domain sdm:Vaccine;
    rdfs:range xsd:string.
sdm:marketingAuthorizationHolder dcterms:description "Property. Model:'https://schema.org/Text'. Marketing Authorization Holder";
    rdf:type rdf:Property;
    rdfs:label "marketingAuthorizationHolder";
    rdfs:domain sdm:Vaccine;
    rdfs:range xsd:string.
sdm:proof dcterms:description "Property. Proof of Immunization";
    rdf:type rdf:Property;
    rdfs:label "proof";
    rdfs:domain sdm:CredentialSubject;
    rdfs:range sdm:Proof.
sdm:Proof rdf:type rdfs:Class;
    rdfs:label "Proof".
sdm:created dcterms:description "Property. Model:'https://schema.org/DateTime'. Date and time of proof creation";
    rdf:type rdf:Property;
    rdfs:label "created";
    rdfs:domain sdm:Proof;
    rdfs:range xsd:dateTime.
sdm:proofValue dcterms:description "Property. Model:'https://schema.org/Text'. Signature, Hash or JWT value of the proof";
    rdf:type rdf:Property;
    rdfs:label "proofValue";
    rdfs:domain sdm:Proof;
    rdfs:range xsd:string.
sdm:verificationMethod dcterms:description "Relationship. Model:'http://schema.org/URL'. verificationMethod object";
    rdf:type rdf:Property;
    rdfs:label "verificationMethod";
    rdfs:domain sdm:Proof.
