@prefix schema: <https://schema.org/>.
@prefix skos: <http://www.w3.org/2004/02/skos/core#>.
@prefix rdf: <http://www.w3.org/1999/02/22-rdf-syntax-ns#>.
@prefix rdfs: <http://www.w3.org/2000/01/rdf-schema#>.
@prefix foaf: <http://xmlns.com/foaf/0.1/>.
@prefix xsd: <http://www.w3.org/2001/XMLSchema#>.
@prefix dcterms: <http://purl.org/dc/terms/>.
@prefix owl: <http://www.w3.org/2002/07/owl#>.
@prefix jsonsc: <https://www.w3.org/2019/wot/json-schema#>.
@prefix jsonsc-ld: <http://w3id.org/jsonsc-ld/>.
@prefix api: <http://purl.org/linked-data/api/vocab>.
@prefix geo: <http://www.w3.org/2003/01/geo/wgs84_pos#>.
@prefix mobivoc: <http://schema.mobivoc.org/#>.
@prefix geosparql: <http://www.opengis.net/ont/geosparql#>.
@prefix sdm: <https://w3id.org/sdm#>.

<https://smart-data-models.github.io/data-models.OpenChannelManagement/RegulationStructure/schema.json> dcterms:title "Open Channel Management - RegulationStructure";
    dcterms:description "This entity contains a harmonised description of a generic Regulation Structure made for Raw-Water (Open Channels) System Management domain. Regulation structure represents a junction-type object, controlling the water flow in the raw-water system.".
sdm:type dcterms:description "Property. NGSI-LD Entity Type. It has to be RegulationStructure";
    rdf:type rdf:Property;
    rdfs:label "type";
    rdfs:domain <https://smart-data-models.github.io/data-models.OpenChannelManagement/RegulationStructure/schema.json>.
sdm:Type rdf:type skos:ConceptScheme.
sdm:type rdfs:range [
  owl:oneOf (sdm:RegulationStructure)
].
sdm:RegulationStructure rdf:type skos:Concept;
    skos:inScheme sdm:Type;
    rdfs:label "RegulationStructure".
sdm:numberOfGates dcterms:description "Property. An integer value defining the number of control gates attached to the regulation structure.";
    rdf:type rdf:Property;
    rdfs:label "numberOfGates";
    rdfs:domain <https://smart-data-models.github.io/data-models.OpenChannelManagement/RegulationStructure/schema.json>;
    rdfs:range xsd:decimal.
sdm:numberOfSpillways dcterms:description "Property. An integer value defining the number of spillways attached to the regulation structure.";
    rdf:type rdf:Property;
    rdfs:label "numberOfSpillways";
    rdfs:domain <https://smart-data-models.github.io/data-models.OpenChannelManagement/RegulationStructure/schema.json>;
    rdfs:range xsd:decimal.
sdm:teleCommand dcterms:description "Property. Define whether the regulation structure is controlled remotely or manually. True/False value.";
    rdf:type rdf:Property;
    rdfs:label "teleCommand";
    rdfs:domain <https://smart-data-models.github.io/data-models.OpenChannelManagement/RegulationStructure/schema.json>;
    rdfs:range xsd:boolean.
sdm:hasSluiceGate dcterms:description "Relationship. Reference to an entity of type Sluice gate.";
    rdf:type rdf:Property;
    rdfs:label "hasSluiceGate";
    rdfs:domain <https://smart-data-models.github.io/data-models.OpenChannelManagement/RegulationStructure/schema.json>.
sdm:hasSpillway dcterms:description "Relationship. Reference to an entity of type Sluice gate Spillway.";
    rdf:type rdf:Property;
    rdfs:label "hasSpillway";
    rdfs:domain <https://smart-data-models.github.io/data-models.OpenChannelManagement/RegulationStructure/schema.json>.
sdm:position dcterms:description "Property. Object providing information about the distance with the rest of the elements and a relationship with them.";
    rdf:type rdf:Property;
    rdfs:label "position";
    rdfs:domain <https://smart-data-models.github.io/data-models.OpenChannelManagement/RegulationStructure/schema.json>;
    rdfs:range sdm:Position.
sdm:Position rdf:type rdfs:Class;
    rdfs:label "Position".
sdm:distance dcterms:description "Property. The distance between this Entity and a reference point (e.g., the most upstream point of the system). Units:'Km' ";
    rdf:type rdf:Property;
    rdfs:label "distance";
    rdfs:domain sdm:Position;
    rdfs:range xsd:decimal.
sdm:refPoint dcterms:description "Relationship. The reference point distance is measured from.";
    rdf:type rdf:Property;
    rdfs:label "refPoint";
    rdfs:domain sdm:Position.
