@prefix : <http://w3id.org/jsonsc-ld/> .
@prefix owl: <http://www.w3.org/2002/07/owl#> .
@prefix rdf: <http://www.w3.org/1999/02/22-rdf-syntax-ns#> .
@prefix xml: <http://www.w3.org/XML/1998/namespace> .
@prefix xsd: <http://www.w3.org/2001/XMLSchema#> .
@prefix rdfs: <http://www.w3.org/2000/01/rdf-schema#> .
@prefix dcterms: <http://purl.org/dc/terms/> .
@prefix jsonsc-ld: <http://w3id.org/jsonsc-ld/> .
@base <http://w3id.org/jsonsc-ld/> .

<http://w3id.org/jsonsc-ld/> rdf:type owl:Ontology ;
                              owl:versionIRI <http://w3id.org/jsonsc-ld/1.0> ;
                              owl:imports rdfs: ,
                                          <http://www.w3.org/2004/02/skos/core> ;
                              dcterms:creator <https://data.knows.idlab.ugent.be/person/jilong/#me> ;
                              rdfs:comment "JSON schema LD is a metadata schema vocabulary empowers JSON schema with semantics. It is needed in supporting the conversion of a JSON schema to a RDF schema (RDFS) and Shacl shapes."@en ;
                              rdfs:label "JSON schema LD"@en .

#################################################################
#    Annotation properties
#################################################################

###  http://purl.org/dc/terms/creator
dcterms:creator rdf:type owl:AnnotationProperty .


#################################################################
#    Object Properties
#################################################################

###  http://w3id.org/jsonsc-ld/datatype
jsonsc-ld:datatype rdf:type owl:ObjectProperty ;
                   rdfs:domain jsonsc-ld:Property ;
                   rdfs:range rdfs:Datatype ;
                   owl:propertyDisjointWith jsonsc-ld:range ;
                   rdfs:comment "jsonsc-ld:datatype connects a property in a JSON schema to rdfs:DataType."@en ;
                   rdfs:label "data type"@en .


###  http://w3id.org/jsonsc-ld/enriches
jsonsc-ld:enriches rdf:type owl:ObjectProperty ;
                 rdfs:domain jsonsc-ld:Schema ;
                 rdfs:range <https://www.w3.org/2019/wot/json-schema#DataSchema> ;
                 rdfs:comment "jsonsc-ld:enriches relates a jsonsc-ld:Schema to a jsonsc:DataSchema."@en ;
                 rdfs:label "enriches"@en .


###  http://w3id.org/jsonsc-ld/enum
jsonsc-ld:enum rdf:type owl:ObjectProperty ;
               rdfs:domain jsonsc-ld:Property ;
               rdfs:range <http://www.w3.org/2004/02/skos/core#ConceptScheme> ;
               rdfs:comment "jsonsc-ld:enum declares a JSON schema property, containing an array/list of enumerated items, is represented as a skos:ConceptScheme (a situational knowledge). Each enumerated item is a concept in the context of this property."@en ;
               rdfs:label "enum"@en .


###  http://w3id.org/jsonsc-ld/ignore
jsonsc-ld:ignore rdf:type owl:ObjectProperty ;
                 rdfs:domain jsonsc-ld:Schema ;
                 rdfs:range jsonsc-ld:Property ;
                 rdfs:comment "jsonsc-ld:ignore neglects a property defined in a JSON schema in the context of RDFS and Shacl conversion."@en ;
                 rdfs:label "ignore"@en .


###  http://w3id.org/jsonsc-ld/included
jsonsc-ld:included rdf:type owl:ObjectProperty ;
                   rdfs:domain jsonsc-ld:Schema ;
                   rdfs:range rdf:Property ;
                   rdfs:comment "jsonsc-ld:included is an analogous to @included in JSON-LD. It is specifically applied to handle the object of array of objects structure in the JSON schema."@en ;
                   rdfs:label "included"@en .


###  http://w3id.org/jsonsc-ld/range
jsonsc-ld:range rdf:type owl:ObjectProperty ;
                rdfs:subPropertyOf rdfs:range ;
                rdfs:domain jsonsc-ld:Property ;
                rdfs:comment "jsonsc-ld:range is a SubClass of rdfs:range. It points a jsonsc-ld:Property to an object which is not a data type."@en ;
                rdfs:label "range"@en .


#################################################################
#    Data properties
#################################################################

###  http://w3id.org/jsonsc-ld/existing
jsonsc-ld:existing rdf:type owl:DatatypeProperty ;
                   rdfs:domain jsonsc-ld:Property ;
                   rdfs:range xsd:boolean ;
                   rdfs:comment """jsonsc-ld:existing indicates whether or not a property in a JSON (sub) schema
can be represented by a term in an existing vocabulary.  It has a range of xsd:boolean data type. The default value of jsonsc-ld:existing is false, when it is not declared. If the value is set to true, the property will be enriched with the value of jsonsc-ld:id via rdfs:seeAlso."""@en ;
                   rdfs:label "existing"@en .


###  http://w3id.org/jsonsc-ld/geoJsonFeature
jsonsc-ld:geoJsonFeature rdf:type owl:DatatypeProperty ;
                         rdfs:domain jsonsc-ld:Property ;
                         rdfs:range xsd:boolean ;
                         rdfs:comment "jsonsc-ld:geoJSONFeature indicates a property in a JSON schema is a geo:Gemetry object when it is set to true."@en ;
                         rdfs:label "geoJsonFeature"@en .


#################################################################
#    Classes
#################################################################

###  http://w3id.org/jsonsc-ld/Property
jsonsc-ld:Property rdf:type owl:Class ;
                   rdfs:subClassOf rdf:Property ;
                   rdfs:comment "jsonsc-ld:Property is the class of JSON schema LD properties, which are analogous to JSON schema properties."@en ;
                   rdfs:seeAlso "Property"@en .


###  http://w3id.org/jsonsc-ld/Schema
jsonsc-ld:Schema rdf:type owl:Class ;
                 rdfs:comment "jsonsc-ld:schema defines the  RDF terms to introduce semantics to JSON schema, and hence to convert JSON schema to RDF schema constrained by SHACL shapes orignated from JSON schema."@en ;
                 rdfs:label "Schema"@en .


###  https://www.w3.org/2019/wot/json-schema#DataSchema
<https://www.w3.org/2019/wot/json-schema#DataSchema> rdf:type owl:Class .


###  Generated by the OWL API (version 4.5.9.2019-02-01T07:24:44Z) https://github.com/owlcs/owlapi
